[
  {
    "@type": "datmm:Dataset",
    "dct:description": "This data collection consists of images acquired during chemoradiotherapy of 20 locally-advanced, non-small cell lung cancer patients. The images include four-dimensional (4D) fan beam (4D-FBCT) and 4D cone beam CT (4D-CBCT). All patients underwent concurrent radiochemotherapy to a total dose of 64.8-70\u00a0Gy using daily 1.8 or 2\u00a0Gy fractions.\u00a0",
    "dct:format": "Unknown",
    "dct:issued": "2016/10/19",
    "foaf:homepage": "https://www.ncbi.nlm.nih.gov/gap",
    "dct:title": "4D-Lung",
    "dct:language": "English",
    "bf:contribution": [],
    "dct:isPartOf": {
      "@type": "datmm:Repository",
      "dct:alternative": "TCIA",
      "foaf:homepage": "https://www.cancerimagingarchive.net",
      "dct:title": "The Cancer Imaging Archive",
      "@context": {
        "dct": "http://purl.org/dc/terms/",
        "foaf": "http://xmlns.com/foaf/0.1/",
        "datmm": "http://schema.org/"
      }
    },
    "frapo:isSupportedBy": [],
    "schema:distribution": [
      {
        "@type": "schema:DataDownload",
        "schema:contentSize": "183GB",
        "schema:encodingFormat": "DICOM",
        "schema:inLanguage": "en",
        "schema:name": "Images\u00a0and Radiation Therapy Structures ",
        "schema:url": "https://wiki.cancerimagingarchive.net/display/Public/4D-Lung/download/attachments/21267414/doiJNLP-Y71kLpdQ.tcia?version=1&modificationDate=1534787014809&api=v2",
        "@context": {
          "schema": "http://schema.org/"
        }
      }
    ],
    "dct:isReferencedBy": [
      {
        "@type": "datmm:Documentation",
        "rdf:type": "Journal Article",
        "dct:title": "A longitudinal four-dimensional computed tomography and cone beam computed tomography dataset for image-guided radiation therapy research in lung cancer.",
        "dct:bibliographicCitation": "Hugo GD, et al. A longitudinal four-dimensional computed tomography and cone beam computed tomography dataset for image-guided radiation therapy research in lung cancer. Med Phys",
        "prism:doi": "10.1002/mp.12059",
        "fabio:hasPubMedId": "27991677",
        "foaf:homepage": "https://pubmed.ncbi.nlm.nih.gov/27991677",
        "dct:identifier": "27991677",
        "@context": {
          "dct": "http://purl.org/dc/terms/",
          "prism": "http://prismstandard.org/namespaces/basic/3.0/",
          "rdf": "http://www.w3.org/1999/02/22-rdf-syntax-ns#",
          "foaf": "http://xmlns.com/foaf/0.1/",
          "datmm": "http://schema.org/",
          "fabio": "http://purl.org/spar/fabio/"
        }
      },
      {
        "@type": "datmm:Documentation",
        "rdf:type": "Journal Article",
        "dct:title": "Evaluation of 4-dimensional computed tomography to 4-dimensional cone-beam computed tomography deformable image registration for lung cancer adaptive radiation therapy.",
        "dct:bibliographicCitation": "Balik S, et al. Evaluation of 4-dimensional computed tomography to 4-dimensional cone-beam computed tomography deformable image registration for lung cancer adaptive radiation therapy. Int J Radiat Oncol Biol Phys",
        "prism:doi": "10.1016/j.ijrobp.2012.12.023",
        "fabio:hasPubMedId": "23462422",
        "foaf:homepage": "https://pubmed.ncbi.nlm.nih.gov/23462422",
        "dct:identifier": "23462422",
        "@context": {
          "dct": "http://purl.org/dc/terms/",
          "prism": "http://prismstandard.org/namespaces/basic/3.0/",
          "rdf": "http://www.w3.org/1999/02/22-rdf-syntax-ns#",
          "foaf": "http://xmlns.com/foaf/0.1/",
          "datmm": "http://schema.org/",
          "fabio": "http://purl.org/spar/fabio/"
        }
      },
      {
        "@type": "datmm:Documentation",
        "rdf:type": "Journal Article",
        "dct:title": "Interfractional positional variability of fiducial markers and primary tumors in locally advanced non-small-cell lung cancer during audiovisual biofeedback radiotherapy.",
        "dct:bibliographicCitation": "Roman NO, et al. Interfractional positional variability of fiducial markers and primary tumors in locally advanced non-small-cell lung cancer during audiovisual biofeedback radiotherapy. Int J Radiat Oncol Biol Phys",
        "prism:doi": "10.1016/j.ijrobp.2011.10.051",
        "fabio:hasPubMedId": "22391105",
        "foaf:homepage": "https://pubmed.ncbi.nlm.nih.gov/22391105",
        "dct:identifier": "22391105",
        "@context": {
          "dct": "http://purl.org/dc/terms/",
          "prism": "http://prismstandard.org/namespaces/basic/3.0/",
          "rdf": "http://www.w3.org/1999/02/22-rdf-syntax-ns#",
          "foaf": "http://xmlns.com/foaf/0.1/",
          "datmm": "http://schema.org/",
          "fabio": "http://purl.org/spar/fabio/"
        }
      }
    ],
    "dct:subject": [
      {
        "@type": "skos:Concept",
        "dct:identifier": "D054893",
        "skos:inScheme": "MeSH",
        "rdfs:label": "Cone-Beam Computed Tomography",
        "@context": {
          "rdfs": "http://www.w3.org/2000/01/rdf-schema#",
          "skos": "http://www.w3.org/2004/02/skos/core#",
          "dct": "http://purl.org/dc/terms/"
        }
      },
      {
        "@type": "skos:Concept",
        "dct:identifier": "D056973",
        "skos:inScheme": "MeSH",
        "rdfs:label": "Four-Dimensional Computed Tomography",
        "@context": {
          "rdfs": "http://www.w3.org/2000/01/rdf-schema#",
          "skos": "http://www.w3.org/2004/02/skos/core#",
          "dct": "http://purl.org/dc/terms/"
        }
      },
      {
        "@type": "skos:Concept",
        "dct:identifier": "D061089",
        "skos:inScheme": "MeSH",
        "rdfs:label": "Radiotherapy, Image-Guided",
        "@context": {
          "rdfs": "http://www.w3.org/2000/01/rdf-schema#",
          "skos": "http://www.w3.org/2004/02/skos/core#",
          "dct": "http://purl.org/dc/terms/"
        }
      },
      {
        "@type": "skos:Concept",
        "dct:identifier": "D000465",
        "skos:inScheme": "MeSH",
        "rdfs:label": "Algorithms",
        "@context": {
          "rdfs": "http://www.w3.org/2000/01/rdf-schema#",
          "skos": "http://www.w3.org/2004/02/skos/core#",
          "dct": "http://purl.org/dc/terms/"
        }
      },
      {
        "@type": "skos:Concept",
        "dct:identifier": "D057918",
        "skos:inScheme": "MeSH",
        "rdfs:label": "Fiducial Markers",
        "@context": {
          "rdfs": "http://www.w3.org/2000/01/rdf-schema#",
          "skos": "http://www.w3.org/2004/02/skos/core#",
          "dct": "http://purl.org/dc/terms/"
        }
      },
      {
        "@type": "skos:Concept",
        "dct:identifier": "D009068",
        "skos:inScheme": "MeSH",
        "rdfs:label": "Movement",
        "@context": {
          "rdfs": "http://www.w3.org/2000/01/rdf-schema#",
          "skos": "http://www.w3.org/2004/02/skos/core#",
          "dct": "http://purl.org/dc/terms/"
        }
      }
    ],
    "@context": {
      "dct": "http://purl.org/dc/terms/",
      "foaf": "http://xmlns.com/foaf/0.1/",
      "datmm": "http://schema.org/"
    }
  },
  {
    "@type": "datmm:Dataset",
    "dct:description": "This data set was provided in association with a\u00a0 challenge competition",
    "dct:format": "Unknown",
    "dct:issued": "2020/07/20",
    "foaf:homepage": "https://www.ncbi.nlm.nih.gov/gap",
    "dct:title": "AAPM RT-MAC Grand Challenge 2019",
    "dct:language": "English",
    "bf:contribution": [],
    "dct:isPartOf": {
      "@type": "datmm:Repository",
      "dct:alternative": "TCIA",
      "foaf:homepage": "https://www.cancerimagingarchive.net",
      "dct:title": "The Cancer Imaging Archive",
      "@context": {
        "dct": "http://purl.org/dc/terms/",
        "foaf": "http://xmlns.com/foaf/0.1/",
        "datmm": "http://schema.org/"
      }
    },
    "frapo:isSupportedBy": [],
    "schema:distribution": [
      {
        "@type": "schema:DataDownload",
        "schema:contentSize": "3.5 GB",
        "schema:encodingFormat": "DICOM",
        "schema:inLanguage": "en",
        "schema:name": "Images and Radiation Therapy Structures ",
        "schema:url": "https://wiki.cancerimagingarchive.net/display/Public/AAPM+RT-MAC+Grand+Challenge+2019/download/attachments/50135916/AAPM%20RT%20MAC%20July%2020%202020%20NBIA-manifest.tcia?version=1&modificationDate=1595265571711&api=v2",
        "@context": {
          "schema": "http://schema.org/"
        }
      }
    ],
    "dct:isReferencedBy": [
      {
        "@type": "datmm:Documentation",
        "rdf:type": "Journal Article",
        "dct:title": "Head and neck cancer patient images for determining auto-segmentation accuracy in T2-weighted magnetic resonance imaging through expert manual segmentations.",
        "dct:bibliographicCitation": "Cardenas CE, et al. Head and neck cancer patient images for determining auto-segmentation accuracy in T2-weighted magnetic resonance imaging through expert manual segmentations. Med Phys",
        "prism:doi": "10.1002/mp.13942",
        "fabio:hasPubMedId": "32418343",
        "foaf:homepage": "https://pubmed.ncbi.nlm.nih.gov/32418343",
        "dct:identifier": "32418343",
        "@context": {
          "dct": "http://purl.org/dc/terms/",
          "prism": "http://prismstandard.org/namespaces/basic/3.0/",
          "rdf": "http://www.w3.org/1999/02/22-rdf-syntax-ns#",
          "foaf": "http://xmlns.com/foaf/0.1/",
          "datmm": "http://schema.org/",
          "fabio": "http://purl.org/spar/fabio/"
        }
      }
    ],
    "dct:subject": [
      {
        "@type": "skos:Concept",
        "dct:identifier": "D008279",
        "skos:inScheme": "MeSH",
        "rdfs:label": "Magnetic Resonance Imaging",
        "@context": {
          "rdfs": "http://www.w3.org/2000/01/rdf-schema#",
          "skos": "http://www.w3.org/2004/02/skos/core#",
          "dct": "http://purl.org/dc/terms/"
        }
      }
    ],
    "@context": {
      "dct": "http://purl.org/dc/terms/",
      "foaf": "http://xmlns.com/foaf/0.1/",
      "datmm": "http://schema.org/"
    }
  },
  {
    "@type": "datmm:Dataset",
    "dct:description": "The American College of Radiology Imaging Network (ACRIN) trial 6698 was a multi-center study to evaluate the effectiveness of quantitative diffusion weighted imaging (DWI) for assessing breast cancer response to neoadjuvant chemotherapy (NAC).\u00a0 \u00a0ACRIN 6698 was performed as a sub-study of the ongoing I-SPY 2 TRIAL (Investigation of Serial studies to Predict Your Therapeutic Response with Imaging And moLecular Analysis 2), an adaptive, multi-agent phase II trial designed to quickly identify new agents for breast cancer.\u00a0\u00a0",
    "dct:format": "Unknown",
    "dct:issued": "Current",
    "foaf:homepage": "https://www.ncbi.nlm.nih.gov/gap",
    "dct:title": "ACRIN 6698/I-SPY2 Breast DWI (ACRIN 6698)",
    "dct:language": "English",
    "bf:contribution": [],
    "dct:isPartOf": {
      "@type": "datmm:Repository",
      "dct:alternative": "TCIA",
      "foaf:homepage": "https://www.cancerimagingarchive.net",
      "dct:title": "The Cancer Imaging Archive",
      "@context": {
        "dct": "http://purl.org/dc/terms/",
        "foaf": "http://xmlns.com/foaf/0.1/",
        "datmm": "http://schema.org/"
      }
    },
    "frapo:isSupportedBy": [],
    "schema:distribution": [],
    "dct:isReferencedBy": [
      {
        "@type": "datmm:Documentation",
        "rdf:type": "Journal Article",
        "dct:title": "Test-retest repeatability and reproducibility of ADC measures by breast DWI: Results from the ACRIN 6698 trial.",
        "dct:bibliographicCitation": "Newitt DC, et al. Test-retest repeatability and reproducibility of ADC measures by breast DWI: Results from the ACRIN 6698 trial. J Magn Reson Imaging",
        "prism:doi": "10.1002/jmri.26539",
        "fabio:hasPubMedId": "30350329",
        "foaf:homepage": "https://pubmed.ncbi.nlm.nih.gov/30350329",
        "dct:identifier": "30350329",
        "@context": {
          "dct": "http://purl.org/dc/terms/",
          "prism": "http://prismstandard.org/namespaces/basic/3.0/",
          "rdf": "http://www.w3.org/1999/02/22-rdf-syntax-ns#",
          "foaf": "http://xmlns.com/foaf/0.1/",
          "datmm": "http://schema.org/",
          "fabio": "http://purl.org/spar/fabio/"
        }
      }
    ],
    "dct:subject": [
      {
        "@type": "skos:Concept",
        "dct:identifier": "D038524",
        "skos:inScheme": "MeSH",
        "rdfs:label": "Diffusion Magnetic Resonance Imaging",
        "@context": {
          "rdfs": "http://www.w3.org/2000/01/rdf-schema#",
          "skos": "http://www.w3.org/2004/02/skos/core#",
          "dct": "http://purl.org/dc/terms/"
        }
      }
    ],
    "@context": {
      "dct": "http://purl.org/dc/terms/",
      "foaf": "http://xmlns.com/foaf/0.1/",
      "datmm": "http://schema.org/"
    }
  },
  {
    "@type": "datmm:Dataset",
    "dct:description": "This dataset relates to NCI Clinical trial, \"Magnetic Resonance Imaging in Women Recently Diagnosed With Unilateral Breast Cancer (",
    "dct:format": "Unknown",
    "dct:issued": "2021/03/05",
    "foaf:homepage": "https://www.ncbi.nlm.nih.gov/gap",
    "dct:title": "ACRIN-Contralateral-Breast-MR (ACRIN 6667)",
    "dct:language": "English",
    "bf:contribution": [],
    "dct:isPartOf": {
      "@type": "datmm:Repository",
      "dct:alternative": "TCIA",
      "foaf:homepage": "https://www.cancerimagingarchive.net",
      "dct:title": "The Cancer Imaging Archive",
      "@context": {
        "dct": "http://purl.org/dc/terms/",
        "foaf": "http://xmlns.com/foaf/0.1/",
        "datmm": "http://schema.org/"
      }
    },
    "frapo:isSupportedBy": [],
    "schema:distribution": [],
    "dct:isReferencedBy": [
      {
        "@type": "datmm:Documentation",
        "rdf:type": "Clinical Trial",
        "dct:title": "MRI evaluation of the contralateral breast in women with recently diagnosed breast cancer.",
        "dct:bibliographicCitation": "Lehman CD, et al. MRI evaluation of the contralateral breast in women with recently diagnosed breast cancer. N Engl J Med",
        "prism:doi": "10.1056/NEJMoa065447",
        "fabio:hasPubMedId": "17392300",
        "foaf:homepage": "https://pubmed.ncbi.nlm.nih.gov/17392300",
        "dct:identifier": "17392300",
        "@context": {
          "dct": "http://purl.org/dc/terms/",
          "prism": "http://prismstandard.org/namespaces/basic/3.0/",
          "rdf": "http://www.w3.org/1999/02/22-rdf-syntax-ns#",
          "foaf": "http://xmlns.com/foaf/0.1/",
          "datmm": "http://schema.org/",
          "fabio": "http://purl.org/spar/fabio/"
        }
      }
    ],
    "dct:subject": [
      {
        "@type": "skos:Concept",
        "dct:identifier": "D008279",
        "skos:inScheme": "MeSH",
        "rdfs:label": "Magnetic Resonance Imaging",
        "@context": {
          "rdfs": "http://www.w3.org/2000/01/rdf-schema#",
          "skos": "http://www.w3.org/2004/02/skos/core#",
          "dct": "http://purl.org/dc/terms/"
        }
      }
    ],
    "@context": {
      "dct": "http://purl.org/dc/terms/",
      "foaf": "http://xmlns.com/foaf/0.1/",
      "datmm": "http://schema.org/"
    }
  },
  {
    "@type": "datmm:Dataset",
    "dct:description": "RTOG 0625/ACRIN 6677 is a multicenter, randomized, phase II trial of bevacizumab with irinotecan or temozolomide in recurrent glioblastoma (GBM). This study investigated whether early posttreatment progression on FLAIR or postcontrast MRI assessed by central reading predicts overall survival (OS).",
    "dct:format": "Unknown",
    "dct:issued": "2019/02/07",
    "foaf:homepage": "https://www.ncbi.nlm.nih.gov/gap",
    "dct:title": "ACRIN-DSC-MR-Brain (ACRIN 6677/RTOG 0625)",
    "dct:language": "English",
    "bf:contribution": [],
    "dct:isPartOf": {
      "@type": "datmm:Repository",
      "dct:alternative": "TCIA",
      "foaf:homepage": "https://www.cancerimagingarchive.net",
      "dct:title": "The Cancer Imaging Archive",
      "@context": {
        "dct": "http://purl.org/dc/terms/",
        "foaf": "http://xmlns.com/foaf/0.1/",
        "datmm": "http://schema.org/"
      }
    },
    "frapo:isSupportedBy": [],
    "schema:distribution": [],
    "dct:isReferencedBy": [
      {
        "@type": "datmm:Documentation",
        "rdf:type": "Journal Article",
        "dct:title": "Early post-bevacizumab progression on contrast-enhanced MRI as a prognostic marker for overall survival in recurrent glioblastoma: results from the ACRIN 6677/RTOG 0625 Central Reader Study.",
        "dct:bibliographicCitation": "Boxerman JL, et al. Early post-bevacizumab progression on contrast-enhanced MRI as a prognostic marker for overall survival in recurrent glioblastoma: results from the ACRIN 6677/RTOG 0625 Central Reader Study. Neuro Oncol",
        "prism:doi": "10.1093/neuonc/not049",
        "fabio:hasPubMedId": "23788270",
        "foaf:homepage": "https://pubmed.ncbi.nlm.nih.gov/23788270",
        "dct:identifier": "23788270",
        "@context": {
          "dct": "http://purl.org/dc/terms/",
          "prism": "http://prismstandard.org/namespaces/basic/3.0/",
          "rdf": "http://www.w3.org/1999/02/22-rdf-syntax-ns#",
          "foaf": "http://xmlns.com/foaf/0.1/",
          "datmm": "http://schema.org/",
          "fabio": "http://purl.org/spar/fabio/"
        }
      }
    ],
    "dct:subject": [
      {
        "@type": "skos:Concept",
        "dct:identifier": "D003287",
        "skos:inScheme": "MeSH",
        "rdfs:label": "Contrast Media",
        "@context": {
          "rdfs": "http://www.w3.org/2000/01/rdf-schema#",
          "skos": "http://www.w3.org/2004/02/skos/core#",
          "dct": "http://purl.org/dc/terms/"
        }
      }
    ],
    "@context": {
      "dct": "http://purl.org/dc/terms/",
      "foaf": "http://xmlns.com/foaf/0.1/",
      "datmm": "http://schema.org/"
    }
  },
  {
    "@type": "datmm:Dataset",
    "dct:description": "The objective of the ACRIN 6688 multi-center clinical trial was to correlate changes measured by ",
    "dct:format": "Unknown",
    "dct:issued": "2020/01/24",
    "foaf:homepage": "https://www.ncbi.nlm.nih.gov/gap",
    "dct:title": "ACRIN-FLT-Breast (ACRIN 6688)",
    "dct:language": "English",
    "bf:contribution": [],
    "dct:isPartOf": {
      "@type": "datmm:Repository",
      "dct:alternative": "TCIA",
      "foaf:homepage": "https://www.cancerimagingarchive.net",
      "dct:title": "The Cancer Imaging Archive",
      "@context": {
        "dct": "http://purl.org/dc/terms/",
        "foaf": "http://xmlns.com/foaf/0.1/",
        "datmm": "http://schema.org/"
      }
    },
    "frapo:isSupportedBy": [],
    "schema:distribution": [
      {
        "@type": "schema:DataDownload",
        "schema:contentSize": "74.2 GB",
        "schema:encodingFormat": "DICOM",
        "schema:inLanguage": "en",
        "schema:name": "Images ",
        "schema:url": "https://wiki.cancerimagingarchive.net/pages/viewpage.action?pageId=30671268/download/attachments/30671268/ACRIN-FLT-Breast_2020-01-24.tcia?version=1&modificationDate=1579882645928&api=v2",
        "@context": {
          "schema": "http://schema.org/"
        }
      }
    ],
    "dct:isReferencedBy": [
      {
        "@type": "datmm:Documentation",
        "rdf:type": "Journal Article",
        "dct:title": "A Phase II Study of 3'-Deoxy-3'-18F-Fluorothymidine PET in the Assessment of Early Response of Breast Cancer to Neoadjuvant Chemotherapy: Results from ACRIN 6688.",
        "dct:bibliographicCitation": "Kostakoglu L, et al. A Phase II Study of 3'-Deoxy-3'-18F-Fluorothymidine PET in the Assessment of Early Response of Breast Cancer to Neoadjuvant Chemotherapy: Results from ACRIN 6688. J Nucl Med",
        "prism:doi": "10.2967/jnumed.115.160663",
        "fabio:hasPubMedId": "26359256",
        "foaf:homepage": "https://pubmed.ncbi.nlm.nih.gov/26359256",
        "dct:identifier": "26359256",
        "@context": {
          "dct": "http://purl.org/dc/terms/",
          "prism": "http://prismstandard.org/namespaces/basic/3.0/",
          "rdf": "http://www.w3.org/1999/02/22-rdf-syntax-ns#",
          "foaf": "http://xmlns.com/foaf/0.1/",
          "datmm": "http://schema.org/",
          "fabio": "http://purl.org/spar/fabio/"
        }
      }
    ],
    "dct:subject": [
      {
        "@type": "skos:Concept",
        "dct:identifier": "D015224",
        "skos:inScheme": "MeSH",
        "rdfs:label": "Dideoxynucleosides",
        "@context": {
          "rdfs": "http://www.w3.org/2000/01/rdf-schema#",
          "skos": "http://www.w3.org/2004/02/skos/core#",
          "dct": "http://purl.org/dc/terms/"
        }
      },
      {
        "@type": "skos:Concept",
        "dct:identifier": "D019275",
        "skos:inScheme": "MeSH",
        "rdfs:label": "Radiopharmaceuticals",
        "@context": {
          "rdfs": "http://www.w3.org/2000/01/rdf-schema#",
          "skos": "http://www.w3.org/2004/02/skos/core#",
          "dct": "http://purl.org/dc/terms/"
        }
      }
    ],
    "@context": {
      "dct": "http://purl.org/dc/terms/",
      "foaf": "http://xmlns.com/foaf/0.1/",
      "datmm": "http://schema.org/"
    }
  },
  {
    "@type": "datmm:Dataset",
    "dct:description": "The objective of the ACRIN 6684 multi-center clinical trial was to determine the association of baseline FMISO PET uptake (maximal tumor to blood ratio, hypoxic volume) and MRI parameters (K",
    "dct:format": "Unknown",
    "dct:issued": "2019/07/02",
    "foaf:homepage": "https://www.ncbi.nlm.nih.gov/gap",
    "dct:title": "ACRIN-FMISO-Brain (ACRIN 6684)",
    "dct:language": "English",
    "bf:contribution": [],
    "dct:isPartOf": {
      "@type": "datmm:Repository",
      "dct:alternative": "TCIA",
      "foaf:homepage": "https://www.cancerimagingarchive.net",
      "dct:title": "The Cancer Imaging Archive",
      "@context": {
        "dct": "http://purl.org/dc/terms/",
        "foaf": "http://xmlns.com/foaf/0.1/",
        "datmm": "http://schema.org/"
      }
    },
    "frapo:isSupportedBy": [],
    "schema:distribution": [
      {
        "@type": "schema:DataDownload",
        "schema:contentSize": "96GB",
        "schema:encodingFormat": "DICOM",
        "schema:inLanguage": "en",
        "schema:name": "Images ",
        "schema:url": "https://wiki.cancerimagingarchive.net/pages/viewpage.action?pageId=33948305/download/attachments/33948305/ACRIN-FMISO-Brain%20July%202%202019%20NBIA%20manifest.tcia?version=1&modificationDate=1562170452478&api=v2",
        "@context": {
          "schema": "http://schema.org/"
        }
      }
    ],
    "dct:isReferencedBy": [
      {
        "@type": "datmm:Documentation",
        "rdf:type": "Journal Article",
        "dct:title": "ACRIN 6684: Assessment of Tumor Hypoxia in Newly Diagnosed Glioblastoma Using 18F-FMISO PET and MRI.",
        "dct:bibliographicCitation": "Gerstner ER, et al. ACRIN 6684: Assessment of Tumor Hypoxia in Newly Diagnosed Glioblastoma Using 18F-FMISO PET and MRI. Clin Cancer Res",
        "prism:doi": "10.1158/1078-0432.CCR-15-2529",
        "fabio:hasPubMedId": "27185374",
        "foaf:homepage": "https://pubmed.ncbi.nlm.nih.gov/27185374",
        "dct:identifier": "27185374",
        "@context": {
          "dct": "http://purl.org/dc/terms/",
          "prism": "http://prismstandard.org/namespaces/basic/3.0/",
          "rdf": "http://www.w3.org/1999/02/22-rdf-syntax-ns#",
          "foaf": "http://xmlns.com/foaf/0.1/",
          "datmm": "http://schema.org/",
          "fabio": "http://purl.org/spar/fabio/"
        }
      },
      {
        "@type": "datmm:Documentation",
        "rdf:type": "Journal Article",
        "dct:title": "ACRIN 6684: Multicenter, phase II assessment of tumor hypoxia in newly diagnosed glioblastoma using magnetic resonance spectroscopy.",
        "dct:bibliographicCitation": "Ratai EM, et al. ACRIN 6684: Multicenter, phase II assessment of tumor hypoxia in newly diagnosed glioblastoma using magnetic resonance spectroscopy. PLoS One",
        "prism:doi": "10.1371/journal.pone.0198548",
        "fabio:hasPubMedId": "29902200",
        "foaf:homepage": "https://pubmed.ncbi.nlm.nih.gov/29902200",
        "dct:identifier": "29902200",
        "@context": {
          "dct": "http://purl.org/dc/terms/",
          "prism": "http://prismstandard.org/namespaces/basic/3.0/",
          "rdf": "http://www.w3.org/1999/02/22-rdf-syntax-ns#",
          "foaf": "http://xmlns.com/foaf/0.1/",
          "datmm": "http://schema.org/",
          "fabio": "http://purl.org/spar/fabio/"
        }
      }
    ],
    "dct:subject": [
      {
        "@type": "skos:Concept",
        "dct:identifier": "D008279",
        "skos:inScheme": "MeSH",
        "rdfs:label": "Magnetic Resonance Imaging",
        "@context": {
          "rdfs": "http://www.w3.org/2000/01/rdf-schema#",
          "skos": "http://www.w3.org/2004/02/skos/core#",
          "dct": "http://purl.org/dc/terms/"
        }
      },
      {
        "@type": "skos:Concept",
        "dct:identifier": "D049268",
        "skos:inScheme": "MeSH",
        "rdfs:label": "Positron-Emission Tomography",
        "@context": {
          "rdfs": "http://www.w3.org/2000/01/rdf-schema#",
          "skos": "http://www.w3.org/2004/02/skos/core#",
          "dct": "http://purl.org/dc/terms/"
        }
      },
      {
        "@type": "skos:Concept",
        "dct:identifier": "D066244",
        "skos:inScheme": "MeSH",
        "rdfs:label": "Proton Magnetic Resonance Spectroscopy",
        "@context": {
          "rdfs": "http://www.w3.org/2000/01/rdf-schema#",
          "skos": "http://www.w3.org/2004/02/skos/core#",
          "dct": "http://purl.org/dc/terms/"
        }
      },
      {
        "@type": "skos:Concept",
        "dct:identifier": "D000072258",
        "skos:inScheme": "MeSH",
        "rdfs:label": "Tumor Hypoxia",
        "@context": {
          "rdfs": "http://www.w3.org/2000/01/rdf-schema#",
          "skos": "http://www.w3.org/2004/02/skos/core#",
          "dct": "http://purl.org/dc/terms/"
        }
      }
    ],
    "@context": {
      "dct": "http://purl.org/dc/terms/",
      "foaf": "http://xmlns.com/foaf/0.1/",
      "datmm": "http://schema.org/"
    }
  },
  {
    "@type": "datmm:Dataset",
    "dct:description": "ACRIN-HNSCC-FDG-PET/CT (ACRIN 6685) is a Multicenter Trial of FDG-PET/CT Staging of Head and Neck Cancer\u00a0",
    "dct:format": "Unknown",
    "dct:issued": "2020/03/13",
    "foaf:homepage": "https://www.ncbi.nlm.nih.gov/gap",
    "dct:title": "ACRIN-HNSCC-FDG-PET/CT (ACRIN 6685)",
    "dct:language": "English",
    "bf:contribution": [],
    "dct:isPartOf": {
      "@type": "datmm:Repository",
      "dct:alternative": "TCIA",
      "foaf:homepage": "https://www.cancerimagingarchive.net",
      "dct:title": "The Cancer Imaging Archive",
      "@context": {
        "dct": "http://purl.org/dc/terms/",
        "foaf": "http://xmlns.com/foaf/0.1/",
        "datmm": "http://schema.org/"
      }
    },
    "frapo:isSupportedBy": [],
    "schema:distribution": [],
    "dct:isReferencedBy": [
      {
        "@type": "datmm:Documentation",
        "rdf:type": "Clinical Trial",
        "dct:title": "Multicenter Trial of [<sup>18</sup>F]fluorodeoxyglucose Positron Emission Tomography/Computed Tomography Staging of Head and Neck Cancer and Negative Predictive Value and Surgical Impact in the N0 Neck: Results From ACRIN 6685.",
        "dct:bibliographicCitation": "Lowe VJ, et al. Multicenter Trial of [<sup>18</sup>F]fluorodeoxyglucose Positron Emission Tomography/Computed Tomography Staging of Head and Neck Cancer and Negative Predictive Value and Surgical Impact in the N0 Neck: Results From ACRIN 6685. J Clin Oncol",
        "prism:doi": "10.1200/JCO.18.01182",
        "fabio:hasPubMedId": "30768363",
        "foaf:homepage": "https://pubmed.ncbi.nlm.nih.gov/30768363",
        "dct:identifier": "30768363",
        "@context": {
          "dct": "http://purl.org/dc/terms/",
          "prism": "http://prismstandard.org/namespaces/basic/3.0/",
          "rdf": "http://www.w3.org/1999/02/22-rdf-syntax-ns#",
          "foaf": "http://xmlns.com/foaf/0.1/",
          "datmm": "http://schema.org/",
          "fabio": "http://purl.org/spar/fabio/"
        }
      }
    ],
    "dct:subject": [
      {
        "@type": "skos:Concept",
        "dct:identifier": "D000072078",
        "skos:inScheme": "MeSH",
        "rdfs:label": "Positron Emission Tomography Computed Tomography",
        "@context": {
          "rdfs": "http://www.w3.org/2000/01/rdf-schema#",
          "skos": "http://www.w3.org/2004/02/skos/core#",
          "dct": "http://purl.org/dc/terms/"
        }
      }
    ],
    "@context": {
      "dct": "http://purl.org/dc/terms/",
      "foaf": "http://xmlns.com/foaf/0.1/",
      "datmm": "http://schema.org/"
    }
  },
  {
    "@type": "datmm:Dataset",
    "dct:description": "Positron Emission Tomography Pre- and Post-treatment Assessment for Locally Advanced Non-small Cell Lung Carcinoma\u00a0",
    "dct:format": "Unknown",
    "dct:issued": "2020/02/11",
    "foaf:homepage": "https://www.ncbi.nlm.nih.gov/gap",
    "dct:title": "ACRIN-NSCLC-FDG-PET (ACRIN 6668)",
    "dct:language": "English",
    "bf:contribution": [],
    "dct:isPartOf": {
      "@type": "datmm:Repository",
      "dct:alternative": "TCIA",
      "foaf:homepage": "https://www.cancerimagingarchive.net",
      "dct:title": "The Cancer Imaging Archive",
      "@context": {
        "dct": "http://purl.org/dc/terms/",
        "foaf": "http://xmlns.com/foaf/0.1/",
        "datmm": "http://schema.org/"
      }
    },
    "frapo:isSupportedBy": [],
    "schema:distribution": [
      {
        "@type": "schema:DataDownload",
        "schema:contentSize": "145.5 GB",
        "schema:encodingFormat": "DICOM",
        "schema:inLanguage": "en",
        "schema:name": "Images ",
        "schema:url": "https://wiki.cancerimagingarchive.net/pages/viewpage.action?pageId=39879162/download/attachments/39879162/ACRIN-6668-NSCLC-FDG-PET%20FEB%2004%202020%20manifest.tcia?version=1&modificationDate=1580838316208&api=v2",
        "@context": {
          "schema": "http://schema.org/"
        }
      }
    ],
    "dct:isReferencedBy": [
      {
        "@type": "datmm:Documentation",
        "rdf:type": "Clinical Trial",
        "dct:title": "Prediction of survival by [18F]fluorodeoxyglucose positron emission tomography in patients with locally advanced non-small-cell lung cancer undergoing definitive chemoradiation therapy: results of the ACRIN 6668/RTOG 0235 trial.",
        "dct:bibliographicCitation": "Machtay M, et al. Prediction of survival by [18F]fluorodeoxyglucose positron emission tomography in patients with locally advanced non-small-cell lung cancer undergoing definitive chemoradiation therapy: results of the ACRIN 6668/RTOG 0235 trial. J Clin Oncol",
        "prism:doi": "10.1200/JCO.2012.47.5947",
        "fabio:hasPubMedId": "24043740",
        "foaf:homepage": "https://pubmed.ncbi.nlm.nih.gov/24043740",
        "dct:identifier": "24043740",
        "@context": {
          "dct": "http://purl.org/dc/terms/",
          "prism": "http://prismstandard.org/namespaces/basic/3.0/",
          "rdf": "http://www.w3.org/1999/02/22-rdf-syntax-ns#",
          "foaf": "http://xmlns.com/foaf/0.1/",
          "datmm": "http://schema.org/",
          "fabio": "http://purl.org/spar/fabio/"
        }
      }
    ],
    "dct:subject": [
      {
        "@type": "skos:Concept",
        "dct:identifier": "D019788",
        "skos:inScheme": "MeSH",
        "rdfs:label": "Fluorodeoxyglucose F18",
        "@context": {
          "rdfs": "http://www.w3.org/2000/01/rdf-schema#",
          "skos": "http://www.w3.org/2004/02/skos/core#",
          "dct": "http://purl.org/dc/terms/"
        }
      },
      {
        "@type": "skos:Concept",
        "dct:identifier": "D049268",
        "skos:inScheme": "MeSH",
        "rdfs:label": "Positron-Emission Tomography",
        "@context": {
          "rdfs": "http://www.w3.org/2000/01/rdf-schema#",
          "skos": "http://www.w3.org/2004/02/skos/core#",
          "dct": "http://purl.org/dc/terms/"
        }
      },
      {
        "@type": "skos:Concept",
        "dct:identifier": "D019275",
        "skos:inScheme": "MeSH",
        "rdfs:label": "Radiopharmaceuticals",
        "@context": {
          "rdfs": "http://www.w3.org/2000/01/rdf-schema#",
          "skos": "http://www.w3.org/2004/02/skos/core#",
          "dct": "http://purl.org/dc/terms/"
        }
      }
    ],
    "@context": {
      "dct": "http://purl.org/dc/terms/",
      "foaf": "http://xmlns.com/foaf/0.1/",
      "datmm": "http://schema.org/"
    }
  },
  {
    "@type": "datmm:Dataset",
    "dct:description": "Open access or shared research data must comply with (HIPAA) patient privacy regulations. These regulations require the de-identification of datasets before they can be placed in the public domain.\u00a0 The process of image de-identification is time consuming, requires significant human resources, and is prone to human error. \u00a0Automated image de-identification algorithms have been developed but the research community requires some method of evaluation before such tools can be widely accepted.\u00a0 This evaluation requires a robust dataset that can be used as part of an evaluation process for de-identification algorithms. \u00a0",
    "dct:format": "Unknown",
    "dct:issued": "2021/04/07",
    "foaf:homepage": "https://www.ncbi.nlm.nih.gov/gap",
    "dct:title": "A DICOM dataset for evaluation of medical image de-identification (Pseudo-PHI-DICOM-Data)",
    "dct:language": "English",
    "bf:contribution": [],
    "dct:isPartOf": {
      "@type": "datmm:Repository",
      "dct:alternative": "TCIA",
      "foaf:homepage": "https://www.cancerimagingarchive.net",
      "dct:title": "The Cancer Imaging Archive",
      "@context": {
        "dct": "http://purl.org/dc/terms/",
        "foaf": "http://xmlns.com/foaf/0.1/",
        "datmm": "http://schema.org/"
      }
    },
    "frapo:isSupportedBy": [],
    "schema:distribution": [],
    "dct:isReferencedBy": [],
    "dct:subject": [],
    "@context": {
      "dct": "http://purl.org/dc/terms/",
      "foaf": "http://xmlns.com/foaf/0.1/",
      "datmm": "http://schema.org/"
    }
  },
  {
    "@type": "datmm:Dataset",
    "dct:description": "This dataset consists of CT and PET-CT DICOM images of lung cancer subjects with XML Annotation files that indicate tumor location with bounding boxes.\u00a0The images were retrospectively acquired from patients with suspicion of lung cancer, and who\u00a0underwent standard-of-care lung biopsy and PET/CT. Subjects were grouped according to a tissue histopathological diagnosis. Patients with Names/IDs containing the letter 'A' were diagnosed with Adenocarcinoma, 'B' with Small Cell Carcinoma, 'E' with Large Cell Carcinoma, and 'G' with Squamous Cell Carcinoma.",
    "dct:format": "Unknown",
    "dct:issued": "2020/12/22",
    "foaf:homepage": "https://www.ncbi.nlm.nih.gov/gap",
    "dct:title": "A Large-Scale CT and PET/CT Dataset for Lung Cancer Diagnosis (Lung-PET-CT-Dx)",
    "dct:language": "English",
    "bf:contribution": [],
    "dct:isPartOf": {
      "@type": "datmm:Repository",
      "dct:alternative": "TCIA",
      "foaf:homepage": "https://www.cancerimagingarchive.net",
      "dct:title": "The Cancer Imaging Archive",
      "@context": {
        "dct": "http://purl.org/dc/terms/",
        "foaf": "http://xmlns.com/foaf/0.1/",
        "datmm": "http://schema.org/"
      }
    },
    "frapo:isSupportedBy": [],
    "schema:distribution": [
      {
        "@type": "schema:DataDownload",
        "schema:contentSize": "127.2 GB",
        "schema:encodingFormat": "DICOM",
        "schema:inLanguage": "en",
        "schema:name": "Images ",
        "schema:url": "https://wiki.cancerimagingarchive.net/pages/viewpage.action?pageId=70224216/download/attachments/70224216/Lung-PET-CT-Dx-NBIA-Manifest-122220.tcia?version=1&modificationDate=1608669250614&api=v2",
        "@context": {
          "schema": "http://schema.org/"
        }
      }
    ],
    "dct:isReferencedBy": [],
    "dct:subject": [],
    "@context": {
      "dct": "http://purl.org/dc/terms/",
      "foaf": "http://xmlns.com/foaf/0.1/",
      "datmm": "http://schema.org/"
    }
  },
  {
    "@type": "datmm:Dataset",
    "dct:description": "\n This collection includes 46 lung cases treated with\u00a0",
    "dct:format": "Unknown",
    "dct:issued": "2019",
    "foaf:homepage": "https://www.ncbi.nlm.nih.gov/gap",
    "dct:title": "Anti-PD-1 Immunotherapy Lung (Anti-PD-1_Lung)",
    "dct:language": "English",
    "bf:contribution": [],
    "dct:isPartOf": {
      "@type": "datmm:Repository",
      "dct:alternative": "TCIA",
      "foaf:homepage": "https://www.cancerimagingarchive.net",
      "dct:title": "The Cancer Imaging Archive",
      "@context": {
        "dct": "http://purl.org/dc/terms/",
        "foaf": "http://xmlns.com/foaf/0.1/",
        "datmm": "http://schema.org/"
      }
    },
    "frapo:isSupportedBy": [],
    "schema:distribution": [
      {
        "@type": "schema:DataDownload",
        "schema:contentSize": "62.1 GB",
        "schema:encodingFormat": "DICOM",
        "schema:inLanguage": "en",
        "schema:name": "Images ",
        "schema:url": "https://wiki.cancerimagingarchive.net/pages/viewpage.action?pageId=41517500/download/attachments/41517500/Anti-PD-1%20LungNBIA-manifest-1555593712098.tcia?version=1&modificationDate=1555594875306&api=v2",
        "@context": {
          "schema": "http://schema.org/"
        }
      }
    ],
    "dct:isReferencedBy": [],
    "dct:subject": [],
    "@context": {
      "dct": "http://purl.org/dc/terms/",
      "foaf": "http://xmlns.com/foaf/0.1/",
      "datmm": "http://schema.org/"
    }
  },
  {
    "@type": "datmm:Dataset",
    "dct:description": "\n This collection includes 47 melanoma cases treated with anti-PD1 immunotherapy in 2016, each with pre-treatment and 1 or more imaging follow-up timepoints.",
    "dct:format": "Unknown",
    "dct:issued": "07-30-2018",
    "foaf:homepage": "https://www.ncbi.nlm.nih.gov/gap",
    "dct:title": "Anti-PD-1 Immunotherapy Melanoma (Anti-PD-1_MELANOMA)",
    "dct:language": "English",
    "bf:contribution": [],
    "dct:isPartOf": {
      "@type": "datmm:Repository",
      "dct:alternative": "TCIA",
      "foaf:homepage": "https://www.cancerimagingarchive.net",
      "dct:title": "The Cancer Imaging Archive",
      "@context": {
        "dct": "http://purl.org/dc/terms/",
        "foaf": "http://xmlns.com/foaf/0.1/",
        "datmm": "http://schema.org/"
      }
    },
    "frapo:isSupportedBy": [],
    "schema:distribution": [
      {
        "@type": "schema:DataDownload",
        "schema:contentSize": "98.4 GB",
        "schema:encodingFormat": "DICOM",
        "schema:inLanguage": "en",
        "schema:name": "Images ",
        "schema:url": "https://wiki.cancerimagingarchive.net/pages/viewpage.action?pageId=37225348/download/attachments/37225348/Anti-PD-1_MELANOMA-7-30-2018.tcia?version=1&modificationDate=1540860899780&api=v2",
        "@context": {
          "schema": "http://schema.org/"
        }
      }
    ],
    "dct:isReferencedBy": [],
    "dct:subject": [],
    "@context": {
      "dct": "http://purl.org/dc/terms/",
      "foaf": "http://xmlns.com/foaf/0.1/",
      "datmm": "http://schema.org/"
    }
  },
  {
    "@type": "datmm:Dataset",
    "dct:description": "The Munich AML Morphology Dataset contains 18,365 expert-labeled single-cell images taken from peripheral blood smears of 100 patients diagnosed with Acute Myeloid Leukemia at Munich University Hospital between 2014 and 2017, as well as 100 patients without signs of hematological malignancy. Image acquisition was done using a M8 digital microscope / scanner (Precipoint GmbH, Freising, Germany) at 100-fold optical magnification and oil immersion. Pathological and non-pathological leukocytes were classified into a standard morphological classification scheme derived from clinical practice by trained experts. To quantify inter- and intra-rater variability of examiners, a subset of images was re-annotated up to two times. The dataset has been used by the authors to train a convolutional neural network for single-cell morphology classification.",
    "dct:format": "Unknown",
    "dct:issued": "2019/10/24",
    "foaf:homepage": "https://www.ncbi.nlm.nih.gov/gap",
    "dct:title": "A Single-cell Morphological Dataset of Leukocytes from AML Patients and Non-malignant Controls (AML-Cytomorphology_LMU)",
    "dct:language": "English",
    "bf:contribution": [],
    "dct:isPartOf": {
      "@type": "datmm:Repository",
      "dct:alternative": "TCIA",
      "foaf:homepage": "https://www.cancerimagingarchive.net",
      "dct:title": "The Cancer Imaging Archive",
      "@context": {
        "dct": "http://purl.org/dc/terms/",
        "foaf": "http://xmlns.com/foaf/0.1/",
        "datmm": "http://schema.org/"
      }
    },
    "frapo:isSupportedBy": [],
    "schema:distribution": [],
    "dct:isReferencedBy": [
      {
        "@type": "datmm:Documentation",
        "rdf:type": "Journal Article",
        "dct:title": "Heterogeneous somatostatin-expressing neuron population in mouse ventral tegmental area.",
        "dct:bibliographicCitation": "Nagaeva E, et al. Heterogeneous somatostatin-expressing neuron population in mouse ventral tegmental area. Elife",
        "prism:doi": "10.7554/eLife.59328",
        "fabio:hasPubMedId": "32749220",
        "foaf:homepage": "https://pubmed.ncbi.nlm.nih.gov/32749220",
        "dct:identifier": "32749220",
        "@context": {
          "dct": "http://purl.org/dc/terms/",
          "prism": "http://prismstandard.org/namespaces/basic/3.0/",
          "rdf": "http://www.w3.org/1999/02/22-rdf-syntax-ns#",
          "foaf": "http://xmlns.com/foaf/0.1/",
          "datmm": "http://schema.org/",
          "fabio": "http://purl.org/spar/fabio/"
        }
      },
      {
        "@type": "datmm:Documentation",
        "rdf:type": "Journal Article",
        "dct:title": "Large-scale tight-binding simulations of quantum transport in ballistic graphene.",
        "dct:bibliographicCitation": "Calogero G, et al. Large-scale tight-binding simulations of quantum transport in ballistic graphene. J Phys Condens Matter",
        "prism:doi": "10.1088/1361-648X/aad6f1",
        "fabio:hasPubMedId": "30061475",
        "foaf:homepage": "https://pubmed.ncbi.nlm.nih.gov/30061475",
        "dct:identifier": "30061475",
        "@context": {
          "dct": "http://purl.org/dc/terms/",
          "prism": "http://prismstandard.org/namespaces/basic/3.0/",
          "rdf": "http://www.w3.org/1999/02/22-rdf-syntax-ns#",
          "foaf": "http://xmlns.com/foaf/0.1/",
          "datmm": "http://schema.org/",
          "fabio": "http://purl.org/spar/fabio/"
        }
      },
      {
        "@type": "datmm:Documentation",
        "rdf:type": "Journal Article",
        "dct:title": "Serum S100 calcium binding protein A4 improves the diagnostic accuracy of transient elastography for assessing liver fibrosis in hepatitis B.",
        "dct:bibliographicCitation": "Yan LB, et al. Serum S100 calcium binding protein A4 improves the diagnostic accuracy of transient elastography for assessing liver fibrosis in hepatitis B. Clin Res Hepatol Gastroenterol",
        "prism:doi": "10.1016/j.clinre.2017.05.013",
        "fabio:hasPubMedId": "28688902",
        "foaf:homepage": "https://pubmed.ncbi.nlm.nih.gov/28688902",
        "dct:identifier": "28688902",
        "@context": {
          "dct": "http://purl.org/dc/terms/",
          "prism": "http://prismstandard.org/namespaces/basic/3.0/",
          "rdf": "http://www.w3.org/1999/02/22-rdf-syntax-ns#",
          "foaf": "http://xmlns.com/foaf/0.1/",
          "datmm": "http://schema.org/",
          "fabio": "http://purl.org/spar/fabio/"
        }
      },
      {
        "@type": "datmm:Documentation",
        "rdf:type": "Journal Article",
        "dct:title": "Image-based adaptive optics for in vivo imaging in the hippocampus.",
        "dct:bibliographicCitation": "Champelovier D, et al. Image-based adaptive optics for in vivo imaging in the hippocampus. Sci Rep",
        "prism:doi": "10.1038/srep42924",
        "fabio:hasPubMedId": "28220868",
        "foaf:homepage": "https://pubmed.ncbi.nlm.nih.gov/28220868",
        "dct:identifier": "28220868",
        "@context": {
          "dct": "http://purl.org/dc/terms/",
          "prism": "http://prismstandard.org/namespaces/basic/3.0/",
          "rdf": "http://www.w3.org/1999/02/22-rdf-syntax-ns#",
          "foaf": "http://xmlns.com/foaf/0.1/",
          "datmm": "http://schema.org/",
          "fabio": "http://purl.org/spar/fabio/"
        }
      },
      {
        "@type": "datmm:Documentation",
        "rdf:type": "Published Erratum",
        "dct:title": "Molecular mechanisms of cell death: central implication of ATP synthase in mitochondrial permeability transition.",
        "dct:bibliographicCitation": "Bonora M, et al. Molecular mechanisms of cell death: central implication of ATP synthase in mitochondrial permeability transition. Oncogene",
        "prism:doi": "10.1038/onc.2014.462",
        "fabio:hasPubMedId": "25790189",
        "foaf:homepage": "https://pubmed.ncbi.nlm.nih.gov/25790189",
        "dct:identifier": "25790189",
        "@context": {
          "dct": "http://purl.org/dc/terms/",
          "prism": "http://prismstandard.org/namespaces/basic/3.0/",
          "rdf": "http://www.w3.org/1999/02/22-rdf-syntax-ns#",
          "foaf": "http://xmlns.com/foaf/0.1/",
          "datmm": "http://schema.org/",
          "fabio": "http://purl.org/spar/fabio/"
        }
      }
    ],
    "dct:subject": [
      {
        "@type": "skos:Concept",
        "dct:identifier": "D054459",
        "skos:inScheme": "MeSH",
        "rdfs:label": "Elasticity Imaging Techniques",
        "@context": {
          "rdfs": "http://www.w3.org/2000/01/rdf-schema#",
          "skos": "http://www.w3.org/2004/02/skos/core#",
          "dct": "http://purl.org/dc/terms/"
        }
      }
    ],
    "@context": {
      "dct": "http://purl.org/dc/terms/",
      "foaf": "http://xmlns.com/foaf/0.1/",
      "datmm": "http://schema.org/"
    }
  },
  {
    "@type": "datmm:Dataset",
    "dct:description": "Breast cancer (BC) is the second most commonly diagnosed cancer in the U.S. with more than 250,000 new cases of invasive breast cancers reported in 2017. The majority of women with locally advanced and a subset of patients with operable breast cancer will undergo systemic therapy prior to their surgery (neoadjuvant therapy/ NAT) to reduce the size of tumor(s) and possibly further undergo breast conserving surgery. The Post-NAT-BRCA dataset is a collection of representative sections from breast resections in patients with residual invasive BC following NAT. Histologic sections were prepared and digitized to produce high resolution, microscopic images of treated BC tumors. Also included, are clinical features and expert pathology annotations of tumor cellularity and cell types. ",
    "dct:format": "Unknown",
    "dct:issued": "2019/10/01",
    "foaf:homepage": "https://www.ncbi.nlm.nih.gov/gap",
    "dct:title": "Assessment of Residual Breast Cancer Cellularity after Neoadjuvant Chemotherapy using Digital Pathology (Post-NAT-BRCA)",
    "dct:language": "English",
    "bf:contribution": [],
    "dct:isPartOf": {
      "@type": "datmm:Repository",
      "dct:alternative": "TCIA",
      "foaf:homepage": "https://www.cancerimagingarchive.net",
      "dct:title": "The Cancer Imaging Archive",
      "@context": {
        "dct": "http://purl.org/dc/terms/",
        "foaf": "http://xmlns.com/foaf/0.1/",
        "datmm": "http://schema.org/"
      }
    },
    "frapo:isSupportedBy": [],
    "schema:distribution": [],
    "dct:isReferencedBy": [
      {
        "@type": "datmm:Documentation",
        "rdf:type": "Journal Article",
        "dct:title": "Automatic cellularity assessment from post-treated breast surgical specimens.",
        "dct:bibliographicCitation": "Peikari M, et al. Automatic cellularity assessment from post-treated breast surgical specimens. Cytometry A",
        "prism:doi": "10.1002/cyto.a.23244",
        "fabio:hasPubMedId": "28976721",
        "foaf:homepage": "https://pubmed.ncbi.nlm.nih.gov/28976721",
        "dct:identifier": "28976721",
        "@context": {
          "dct": "http://purl.org/dc/terms/",
          "prism": "http://prismstandard.org/namespaces/basic/3.0/",
          "rdf": "http://www.w3.org/1999/02/22-rdf-syntax-ns#",
          "foaf": "http://xmlns.com/foaf/0.1/",
          "datmm": "http://schema.org/",
          "fabio": "http://purl.org/spar/fabio/"
        }
      }
    ],
    "dct:subject": [],
    "@context": {
      "dct": "http://purl.org/dc/terms/",
      "foaf": "http://xmlns.com/foaf/0.1/",
      "datmm": "http://schema.org/"
    }
  },
  {
    "@type": "datmm:Dataset",
    "dct:description": "This collection includes datasets from 20 subjects with primary newly diagnosed glioblastoma who were treated with surgery and standard concomitant chemo-radiation therapy (CRT) followed by adjuvant chemotherapy.\u00a0 Two MRI exams are included for each patient: within 90 days following CRT completion and at progression (determined clinically, and based on a combination of clinical performance and/or imaging findings, and punctuated by a change in treatment or intervention).\u00a0 ",
    "dct:format": "Unknown",
    "dct:issued": "2018/01/31",
    "foaf:homepage": "https://www.ncbi.nlm.nih.gov/gap",
    "dct:title": "Brain-Tumor-Progression",
    "dct:language": "English",
    "bf:contribution": [],
    "dct:isPartOf": {
      "@type": "datmm:Repository",
      "dct:alternative": "TCIA",
      "foaf:homepage": "https://www.cancerimagingarchive.net",
      "dct:title": "The Cancer Imaging Archive",
      "@context": {
        "dct": "http://purl.org/dc/terms/",
        "foaf": "http://xmlns.com/foaf/0.1/",
        "datmm": "http://schema.org/"
      }
    },
    "frapo:isSupportedBy": [],
    "schema:distribution": [
      {
        "@type": "schema:DataDownload",
        "schema:contentSize": "3.2GB",
        "schema:encodingFormat": "DICOM",
        "schema:inLanguage": "en",
        "schema:name": "Images ",
        "schema:url": "https://wiki.cancerimagingarchive.net/display/Public/Brain-Tumor-Progression/download/attachments/33948119/Brain-Tumor-Progression_2018-01-31.tcia?version=1&modificationDate=1542736404824&api=v2",
        "@context": {
          "schema": "http://schema.org/"
        }
      }
    ],
    "dct:isReferencedBy": [],
    "dct:subject": [],
    "@context": {
      "dct": "http://purl.org/dc/terms/",
      "foaf": "http://xmlns.com/foaf/0.1/",
      "datmm": "http://schema.org/"
    }
  },
  {
    "@type": "datmm:Dataset",
    "dct:description": "Breast cancer is among the most common cancers and a common cause of death among women. Over 39 million breast cancer screening exams are performed every year and are among the most common radiological tests. This creates a high need for accurate image interpretation. Machine learning has shown promise in interpretation of medical images. However, limited data for training and validation remains an issue.",
    "dct:format": "Unknown",
    "dct:issued": "2021/06/08",
    "foaf:homepage": "https://www.ncbi.nlm.nih.gov/gap",
    "dct:title": "Breast Cancer Screening \u2013 Digital Breast Tomosynthesis (BCS-DBT)",
    "dct:language": "English",
    "bf:contribution": [],
    "dct:isPartOf": {
      "@type": "datmm:Repository",
      "dct:alternative": "TCIA",
      "foaf:homepage": "https://www.cancerimagingarchive.net",
      "dct:title": "The Cancer Imaging Archive",
      "@context": {
        "dct": "http://purl.org/dc/terms/",
        "foaf": "http://xmlns.com/foaf/0.1/",
        "datmm": "http://schema.org/"
      }
    },
    "frapo:isSupportedBy": [],
    "schema:distribution": [],
    "dct:isReferencedBy": [],
    "dct:subject": [],
    "@context": {
      "dct": "http://purl.org/dc/terms/",
      "foaf": "http://xmlns.com/foaf/0.1/",
      "datmm": "http://schema.org/"
    }
  },
  {
    "@type": "datmm:Dataset",
    "dct:description": "The Breast-Diagnosis collection contains cases that are high-risk normals, DCIS, fibroids and lobular carcinomas.Each case has 3 or more distinct MR pulse sequences from a Phillips 1.5 T (usual sequences are labeled T2, STIR and BLISS but may occasionally include other pulse sequences and digital mammogram of tumor specimen). Multiple time point studies on the same patient are possible.",
    "dct:format": "Unknown",
    "dct:issued": "2011/11/09",
    "foaf:homepage": "https://www.ncbi.nlm.nih.gov/gap",
    "dct:title": "BREAST-DIAGNOSIS",
    "dct:language": "English",
    "bf:contribution": [],
    "dct:isPartOf": {
      "@type": "datmm:Repository",
      "dct:alternative": "TCIA",
      "foaf:homepage": "https://www.cancerimagingarchive.net",
      "dct:title": "The Cancer Imaging Archive",
      "@context": {
        "dct": "http://purl.org/dc/terms/",
        "foaf": "http://xmlns.com/foaf/0.1/",
        "datmm": "http://schema.org/"
      }
    },
    "frapo:isSupportedBy": [],
    "schema:distribution": [
      {
        "@type": "schema:DataDownload",
        "schema:contentSize": "60.8GB",
        "schema:encodingFormat": "DICOM",
        "schema:inLanguage": "en",
        "schema:name": "Images ",
        "schema:url": "https://wiki.cancerimagingarchive.net/display/Public/BREAST-DIAGNOSIS/download/attachments/2621477/TCIA_BREAST-DIAGNOSIS_06-22-2015.tcia?version=1&modificationDate=1534787403426&api=v2",
        "@context": {
          "schema": "http://schema.org/"
        }
      }
    ],
    "dct:isReferencedBy": [],
    "dct:subject": [],
    "@context": {
      "dct": "http://purl.org/dc/terms/",
      "foaf": "http://xmlns.com/foaf/0.1/",
      "datmm": "http://schema.org/"
    }
  },
  {
    "@type": "datmm:Dataset",
    "dct:description": "The detection of breast cancer metastases to lymph nodes is of great prognostic value for patient treatment. Using machine learning to detect metastatic breast cancer to lymph nodes can increase efficiency of pathologist diagnosis and ultimately ensure patients are accurately staged for prospective treatment. This dataset allows for the objective comparison of breast cancer metastases detection algorithms.",
    "dct:format": "Unknown",
    "dct:issued": "2019/07/18",
    "foaf:homepage": "https://www.ncbi.nlm.nih.gov/gap",
    "dct:title": "Breast Metastases to Axillary Lymph Nodes (SLN-Breast)",
    "dct:language": "English",
    "bf:contribution": [],
    "dct:isPartOf": {
      "@type": "datmm:Repository",
      "dct:alternative": "TCIA",
      "foaf:homepage": "https://www.cancerimagingarchive.net",
      "dct:title": "The Cancer Imaging Archive",
      "@context": {
        "dct": "http://purl.org/dc/terms/",
        "foaf": "http://xmlns.com/foaf/0.1/",
        "datmm": "http://schema.org/"
      }
    },
    "frapo:isSupportedBy": [],
    "schema:distribution": [],
    "dct:isReferencedBy": [],
    "dct:subject": [],
    "@context": {
      "dct": "http://purl.org/dc/terms/",
      "foaf": "http://xmlns.com/foaf/0.1/",
      "datmm": "http://schema.org/"
    }
  },
  {
    "@type": "datmm:Dataset",
    "dct:description": "This collection contains longitudinal DCE MRI studies of 64 patients undergoing neoadjuvant chemotherapy (NACT) for invasive breast cancer.",
    "dct:format": "Unknown",
    "dct:issued": "2016/04/16",
    "foaf:homepage": "https://www.ncbi.nlm.nih.gov/gap",
    "dct:title": "Breast-MRI-NACT-Pilot",
    "dct:language": "English",
    "bf:contribution": [],
    "dct:isPartOf": {
      "@type": "datmm:Repository",
      "dct:alternative": "TCIA",
      "foaf:homepage": "https://www.cancerimagingarchive.net",
      "dct:title": "The Cancer Imaging Archive",
      "@context": {
        "dct": "http://purl.org/dc/terms/",
        "foaf": "http://xmlns.com/foaf/0.1/",
        "datmm": "http://schema.org/"
      }
    },
    "frapo:isSupportedBy": [],
    "schema:distribution": [
      {
        "@type": "schema:DataDownload",
        "schema:contentSize": "19.5 GB",
        "schema:encodingFormat": "DICOM",
        "schema:inLanguage": "en",
        "schema:name": "Images and Segmentations\u00a0",
        "schema:url": "https://wiki.cancerimagingarchive.net/display/Public/Breast-MRI-NACT-Pilot/download/attachments/22513764/doiJNLP-J4OtCtbF.tcia?version=1&modificationDate=1534787445626&api=v2",
        "@context": {
          "schema": "http://schema.org/"
        }
      }
    ],
    "dct:isReferencedBy": [],
    "dct:subject": [],
    "@context": {
      "dct": "http://purl.org/dc/terms/",
      "foaf": "http://xmlns.com/foaf/0.1/",
      "datmm": "http://schema.org/"
    }
  },
  {
    "@type": "datmm:Dataset",
    "dct:description": "Acute lymphoblastic leukemia (ALL) constitutes approximately 25% of the pediatric cancers. In general, the task of identifying immature leukemic blasts from normal cells under the microscope is challenging because morphologically the images of the two cells appear similar.",
    "dct:format": "Unknown",
    "dct:issued": "2019/03/26",
    "foaf:homepage": "https://www.ncbi.nlm.nih.gov/gap",
    "dct:title": "C_NMC_2019 Dataset: ALL Challenge dataset of ISBI 2019",
    "dct:language": "English",
    "bf:contribution": [],
    "dct:isPartOf": {
      "@type": "datmm:Repository",
      "dct:alternative": "TCIA",
      "foaf:homepage": "https://www.cancerimagingarchive.net",
      "dct:title": "The Cancer Imaging Archive",
      "@context": {
        "dct": "http://purl.org/dc/terms/",
        "foaf": "http://xmlns.com/foaf/0.1/",
        "datmm": "http://schema.org/"
      }
    },
    "frapo:isSupportedBy": [],
    "schema:distribution": [],
    "dct:isReferencedBy": [
      {
        "@type": "datmm:Documentation",
        "rdf:type": "Published Erratum",
        "dct:title": "Correction to Lancet Infect Dis 2021; published online June 23. https://doi.org/10.1016/ S1473-3099(21)00330-3.",
        "dct:bibliographicCitation": ". Correction to Lancet Infect Dis 2021; published online June 23. https://doi.org/10.1016/ S1473-3099(21)00330-3. Lancet Infect Dis",
        "prism:doi": "10.1016/S1473-3099(21)00397-2",
        "fabio:hasPubMedId": "34237259",
        "foaf:homepage": "https://pubmed.ncbi.nlm.nih.gov/34237259",
        "dct:identifier": "34237259",
        "@context": {
          "dct": "http://purl.org/dc/terms/",
          "prism": "http://prismstandard.org/namespaces/basic/3.0/",
          "rdf": "http://www.w3.org/1999/02/22-rdf-syntax-ns#",
          "foaf": "http://xmlns.com/foaf/0.1/",
          "datmm": "http://schema.org/",
          "fabio": "http://purl.org/spar/fabio/"
        }
      },
      {
        "@type": "datmm:Documentation",
        "rdf:type": "Published Erratum",
        "dct:title": "Correction to Lancet Infectious Diseases 2020; published online April 29. https://doi.org/10.1016/ S1473-3099(20)30064-5.",
        "dct:bibliographicCitation": ". Correction to Lancet Infectious Diseases 2020; published online April 29. https://doi.org/10.1016/ S1473-3099(20)30064-5. Lancet Infect Dis",
        "prism:doi": "10.1016/S1473-3099(20)30370-4",
        "fabio:hasPubMedId": "32595044",
        "foaf:homepage": "https://pubmed.ncbi.nlm.nih.gov/32595044",
        "dct:identifier": "32595044",
        "@context": {
          "dct": "http://purl.org/dc/terms/",
          "prism": "http://prismstandard.org/namespaces/basic/3.0/",
          "rdf": "http://www.w3.org/1999/02/22-rdf-syntax-ns#",
          "foaf": "http://xmlns.com/foaf/0.1/",
          "datmm": "http://schema.org/",
          "fabio": "http://purl.org/spar/fabio/"
        }
      },
      {
        "@type": "datmm:Documentation",
        "rdf:type": "Journal Article",
        "dct:title": "Correction to Lancet Infect Dis 2020; published online March 11, https://doi.org/10.1016/ S1473-3099(20)30144-4.",
        "dct:bibliographicCitation": ". Correction to Lancet Infect Dis 2020; published online March 11, https://doi.org/10.1016/ S1473-3099(20)30144-4. Lancet Infect Dis",
        "prism:doi": "10.1016/S1473-3099(20)30251-6",
        "fabio:hasPubMedId": "32220652",
        "foaf:homepage": "https://pubmed.ncbi.nlm.nih.gov/32220652",
        "dct:identifier": "32220652",
        "@context": {
          "dct": "http://purl.org/dc/terms/",
          "prism": "http://prismstandard.org/namespaces/basic/3.0/",
          "rdf": "http://www.w3.org/1999/02/22-rdf-syntax-ns#",
          "foaf": "http://xmlns.com/foaf/0.1/",
          "datmm": "http://schema.org/",
          "fabio": "http://purl.org/spar/fabio/"
        }
      },
      {
        "@type": "datmm:Documentation",
        "rdf:type": "Published Erratum",
        "dct:title": "Correction to Lancet Diabetes Endocrinol 2019; published online March 1. DOI:10.1016/ S2213-8587(19)30066-X.",
        "dct:bibliographicCitation": ". Correction to Lancet Diabetes Endocrinol 2019; published online March 1. DOI:10.1016/ S2213-8587(19)30066-X. Lancet Diabetes Endocrinol",
        "prism:doi": "10.1016/S2213-8587(19)30109-3",
        "fabio:hasPubMedId": "30872122",
        "foaf:homepage": "https://pubmed.ncbi.nlm.nih.gov/30872122",
        "dct:identifier": "30872122",
        "@context": {
          "dct": "http://purl.org/dc/terms/",
          "prism": "http://prismstandard.org/namespaces/basic/3.0/",
          "rdf": "http://www.w3.org/1999/02/22-rdf-syntax-ns#",
          "foaf": "http://xmlns.com/foaf/0.1/",
          "datmm": "http://schema.org/",
          "fabio": "http://purl.org/spar/fabio/"
        }
      },
      {
        "@type": "datmm:Documentation",
        "rdf:type": "Journal Article",
        "dct:title": "Prohibitin 2: At a communications crossroads.",
        "dct:bibliographicCitation": "Bavelloni A, et al. Prohibitin 2: At a communications crossroads. IUBMB Life",
        "prism:doi": "10.1002/iub.1366",
        "fabio:hasPubMedId": "25904163",
        "foaf:homepage": "https://pubmed.ncbi.nlm.nih.gov/25904163",
        "dct:identifier": "25904163",
        "@context": {
          "dct": "http://purl.org/dc/terms/",
          "prism": "http://prismstandard.org/namespaces/basic/3.0/",
          "rdf": "http://www.w3.org/1999/02/22-rdf-syntax-ns#",
          "foaf": "http://xmlns.com/foaf/0.1/",
          "datmm": "http://schema.org/",
          "fabio": "http://purl.org/spar/fabio/"
        }
      },
      {
        "@type": "datmm:Documentation",
        "rdf:type": "Retraction of Publication",
        "dct:title": "Retraction for Ramos et al., The second RNA chaperone, Hfq2, is also required for survival under stress and full virulence of Burkholderia cenocepacia J2315.",
        "dct:bibliographicCitation": ". Retraction for Ramos et al., The second RNA chaperone, Hfq2, is also required for survival under stress and full virulence of Burkholderia cenocepacia J2315. J Bacteriol",
        "prism:doi": "10.1128/JB.02242-14",
        "fabio:hasPubMedId": "25319526",
        "foaf:homepage": "https://pubmed.ncbi.nlm.nih.gov/25319526",
        "dct:identifier": "25319526",
        "@context": {
          "dct": "http://purl.org/dc/terms/",
          "prism": "http://prismstandard.org/namespaces/basic/3.0/",
          "rdf": "http://www.w3.org/1999/02/22-rdf-syntax-ns#",
          "foaf": "http://xmlns.com/foaf/0.1/",
          "datmm": "http://schema.org/",
          "fabio": "http://purl.org/spar/fabio/"
        }
      },
      {
        "@type": "datmm:Documentation",
        "rdf:type": "Retraction of Publication",
        "dct:title": "Retraction notice to \u201cDifferential impact of diabetes and hypertension in the brain: adverse effects in grey matter\u201d [Neurobiol. Dis., 44 (2011) 161\u2013173, http://dx.doi.org/10.1016/ j.nbd.2011.06.005].",
        "dct:bibliographicCitation": ". Retraction notice to \u201cDifferential impact of diabetes and hypertension in the brain: adverse effects in grey matter\u201d [Neurobiol. Dis., 44 (2011) 161\u2013173, http://dx.doi.org/10.1016/ j.nbd.2011.06.005]. Neurobiol Dis",
        "prism:doi": "10.1016/j.nbd.2014.05.006",
        "fabio:hasPubMedId": "25077353",
        "foaf:homepage": "https://pubmed.ncbi.nlm.nih.gov/25077353",
        "dct:identifier": "25077353",
        "@context": {
          "dct": "http://purl.org/dc/terms/",
          "prism": "http://prismstandard.org/namespaces/basic/3.0/",
          "rdf": "http://www.w3.org/1999/02/22-rdf-syntax-ns#",
          "foaf": "http://xmlns.com/foaf/0.1/",
          "datmm": "http://schema.org/",
          "fabio": "http://purl.org/spar/fabio/"
        }
      },
      {
        "@type": "datmm:Documentation",
        "rdf:type": "Retraction of Publication",
        "dct:title": "Retraction notice to \u201cDifferential impact of diabetes and hypertension in the brain: adverse effects in white matter\u201d [Neurobiol. Dis., 42 (2011) 446\u2013458, http://dx.doi.org/10.1016/ j.nbd.2011.02.007].",
        "dct:bibliographicCitation": ". Retraction notice to \u201cDifferential impact of diabetes and hypertension in the brain: adverse effects in white matter\u201d [Neurobiol. Dis., 42 (2011) 446\u2013458, http://dx.doi.org/10.1016/ j.nbd.2011.02.007]. Neurobiol Dis",
        "prism:doi": "10.1016/j.nbd.2014.05.005",
        "fabio:hasPubMedId": "25077352",
        "foaf:homepage": "https://pubmed.ncbi.nlm.nih.gov/25077352",
        "dct:identifier": "25077352",
        "@context": {
          "dct": "http://purl.org/dc/terms/",
          "prism": "http://prismstandard.org/namespaces/basic/3.0/",
          "rdf": "http://www.w3.org/1999/02/22-rdf-syntax-ns#",
          "foaf": "http://xmlns.com/foaf/0.1/",
          "datmm": "http://schema.org/",
          "fabio": "http://purl.org/spar/fabio/"
        }
      },
      {
        "@type": "datmm:Documentation",
        "rdf:type": "Letter",
        "dct:title": "[Response to the response of the authors (DOI: 10.1016 / j.neuchi.2014.05.001), following our \"expert opinion\" (DOI: 10.1016 / j.neuchi.2014.06.001)].",
        "dct:bibliographicCitation": "Malca S. [Response to the response of the authors (DOI: 10.1016 / j.neuchi.2014.05.001), following our \"expert opinion\" (DOI: 10.1016 / j.neuchi.2014.06.001)]. Neurochirurgie",
        "prism:doi": "10.1016/j.neuchi.2014.06.003",
        "fabio:hasPubMedId": "25064137",
        "foaf:homepage": "https://pubmed.ncbi.nlm.nih.gov/25064137",
        "dct:identifier": "25064137",
        "@context": {
          "dct": "http://purl.org/dc/terms/",
          "prism": "http://prismstandard.org/namespaces/basic/3.0/",
          "rdf": "http://www.w3.org/1999/02/22-rdf-syntax-ns#",
          "foaf": "http://xmlns.com/foaf/0.1/",
          "datmm": "http://schema.org/",
          "fabio": "http://purl.org/spar/fabio/"
        }
      },
      {
        "@type": "datmm:Documentation",
        "rdf:type": "Letter",
        "dct:title": "[Response to the opinion of the expert Samuel Malca, regarding the article \"Ruptured aneurysm of the hepatic artery after lumbar spinal stenosis surgery. Forensic Reflections \"(Neurosurgery 2014; 60 (1-2): 38-41 DOI: 10.1016 / j.neuchi.2013.08.006.)].",
        "dct:bibliographicCitation": "Jecko V, et al. [Response to the opinion of the expert Samuel Malca, regarding the article \"Ruptured aneurysm of the hepatic artery after lumbar spinal stenosis surgery. Forensic Reflections \"(Neurosurgery 2014; 60 (1-2): 38-41 DOI: 10.1016 / j.neuchi.2013.08.006.)]. Neurochirurgie",
        "prism:doi": "10.1016/j.neuchi.2014.05.001",
        "fabio:hasPubMedId": "24994471",
        "foaf:homepage": "https://pubmed.ncbi.nlm.nih.gov/24994471",
        "dct:identifier": "24994471",
        "@context": {
          "dct": "http://purl.org/dc/terms/",
          "prism": "http://prismstandard.org/namespaces/basic/3.0/",
          "rdf": "http://www.w3.org/1999/02/22-rdf-syntax-ns#",
          "foaf": "http://xmlns.com/foaf/0.1/",
          "datmm": "http://schema.org/",
          "fabio": "http://purl.org/spar/fabio/"
        }
      },
      {
        "@type": "datmm:Documentation",
        "rdf:type": "Letter",
        "dct:title": "[Expert opinion on the article: \"Ruptured aneurysm of the hepatic artery after lumbar spinal stenosis surgery. Forensic Reflections \"(Neurosurgery 2014; 60 (1-2): 38-41 DOI: 10.1016 / j.neuchi.2013.08.006.)].",
        "dct:bibliographicCitation": "Malca S. [Expert opinion on the article: \"Ruptured aneurysm of the hepatic artery after lumbar spinal stenosis surgery. Forensic Reflections \"(Neurosurgery 2014; 60 (1-2): 38-41 DOI: 10.1016 / j.neuchi.2013.08.006.)]. Neurochirurgie",
        "prism:doi": "10.1016/j.neuchi.2014.06.001",
        "fabio:hasPubMedId": "24994470",
        "foaf:homepage": "https://pubmed.ncbi.nlm.nih.gov/24994470",
        "dct:identifier": "24994470",
        "@context": {
          "dct": "http://purl.org/dc/terms/",
          "prism": "http://prismstandard.org/namespaces/basic/3.0/",
          "rdf": "http://www.w3.org/1999/02/22-rdf-syntax-ns#",
          "foaf": "http://xmlns.com/foaf/0.1/",
          "datmm": "http://schema.org/",
          "fabio": "http://purl.org/spar/fabio/"
        }
      },
      {
        "@type": "datmm:Documentation",
        "rdf:type": "Journal Article",
        "dct:title": "WITHDRAWN: Ivory vertebra and systemic mastocytosis. Comments on the article by Frenzel et al.",
        "dct:bibliographicCitation": "Marhadour T, Saraux A. WITHDRAWN: Ivory vertebra and systemic mastocytosis. Comments on the article by Frenzel et al. Joint Bone Spine",
        "prism:doi": "10.1016/j.jbspin.2013.04.006",
        "fabio:hasPubMedId": "23731643",
        "foaf:homepage": "https://pubmed.ncbi.nlm.nih.gov/23731643",
        "dct:identifier": "23731643",
        "@context": {
          "dct": "http://purl.org/dc/terms/",
          "prism": "http://prismstandard.org/namespaces/basic/3.0/",
          "rdf": "http://www.w3.org/1999/02/22-rdf-syntax-ns#",
          "foaf": "http://xmlns.com/foaf/0.1/",
          "datmm": "http://schema.org/",
          "fabio": "http://purl.org/spar/fabio/"
        }
      },
      {
        "@type": "datmm:Documentation",
        "rdf:type": "Comment",
        "dct:title": "Comment on \"Ccl2, Cx3cr1 and Ccl2/Cx3cr1 chemokine deficiencies are not sufficient to cause age-related retinal degeneration\" by Luhmann et\u00a0al. (Exp. Eye Res. 2013; 107: 80.doi: 10.1016).",
        "dct:bibliographicCitation": "Combadi\u00e8re C, et al. Comment on \"Ccl2, Cx3cr1 and Ccl2/Cx3cr1 chemokine deficiencies are not sufficient to cause age-related retinal degeneration\" by Luhmann et\u00a0al. (Exp. Eye Res. 2013; 107: 80.doi: 10.1016). Exp Eye Res",
        "prism:doi": "10.1016/j.exer.2013.02.002",
        "fabio:hasPubMedId": "23402809",
        "foaf:homepage": "https://pubmed.ncbi.nlm.nih.gov/23402809",
        "dct:identifier": "23402809",
        "@context": {
          "dct": "http://purl.org/dc/terms/",
          "prism": "http://prismstandard.org/namespaces/basic/3.0/",
          "rdf": "http://www.w3.org/1999/02/22-rdf-syntax-ns#",
          "foaf": "http://xmlns.com/foaf/0.1/",
          "datmm": "http://schema.org/",
          "fabio": "http://purl.org/spar/fabio/"
        }
      }
    ],
    "dct:subject": [
      {
        "@type": "skos:Concept",
        "dct:identifier": "D006499",
        "skos:inScheme": "MeSH",
        "rdfs:label": "Hepatic Artery",
        "@context": {
          "rdfs": "http://www.w3.org/2000/01/rdf-schema#",
          "skos": "http://www.w3.org/2004/02/skos/core#",
          "dct": "http://purl.org/dc/terms/"
        }
      },
      {
        "@type": "skos:Concept",
        "dct:identifier": "D006499",
        "skos:inScheme": "MeSH",
        "rdfs:label": "Hepatic Artery",
        "@context": {
          "rdfs": "http://www.w3.org/2000/01/rdf-schema#",
          "skos": "http://www.w3.org/2004/02/skos/core#",
          "dct": "http://purl.org/dc/terms/"
        }
      },
      {
        "@type": "skos:Concept",
        "dct:identifier": "D006499",
        "skos:inScheme": "MeSH",
        "rdfs:label": "Hepatic Artery",
        "@context": {
          "rdfs": "http://www.w3.org/2000/01/rdf-schema#",
          "skos": "http://www.w3.org/2004/02/skos/core#",
          "dct": "http://purl.org/dc/terms/"
        }
      }
    ],
    "@context": {
      "dct": "http://purl.org/dc/terms/",
      "foaf": "http://xmlns.com/foaf/0.1/",
      "datmm": "http://schema.org/"
    }
  },
  {
    "@type": "datmm:Dataset",
    "dct:description": "This\u00a0CBIS-DDSM (Curated Breast Imaging Subset of DDSM) is an updated and standardized version of the\u00a0",
    "dct:format": "Unknown",
    "dct:issued": "2017/09/14",
    "foaf:homepage": "https://www.ncbi.nlm.nih.gov/gap",
    "dct:title": "CBIS-DDSM",
    "dct:language": "English",
    "bf:contribution": [],
    "dct:isPartOf": {
      "@type": "datmm:Repository",
      "dct:alternative": "TCIA",
      "foaf:homepage": "https://www.cancerimagingarchive.net",
      "dct:title": "The Cancer Imaging Archive",
      "@context": {
        "dct": "http://purl.org/dc/terms/",
        "foaf": "http://xmlns.com/foaf/0.1/",
        "datmm": "http://schema.org/"
      }
    },
    "frapo:isSupportedBy": [],
    "schema:distribution": [
      {
        "@type": "schema:DataDownload",
        "schema:contentSize": "163.6GB",
        "schema:encodingFormat": "DICOM",
        "schema:inLanguage": "en",
        "schema:name": "Images ",
        "schema:url": "https://wiki.cancerimagingarchive.net/display/Public/CBIS-DDSM/download/attachments/22516629/CBIS-DDSM-All-doiJNLP-zzWs5zfZ.tcia?version=1&modificationDate=1534787024127&api=v2",
        "@context": {
          "schema": "http://schema.org/"
        }
      }
    ],
    "dct:isReferencedBy": [
      {
        "@type": "datmm:Documentation",
        "rdf:type": "Journal Article",
        "dct:title": "A curated mammography data set for use in computer-aided detection and diagnosis research.",
        "dct:bibliographicCitation": "Lee RS, et al. A curated mammography data set for use in computer-aided detection and diagnosis research. Sci Data",
        "prism:doi": "10.1038/sdata.2017.177",
        "fabio:hasPubMedId": "29257132",
        "foaf:homepage": "https://pubmed.ncbi.nlm.nih.gov/29257132",
        "dct:identifier": "29257132",
        "@context": {
          "dct": "http://purl.org/dc/terms/",
          "prism": "http://prismstandard.org/namespaces/basic/3.0/",
          "rdf": "http://www.w3.org/1999/02/22-rdf-syntax-ns#",
          "foaf": "http://xmlns.com/foaf/0.1/",
          "datmm": "http://schema.org/",
          "fabio": "http://purl.org/spar/fabio/"
        }
      }
    ],
    "dct:subject": [
      {
        "@type": "skos:Concept",
        "dct:identifier": "D001943",
        "skos:inScheme": "MeSH",
        "rdfs:label": "Breast Neoplasms",
        "@context": {
          "rdfs": "http://www.w3.org/2000/01/rdf-schema#",
          "skos": "http://www.w3.org/2004/02/skos/core#",
          "dct": "http://purl.org/dc/terms/"
        }
      },
      {
        "@type": "skos:Concept",
        "dct:identifier": "D003936",
        "skos:inScheme": "MeSH",
        "rdfs:label": "Diagnosis, Computer-Assisted",
        "@context": {
          "rdfs": "http://www.w3.org/2000/01/rdf-schema#",
          "skos": "http://www.w3.org/2004/02/skos/core#",
          "dct": "http://purl.org/dc/terms/"
        }
      },
      {
        "@type": "skos:Concept",
        "dct:identifier": "D008327",
        "skos:inScheme": "MeSH",
        "rdfs:label": "Mammography",
        "@context": {
          "rdfs": "http://www.w3.org/2000/01/rdf-schema#",
          "skos": "http://www.w3.org/2004/02/skos/core#",
          "dct": "http://purl.org/dc/terms/"
        }
      }
    ],
    "@context": {
      "dct": "http://purl.org/dc/terms/",
      "foaf": "http://xmlns.com/foaf/0.1/",
      "datmm": "http://schema.org/"
    }
  },
  {
    "@type": "datmm:Dataset",
    "dct:description": "This collection contains data from the Children\u2019s Oncology Group (COG) Clinical Trial ",
    "dct:format": "Unknown",
    "dct:issued": "2021/05/04",
    "foaf:homepage": "https://www.ncbi.nlm.nih.gov/gap",
    "dct:title": "Chemotherapy and Radiation Therapy in Treating Young Patients With Newly Diagnosed, Previously Untreated, High-Risk Medulloblastoma/PNET (ACNS0332)",
    "dct:language": "English",
    "bf:contribution": [],
    "dct:isPartOf": {
      "@type": "datmm:Repository",
      "dct:alternative": "TCIA",
      "foaf:homepage": "https://www.cancerimagingarchive.net",
      "dct:title": "The Cancer Imaging Archive",
      "@context": {
        "dct": "http://purl.org/dc/terms/",
        "foaf": "http://xmlns.com/foaf/0.1/",
        "datmm": "http://schema.org/"
      }
    },
    "frapo:isSupportedBy": [],
    "schema:distribution": [],
    "dct:isReferencedBy": [
      {
        "@type": "datmm:Documentation",
        "rdf:type": "Journal Article",
        "dct:title": "Extensive Molecular and Clinical Heterogeneity in Patients With Histologically Diagnosed CNS-PNET Treated as a Single Entity: A Report From the Children's Oncology Group Randomized ACNS0332 Trial.",
        "dct:bibliographicCitation": "Hwang EI, et al. Extensive Molecular and Clinical Heterogeneity in Patients With Histologically Diagnosed CNS-PNET Treated as a Single Entity: A Report From the Children's Oncology Group Randomized ACNS0332 Trial. J Clin Oncol",
        "prism:doi": "10.1200/JCO.2017.76.4720",
        "fabio:hasPubMedId": "30332335",
        "foaf:homepage": "https://pubmed.ncbi.nlm.nih.gov/30332335",
        "dct:identifier": "30332335",
        "@context": {
          "dct": "http://purl.org/dc/terms/",
          "prism": "http://prismstandard.org/namespaces/basic/3.0/",
          "rdf": "http://www.w3.org/1999/02/22-rdf-syntax-ns#",
          "foaf": "http://xmlns.com/foaf/0.1/",
          "datmm": "http://schema.org/",
          "fabio": "http://purl.org/spar/fabio/"
        }
      }
    ],
    "dct:subject": [],
    "@context": {
      "dct": "http://purl.org/dc/terms/",
      "foaf": "http://xmlns.com/foaf/0.1/",
      "datmm": "http://schema.org/"
    }
  },
  {
    "@type": "datmm:Dataset",
    "dct:description": "Radiology imaging\u00a0 is playing an increasingly vital role in the diagnosis of COVID-19 patients and determining therapeutic options, patient care management and new research directions. Publicly available imaging data is essential to drive new research by permitting the creation of large multi-site cohorts for machine learning based analyses.\u00a0 All too frequently rural populations are underrepresented in such public collections. In fact, the literature demonstrates there is very limited data on COVID-19 outcomes in rural populations, while it is well established that such populations have differentially high expression of key comorbidities.\u00a0 Similarly, while the number of genomes of the SARS-COV-2 virus are rapidly growing in public repositories, few samples represent the variants expressed in rural populations.\u00a0 This gap in available data is of particular importance given that the southern United States, as of July 2020, is the most rapidly expanding\u00a0 COVID-19 hot spot on earth. We have published a collection of radiographic and CT imaging studies for patients who tested positive for COVID-19. Each patient is described by a limited set of clinical data correlates that includes demographics, comorbidities, selected lab data and key radiology findings.\u00a0These data are cross-linked to SARS-COV-2 cDNA sequence data extracted from clinical isolates from the same population, uploaded to the Genbank repository. We believe this collection will help to define appropriate correlative data and contribute samples from this normally underrepresented population to the global research community.",
    "dct:format": "Unknown",
    "dct:issued": "2020/07/13",
    "foaf:homepage": "https://www.ncbi.nlm.nih.gov/gap",
    "dct:title": "Chest Imaging with Clinical and Genomic Correlates Representing a Rural COVID-19 Positive Population (COVID-19-AR)",
    "dct:language": "English",
    "bf:contribution": [],
    "dct:isPartOf": {
      "@type": "datmm:Repository",
      "dct:alternative": "TCIA",
      "foaf:homepage": "https://www.cancerimagingarchive.net",
      "dct:title": "The Cancer Imaging Archive",
      "@context": {
        "dct": "http://purl.org/dc/terms/",
        "foaf": "http://xmlns.com/foaf/0.1/",
        "datmm": "http://schema.org/"
      }
    },
    "frapo:isSupportedBy": [],
    "schema:distribution": [],
    "dct:isReferencedBy": [
      {
        "@type": "datmm:Documentation",
        "rdf:type": "Journal Article",
        "dct:title": "Chest imaging representing a COVID-19 positive rural U.S. population.",
        "dct:bibliographicCitation": "Desai S, et al. Chest imaging representing a COVID-19 positive rural U.S. population. Sci Data",
        "prism:doi": "10.1038/s41597-020-00741-6",
        "fabio:hasPubMedId": "33235265",
        "foaf:homepage": "https://pubmed.ncbi.nlm.nih.gov/33235265",
        "dct:identifier": "33235265",
        "@context": {
          "dct": "http://purl.org/dc/terms/",
          "prism": "http://prismstandard.org/namespaces/basic/3.0/",
          "rdf": "http://www.w3.org/1999/02/22-rdf-syntax-ns#",
          "foaf": "http://xmlns.com/foaf/0.1/",
          "datmm": "http://schema.org/",
          "fabio": "http://purl.org/spar/fabio/"
        }
      },
      {
        "@type": "datmm:Documentation",
        "rdf:type": "Journal Article",
        "dct:title": "Two SARS-CoV-2 Genome Sequences of Isolates from Rural U.S. Patients Harboring the D614G Mutation, Obtained Using Nanopore Sequencing.",
        "dct:bibliographicCitation": "Jenjaroenpun P, et al. Two SARS-CoV-2 Genome Sequences of Isolates from Rural U.S. Patients Harboring the D614G Mutation, Obtained Using Nanopore Sequencing. Microbiol Resour Announc",
        "prism:doi": "10.1128/MRA.01109-20",
        "fabio:hasPubMedId": "33334896",
        "foaf:homepage": "https://pubmed.ncbi.nlm.nih.gov/33334896",
        "dct:identifier": "33334896",
        "@context": {
          "dct": "http://purl.org/dc/terms/",
          "prism": "http://prismstandard.org/namespaces/basic/3.0/",
          "rdf": "http://www.w3.org/1999/02/22-rdf-syntax-ns#",
          "foaf": "http://xmlns.com/foaf/0.1/",
          "datmm": "http://schema.org/",
          "fabio": "http://purl.org/spar/fabio/"
        }
      }
    ],
    "dct:subject": [
      {
        "@type": "skos:Concept",
        "dct:identifier": "D013902",
        "skos:inScheme": "MeSH",
        "rdfs:label": "Radiography, Thoracic",
        "@context": {
          "rdfs": "http://www.w3.org/2000/01/rdf-schema#",
          "skos": "http://www.w3.org/2004/02/skos/core#",
          "dct": "http://purl.org/dc/terms/"
        }
      },
      {
        "@type": "skos:Concept",
        "dct:identifier": "D012424",
        "skos:inScheme": "MeSH",
        "rdfs:label": "Rural Population",
        "@context": {
          "rdfs": "http://www.w3.org/2000/01/rdf-schema#",
          "skos": "http://www.w3.org/2004/02/skos/core#",
          "dct": "http://purl.org/dc/terms/"
        }
      }
    ],
    "@context": {
      "dct": "http://purl.org/dc/terms/",
      "foaf": "http://xmlns.com/foaf/0.1/",
      "datmm": "http://schema.org/"
    }
  },
  {
    "@type": "datmm:Dataset",
    "dct:description": "With advancement of immunotherapies, there has been a paradigm shift in the standard of care for cancer treatment and in the focus of cancer research leveraging the immune system in the tumor immune microenvironment. Therefore, accurate characterization of the tumor microenvironment in each disease site is extremely important. We compared multiplex immunofluorescence assay (mIF) using multispectral microscopy and multiplex immunohistochemistry assay (mIHC). Here we report the comparison of these two assays regarding data acquisition, image analyses, and concordance in marker intensities and characterization of the microenvironment.\u00a0\u00a0",
    "dct:format": "Unknown",
    "dct:issued": "2020/06/04",
    "foaf:homepage": "https://www.ncbi.nlm.nih.gov/gap",
    "dct:title": "Comparison of mIF versus mIHC for immune markers in head and neck carcinoma (HNSCC-mIF-mIHC-comparison)",
    "dct:language": "English",
    "bf:contribution": [],
    "dct:isPartOf": {
      "@type": "datmm:Repository",
      "dct:alternative": "TCIA",
      "foaf:homepage": "https://www.cancerimagingarchive.net",
      "dct:title": "The Cancer Imaging Archive",
      "@context": {
        "dct": "http://purl.org/dc/terms/",
        "foaf": "http://xmlns.com/foaf/0.1/",
        "datmm": "http://schema.org/"
      }
    },
    "frapo:isSupportedBy": [],
    "schema:distribution": [],
    "dct:isReferencedBy": [],
    "dct:subject": [],
    "@context": {
      "dct": "http://purl.org/dc/terms/",
      "foaf": "http://xmlns.com/foaf/0.1/",
      "datmm": "http://schema.org/"
    }
  },
  {
    "@type": "datmm:Dataset",
    "dct:description": "This collection contains subjects from the National Cancer Institute\u2019s ",
    "dct:format": "Unknown",
    "dct:issued": "2020/09/03",
    "foaf:homepage": "https://www.ncbi.nlm.nih.gov/gap",
    "dct:title": "CPTAC-AML",
    "dct:language": "English",
    "bf:contribution": [],
    "dct:isPartOf": {
      "@type": "datmm:Repository",
      "dct:alternative": "TCIA",
      "foaf:homepage": "https://www.cancerimagingarchive.net",
      "dct:title": "The Cancer Imaging Archive",
      "@context": {
        "dct": "http://purl.org/dc/terms/",
        "foaf": "http://xmlns.com/foaf/0.1/",
        "datmm": "http://schema.org/"
      }
    },
    "frapo:isSupportedBy": [],
    "schema:distribution": [],
    "dct:isReferencedBy": [],
    "dct:subject": [],
    "@context": {
      "dct": "http://purl.org/dc/terms/",
      "foaf": "http://xmlns.com/foaf/0.1/",
      "datmm": "http://schema.org/"
    }
  },
  {
    "@type": "datmm:Dataset",
    "dct:description": "This collection contains subjects from the National Cancer Institute\u2019s ",
    "dct:format": "Unknown",
    "dct:issued": "2021/02/02",
    "foaf:homepage": "https://www.ncbi.nlm.nih.gov/gap",
    "dct:title": "CPTAC-BRCA",
    "dct:language": "English",
    "bf:contribution": [],
    "dct:isPartOf": {
      "@type": "datmm:Repository",
      "dct:alternative": "TCIA",
      "foaf:homepage": "https://www.cancerimagingarchive.net",
      "dct:title": "The Cancer Imaging Archive",
      "@context": {
        "dct": "http://purl.org/dc/terms/",
        "foaf": "http://xmlns.com/foaf/0.1/",
        "datmm": "http://schema.org/"
      }
    },
    "frapo:isSupportedBy": [],
    "schema:distribution": [],
    "dct:isReferencedBy": [],
    "dct:subject": [],
    "@context": {
      "dct": "http://purl.org/dc/terms/",
      "foaf": "http://xmlns.com/foaf/0.1/",
      "datmm": "http://schema.org/"
    }
  },
  {
    "@type": "datmm:Dataset",
    "dct:description": "This collection contains subjects from the National Cancer Institute\u2019s ",
    "dct:format": "Unknown",
    "dct:issued": "2020/09/03",
    "foaf:homepage": "https://www.ncbi.nlm.nih.gov/gap",
    "dct:title": "CPTAC-CCRCC",
    "dct:language": "English",
    "bf:contribution": [],
    "dct:isPartOf": {
      "@type": "datmm:Repository",
      "dct:alternative": "TCIA",
      "foaf:homepage": "https://www.cancerimagingarchive.net",
      "dct:title": "The Cancer Imaging Archive",
      "@context": {
        "dct": "http://purl.org/dc/terms/",
        "foaf": "http://xmlns.com/foaf/0.1/",
        "datmm": "http://schema.org/"
      }
    },
    "frapo:isSupportedBy": [],
    "schema:distribution": [],
    "dct:isReferencedBy": [],
    "dct:subject": [],
    "@context": {
      "dct": "http://purl.org/dc/terms/",
      "foaf": "http://xmlns.com/foaf/0.1/",
      "datmm": "http://schema.org/"
    }
  },
  {
    "@type": "datmm:Dataset",
    "dct:description": "This collection contains subjects from the National Cancer Institute\u2019s ",
    "dct:format": "Unknown",
    "dct:issued": "2020/09/03",
    "foaf:homepage": "https://www.ncbi.nlm.nih.gov/gap",
    "dct:title": "CPTAC-CM",
    "dct:language": "English",
    "bf:contribution": [],
    "dct:isPartOf": {
      "@type": "datmm:Repository",
      "dct:alternative": "TCIA",
      "foaf:homepage": "https://www.cancerimagingarchive.net",
      "dct:title": "The Cancer Imaging Archive",
      "@context": {
        "dct": "http://purl.org/dc/terms/",
        "foaf": "http://xmlns.com/foaf/0.1/",
        "datmm": "http://schema.org/"
      }
    },
    "frapo:isSupportedBy": [],
    "schema:distribution": [],
    "dct:isReferencedBy": [],
    "dct:subject": [],
    "@context": {
      "dct": "http://purl.org/dc/terms/",
      "foaf": "http://xmlns.com/foaf/0.1/",
      "datmm": "http://schema.org/"
    }
  },
  {
    "@type": "datmm:Dataset",
    "dct:description": "This collection contains subjects from the National Cancer Institute\u2019s ",
    "dct:format": "Unknown",
    "dct:issued": "2021/02/02",
    "foaf:homepage": "https://www.ncbi.nlm.nih.gov/gap",
    "dct:title": "CPTAC-COAD",
    "dct:language": "English",
    "bf:contribution": [],
    "dct:isPartOf": {
      "@type": "datmm:Repository",
      "dct:alternative": "TCIA",
      "foaf:homepage": "https://www.cancerimagingarchive.net",
      "dct:title": "The Cancer Imaging Archive",
      "@context": {
        "dct": "http://purl.org/dc/terms/",
        "foaf": "http://xmlns.com/foaf/0.1/",
        "datmm": "http://schema.org/"
      }
    },
    "frapo:isSupportedBy": [],
    "schema:distribution": [],
    "dct:isReferencedBy": [],
    "dct:subject": [],
    "@context": {
      "dct": "http://purl.org/dc/terms/",
      "foaf": "http://xmlns.com/foaf/0.1/",
      "datmm": "http://schema.org/"
    }
  },
  {
    "@type": "datmm:Dataset",
    "dct:description": "This collection contains subjects from the National Cancer Institute\u2019s ",
    "dct:format": "Unknown",
    "dct:issued": "2020/09/03",
    "foaf:homepage": "https://www.ncbi.nlm.nih.gov/gap",
    "dct:title": "CPTAC-GBM",
    "dct:language": "English",
    "bf:contribution": [],
    "dct:isPartOf": {
      "@type": "datmm:Repository",
      "dct:alternative": "TCIA",
      "foaf:homepage": "https://www.cancerimagingarchive.net",
      "dct:title": "The Cancer Imaging Archive",
      "@context": {
        "dct": "http://purl.org/dc/terms/",
        "foaf": "http://xmlns.com/foaf/0.1/",
        "datmm": "http://schema.org/"
      }
    },
    "frapo:isSupportedBy": [],
    "schema:distribution": [],
    "dct:isReferencedBy": [],
    "dct:subject": [],
    "@context": {
      "dct": "http://purl.org/dc/terms/",
      "foaf": "http://xmlns.com/foaf/0.1/",
      "datmm": "http://schema.org/"
    }
  },
  {
    "@type": "datmm:Dataset",
    "dct:description": "This collection contains subjects from the National Cancer Institute\u2019s ",
    "dct:format": "Unknown",
    "dct:issued": "2020/09/03",
    "foaf:homepage": "https://www.ncbi.nlm.nih.gov/gap",
    "dct:title": "CPTAC-HNSCC",
    "dct:language": "English",
    "bf:contribution": [],
    "dct:isPartOf": {
      "@type": "datmm:Repository",
      "dct:alternative": "TCIA",
      "foaf:homepage": "https://www.cancerimagingarchive.net",
      "dct:title": "The Cancer Imaging Archive",
      "@context": {
        "dct": "http://purl.org/dc/terms/",
        "foaf": "http://xmlns.com/foaf/0.1/",
        "datmm": "http://schema.org/"
      }
    },
    "frapo:isSupportedBy": [],
    "schema:distribution": [],
    "dct:isReferencedBy": [],
    "dct:subject": [],
    "@context": {
      "dct": "http://purl.org/dc/terms/",
      "foaf": "http://xmlns.com/foaf/0.1/",
      "datmm": "http://schema.org/"
    }
  },
  {
    "@type": "datmm:Dataset",
    "dct:description": "This collection contains subjects from the National Cancer Institute\u2019s ",
    "dct:format": "Unknown",
    "dct:issued": "2021/01/27",
    "foaf:homepage": "https://www.ncbi.nlm.nih.gov/gap",
    "dct:title": "CPTAC-LSCC",
    "dct:language": "English",
    "bf:contribution": [],
    "dct:isPartOf": {
      "@type": "datmm:Repository",
      "dct:alternative": "TCIA",
      "foaf:homepage": "https://www.cancerimagingarchive.net",
      "dct:title": "The Cancer Imaging Archive",
      "@context": {
        "dct": "http://purl.org/dc/terms/",
        "foaf": "http://xmlns.com/foaf/0.1/",
        "datmm": "http://schema.org/"
      }
    },
    "frapo:isSupportedBy": [],
    "schema:distribution": [],
    "dct:isReferencedBy": [],
    "dct:subject": [],
    "@context": {
      "dct": "http://purl.org/dc/terms/",
      "foaf": "http://xmlns.com/foaf/0.1/",
      "datmm": "http://schema.org/"
    }
  },
  {
    "@type": "datmm:Dataset",
    "dct:description": "This collection contains subjects from the National Cancer Institute\u2019s ",
    "dct:format": "Unknown",
    "dct:issued": "2020/09/03",
    "foaf:homepage": "https://www.ncbi.nlm.nih.gov/gap",
    "dct:title": "CPTAC-LUAD",
    "dct:language": "English",
    "bf:contribution": [],
    "dct:isPartOf": {
      "@type": "datmm:Repository",
      "dct:alternative": "TCIA",
      "foaf:homepage": "https://www.cancerimagingarchive.net",
      "dct:title": "The Cancer Imaging Archive",
      "@context": {
        "dct": "http://purl.org/dc/terms/",
        "foaf": "http://xmlns.com/foaf/0.1/",
        "datmm": "http://schema.org/"
      }
    },
    "frapo:isSupportedBy": [],
    "schema:distribution": [],
    "dct:isReferencedBy": [],
    "dct:subject": [],
    "@context": {
      "dct": "http://purl.org/dc/terms/",
      "foaf": "http://xmlns.com/foaf/0.1/",
      "datmm": "http://schema.org/"
    }
  },
  {
    "@type": "datmm:Dataset",
    "dct:description": "This collection contains subjects from the National Cancer Institute\u2019s ",
    "dct:format": "Unknown",
    "dct:issued": "2021/02/02",
    "foaf:homepage": "https://www.ncbi.nlm.nih.gov/gap",
    "dct:title": "CPTAC-OV",
    "dct:language": "English",
    "bf:contribution": [],
    "dct:isPartOf": {
      "@type": "datmm:Repository",
      "dct:alternative": "TCIA",
      "foaf:homepage": "https://www.cancerimagingarchive.net",
      "dct:title": "The Cancer Imaging Archive",
      "@context": {
        "dct": "http://purl.org/dc/terms/",
        "foaf": "http://xmlns.com/foaf/0.1/",
        "datmm": "http://schema.org/"
      }
    },
    "frapo:isSupportedBy": [],
    "schema:distribution": [],
    "dct:isReferencedBy": [],
    "dct:subject": [],
    "@context": {
      "dct": "http://purl.org/dc/terms/",
      "foaf": "http://xmlns.com/foaf/0.1/",
      "datmm": "http://schema.org/"
    }
  },
  {
    "@type": "datmm:Dataset",
    "dct:description": "This collection contains subjects from the National Cancer Institute\u2019s ",
    "dct:format": "Unknown",
    "dct:issued": "2021/02/04",
    "foaf:homepage": "https://www.ncbi.nlm.nih.gov/gap",
    "dct:title": "CPTAC-PDA",
    "dct:language": "English",
    "bf:contribution": [],
    "dct:isPartOf": {
      "@type": "datmm:Repository",
      "dct:alternative": "TCIA",
      "foaf:homepage": "https://www.cancerimagingarchive.net",
      "dct:title": "The Cancer Imaging Archive",
      "@context": {
        "dct": "http://purl.org/dc/terms/",
        "foaf": "http://xmlns.com/foaf/0.1/",
        "datmm": "http://schema.org/"
      }
    },
    "frapo:isSupportedBy": [],
    "schema:distribution": [],
    "dct:isReferencedBy": [],
    "dct:subject": [],
    "@context": {
      "dct": "http://purl.org/dc/terms/",
      "foaf": "http://xmlns.com/foaf/0.1/",
      "datmm": "http://schema.org/"
    }
  },
  {
    "@type": "datmm:Dataset",
    "dct:description": "This collection contains subjects from the National Cancer Institute\u2019s ",
    "dct:format": "Unknown",
    "dct:issued": "2020/09/03",
    "foaf:homepage": "https://www.ncbi.nlm.nih.gov/gap",
    "dct:title": "CPTAC-SAR",
    "dct:language": "English",
    "bf:contribution": [],
    "dct:isPartOf": {
      "@type": "datmm:Repository",
      "dct:alternative": "TCIA",
      "foaf:homepage": "https://www.cancerimagingarchive.net",
      "dct:title": "The Cancer Imaging Archive",
      "@context": {
        "dct": "http://purl.org/dc/terms/",
        "foaf": "http://xmlns.com/foaf/0.1/",
        "datmm": "http://schema.org/"
      }
    },
    "frapo:isSupportedBy": [],
    "schema:distribution": [],
    "dct:isReferencedBy": [],
    "dct:subject": [],
    "@context": {
      "dct": "http://purl.org/dc/terms/",
      "foaf": "http://xmlns.com/foaf/0.1/",
      "datmm": "http://schema.org/"
    }
  },
  {
    "@type": "datmm:Dataset",
    "dct:description": "This collection contains subjects from the National Cancer Institute\u2019s ",
    "dct:format": "Unknown",
    "dct:issued": "2020/09/03",
    "foaf:homepage": "https://www.ncbi.nlm.nih.gov/gap",
    "dct:title": "CPTAC-UCEC",
    "dct:language": "English",
    "bf:contribution": [],
    "dct:isPartOf": {
      "@type": "datmm:Repository",
      "dct:alternative": "TCIA",
      "foaf:homepage": "https://www.cancerimagingarchive.net",
      "dct:title": "The Cancer Imaging Archive",
      "@context": {
        "dct": "http://purl.org/dc/terms/",
        "foaf": "http://xmlns.com/foaf/0.1/",
        "datmm": "http://schema.org/"
      }
    },
    "frapo:isSupportedBy": [],
    "schema:distribution": [],
    "dct:isReferencedBy": [],
    "dct:subject": [],
    "@context": {
      "dct": "http://purl.org/dc/terms/",
      "foaf": "http://xmlns.com/foaf/0.1/",
      "datmm": "http://schema.org/"
    }
  },
  {
    "@type": "datmm:Dataset",
    "dct:description": "\n This collection consists of 17 CT scans of the Credence Cartridge Radiomics (CCR) phantom, which was designed for use in studies of texture feature robustness. The scans were acquired at four medical centers using each center\u2019s chest protocol and were taken using GE (7 scans), Philips (5 scans), Siemens (2 scans), and Toshiba (3 scans) scanners. The CCR phantom has 10 cartridges, each with a unique texture, Fig 1. The first four cartridges are 3D printed ABS plastic with 20%, 30%, 40%, and 50% honeycomb fill, and they provide regular, periodic textures. The next three cartridges provide natural textures: sycamore wood, cork, and extra dense cork. A cartridges of shredded rubber particles provides textures similar to those of non-small cell lung cancer. The ninth cartridge is solid, homogenous acrylic and provides a minimal texture control. Finally, the 10",
    "dct:format": "Unknown",
    "dct:issued": "2017/07/28",
    "foaf:homepage": "https://www.ncbi.nlm.nih.gov/gap",
    "dct:title": "Credence Cartridge Radiomics Phantom CT Scans",
    "dct:language": "English",
    "bf:contribution": [],
    "dct:isPartOf": {
      "@type": "datmm:Repository",
      "dct:alternative": "TCIA",
      "foaf:homepage": "https://www.cancerimagingarchive.net",
      "dct:title": "The Cancer Imaging Archive",
      "@context": {
        "dct": "http://purl.org/dc/terms/",
        "foaf": "http://xmlns.com/foaf/0.1/",
        "datmm": "http://schema.org/"
      }
    },
    "frapo:isSupportedBy": [],
    "schema:distribution": [
      {
        "@type": "schema:DataDownload",
        "schema:contentSize": "1.33 GB",
        "schema:encodingFormat": "DICOM",
        "schema:inLanguage": "en",
        "schema:name": "Images\u00a0and Radiation Therapy Structures ",
        "schema:url": "https://wiki.cancerimagingarchive.net/display/Public/Credence+Cartridge+Radiomics+Phantom+CT+Scans/download/attachments/24284300/CC-Radiomics-Phantom-7-28-2017-doiJNLP-2vcxNoRY.tcia?version=1&modificationDate=1534787033680&api=v2",
        "@context": {
          "schema": "http://schema.org/"
        }
      }
    ],
    "dct:isReferencedBy": [],
    "dct:subject": [],
    "@context": {
      "dct": "http://purl.org/dc/terms/",
      "foaf": "http://xmlns.com/foaf/0.1/",
      "datmm": "http://schema.org/"
    }
  },
  {
    "@type": "datmm:Dataset",
    "dct:description": "\n \n \n This collection consists of 251 CT scans of Credence Cartridge Radiomic (CCR) phantom. This texture phantom was developed to investigate the feature robustness in the emerging field of radiomics. This phantom dataset was acquired on 4-8 CT scanners using a set of imaging parameters (e.g., reconstruction Field of View, Slice thickness, reconstruction kernels, mAs, and Pitch). A controlled scanning approach was employed to assess the variability in radiomic features due to each imaging parameter. This dataset will be useful to radiomic research community to identify a subset of robust radiomic features and for establishing the ground truths for future clinical investigations.",
    "dct:format": "Unknown",
    "dct:issued": "02-27-2019",
    "foaf:homepage": "https://www.ncbi.nlm.nih.gov/gap",
    "dct:title": "Credence Cartridge Radiomics Phantom CT Scans with Controlled Scanning Approach (CC-Radiomics-Phantom-2)",
    "dct:language": "English",
    "bf:contribution": [],
    "dct:isPartOf": {
      "@type": "datmm:Repository",
      "dct:alternative": "TCIA",
      "foaf:homepage": "https://www.cancerimagingarchive.net",
      "dct:title": "The Cancer Imaging Archive",
      "@context": {
        "dct": "http://purl.org/dc/terms/",
        "foaf": "http://xmlns.com/foaf/0.1/",
        "datmm": "http://schema.org/"
      }
    },
    "frapo:isSupportedBy": [],
    "schema:distribution": [
      {
        "@type": "schema:DataDownload",
        "schema:contentSize": "30.5GB",
        "schema:encodingFormat": "DICOM",
        "schema:inLanguage": "en",
        "schema:name": "Images ",
        "schema:url": "https://wiki.cancerimagingarchive.net/pages/viewpage.action?pageId=39879218/download/attachments/39879218/CC-Radiomics-Phantom-2-NBIA-manifest.tcia?version=1&modificationDate=1551287978550&api=v2",
        "@context": {
          "schema": "http://schema.org/"
        }
      }
    ],
    "dct:isReferencedBy": [],
    "dct:subject": [],
    "@context": {
      "dct": "http://purl.org/dc/terms/",
      "foaf": "http://xmlns.com/foaf/0.1/",
      "datmm": "http://schema.org/"
    }
  },
  {
    "@type": "datmm:Dataset",
    "dct:description": "In 2004 when presenting the NCI Executive Committee the ACRIN proposal to conduct the National CT Colonography Trial (6664), a case was made that publicly accessible image data sharing would offer a valuable research asset to a wide image processing research community. Adding to the many merits of that proposal, the data-sharing component was strongly endorsed. ACRIN completed the trial expeditiously and its results were published in NEJM in fall 2008 to wide interest. ACRIN has graciously allowed the wider research community access to a portion of the data from that trial here on TCIA, including spreadsheets identifying positive and negative polyp cases.\u00a0",
    "dct:format": "Unknown",
    "dct:issued": "2013/11/15",
    "foaf:homepage": "https://www.ncbi.nlm.nih.gov/gap",
    "dct:title": "CT COLONOGRAPHY",
    "dct:language": "English",
    "bf:contribution": [],
    "dct:isPartOf": {
      "@type": "datmm:Repository",
      "dct:alternative": "TCIA",
      "foaf:homepage": "https://www.cancerimagingarchive.net",
      "dct:title": "The Cancer Imaging Archive",
      "@context": {
        "dct": "http://purl.org/dc/terms/",
        "foaf": "http://xmlns.com/foaf/0.1/",
        "datmm": "http://schema.org/"
      }
    },
    "frapo:isSupportedBy": [],
    "schema:distribution": [
      {
        "@type": "schema:DataDownload",
        "schema:contentSize": "462.6GB",
        "schema:encodingFormat": "DICOM",
        "schema:inLanguage": "en",
        "schema:name": "Images ",
        "schema:url": "https://wiki.cancerimagingarchive.net/display/Public/CT+COLONOGRAPHY/download/attachments/3539213/TCIA_CT_COLONOGRAPHY_06-22-2015.tcia?version=1&modificationDate=1534787407262&api=v2",
        "@context": {
          "schema": "http://schema.org/"
        }
      },
      {
        "@type": "schema:DataDownload",
        "schema:encodingFormat": "DICOM",
        "schema:inLanguage": "en",
        "schema:name": "DICOM Metadata Digest ",
        "schema:url": "https://wiki.cancerimagingarchive.net/display/Public/CT+COLONOGRAPHY/download/attachments/3539213/CTColonography_MetaData.csv?version=1&modificationDate=1495563713054&api=v2",
        "@context": {
          "schema": "http://schema.org/"
        }
      }
    ],
    "dct:isReferencedBy": [
      {
        "@type": "datmm:Documentation",
        "rdf:type": "Clinical Trial",
        "dct:title": "Accuracy of CT colonography for detection of large adenomas and cancers.",
        "dct:bibliographicCitation": "Johnson CD, et al. Accuracy of CT colonography for detection of large adenomas and cancers. N Engl J Med",
        "prism:doi": "10.1056/NEJMoa0800996",
        "fabio:hasPubMedId": "18799557",
        "foaf:homepage": "https://pubmed.ncbi.nlm.nih.gov/18799557",
        "dct:identifier": "18799557",
        "@context": {
          "dct": "http://purl.org/dc/terms/",
          "prism": "http://prismstandard.org/namespaces/basic/3.0/",
          "rdf": "http://www.w3.org/1999/02/22-rdf-syntax-ns#",
          "foaf": "http://xmlns.com/foaf/0.1/",
          "datmm": "http://schema.org/",
          "fabio": "http://purl.org/spar/fabio/"
        }
      }
    ],
    "dct:subject": [
      {
        "@type": "skos:Concept",
        "dct:identifier": "D023881",
        "skos:inScheme": "MeSH",
        "rdfs:label": "Colonography, Computed Tomographic",
        "@context": {
          "rdfs": "http://www.w3.org/2000/01/rdf-schema#",
          "skos": "http://www.w3.org/2004/02/skos/core#",
          "dct": "http://purl.org/dc/terms/"
        }
      }
    ],
    "@context": {
      "dct": "http://purl.org/dc/terms/",
      "foaf": "http://xmlns.com/foaf/0.1/",
      "datmm": "http://schema.org/"
    }
  },
  {
    "@type": "datmm:Dataset",
    "dct:description": "These retrospective NIfTI image datasets consists of unenhanced chest CTs:\u00a0",
    "dct:format": "Unknown",
    "dct:issued": "2021/05/25",
    "foaf:homepage": "https://www.ncbi.nlm.nih.gov/gap",
    "dct:title": "CT Images in COVID-19",
    "dct:language": "English",
    "bf:contribution": [],
    "dct:isPartOf": {
      "@type": "datmm:Repository",
      "dct:alternative": "TCIA",
      "foaf:homepage": "https://www.cancerimagingarchive.net",
      "dct:title": "The Cancer Imaging Archive",
      "@context": {
        "dct": "http://purl.org/dc/terms/",
        "foaf": "http://xmlns.com/foaf/0.1/",
        "datmm": "http://schema.org/"
      }
    },
    "frapo:isSupportedBy": [],
    "schema:distribution": [],
    "dct:isReferencedBy": [
      {
        "@type": "datmm:Documentation",
        "rdf:type": "Journal Article",
        "dct:title": "Artificial intelligence for the detection of COVID-19 pneumonia on chest CT using multinational datasets.",
        "dct:bibliographicCitation": "Harmon SA, et al. Artificial intelligence for the detection of COVID-19 pneumonia on chest CT using multinational datasets. Nat Commun",
        "prism:doi": "10.1038/s41467-020-17971-2",
        "fabio:hasPubMedId": "32796848",
        "foaf:homepage": "https://pubmed.ncbi.nlm.nih.gov/32796848",
        "dct:identifier": "32796848",
        "@context": {
          "dct": "http://purl.org/dc/terms/",
          "prism": "http://prismstandard.org/namespaces/basic/3.0/",
          "rdf": "http://www.w3.org/1999/02/22-rdf-syntax-ns#",
          "foaf": "http://xmlns.com/foaf/0.1/",
          "datmm": "http://schema.org/",
          "fabio": "http://purl.org/spar/fabio/"
        }
      }
    ],
    "dct:subject": [
      {
        "@type": "skos:Concept",
        "dct:identifier": "D001185",
        "skos:inScheme": "MeSH",
        "rdfs:label": "Artificial Intelligence",
        "@context": {
          "rdfs": "http://www.w3.org/2000/01/rdf-schema#",
          "skos": "http://www.w3.org/2004/02/skos/core#",
          "dct": "http://purl.org/dc/terms/"
        }
      }
    ],
    "@context": {
      "dct": "http://purl.org/dc/terms/",
      "foaf": "http://xmlns.com/foaf/0.1/",
      "datmm": "http://schema.org/"
    }
  },
  {
    "@type": "datmm:Dataset",
    "dct:description": "This collection consists of Computed Tomography (CT) images of the mediastinum and abdomen in which lymph node positions are marked by radiologists at the National Institutes of Health, Clinical Center. Radiologists at the ",
    "dct:format": "Unknown",
    "dct:issued": "2015/12/14",
    "foaf:homepage": "https://www.ncbi.nlm.nih.gov/gap",
    "dct:title": "CT Lymph Nodes",
    "dct:language": "English",
    "bf:contribution": [],
    "dct:isPartOf": {
      "@type": "datmm:Repository",
      "dct:alternative": "TCIA",
      "foaf:homepage": "https://www.cancerimagingarchive.net",
      "dct:title": "The Cancer Imaging Archive",
      "@context": {
        "dct": "http://purl.org/dc/terms/",
        "foaf": "http://xmlns.com/foaf/0.1/",
        "datmm": "http://schema.org/"
      }
    },
    "frapo:isSupportedBy": [],
    "schema:distribution": [
      {
        "@type": "schema:DataDownload",
        "schema:contentSize": "57.8GB",
        "schema:encodingFormat": "DICOM",
        "schema:inLanguage": "en",
        "schema:name": "Images ",
        "schema:url": "https://wiki.cancerimagingarchive.net/display/Public/CT+Lymph+Nodes/download/attachments/19726546/TCIA_CT_Lymph_Nodes_06-22-2015.tcia?version=1&modificationDate=1534787005035&api=v2",
        "@context": {
          "schema": "http://schema.org/"
        }
      }
    ],
    "dct:isReferencedBy": [
      {
        "@type": "datmm:Documentation",
        "rdf:type": "Journal Article",
        "dct:title": "A new 2.5D representation for lymph node detection using random sets of deep convolutional neural network observations.",
        "dct:bibliographicCitation": "Roth HR, et al. A new 2.5D representation for lymph node detection using random sets of deep convolutional neural network observations. Med Image Comput Comput Assist Interv",
        "prism:doi": "10.1007/978-3-319-10404-1_65",
        "fabio:hasPubMedId": "25333158",
        "foaf:homepage": "https://pubmed.ncbi.nlm.nih.gov/25333158",
        "dct:identifier": "25333158",
        "@context": {
          "dct": "http://purl.org/dc/terms/",
          "prism": "http://prismstandard.org/namespaces/basic/3.0/",
          "rdf": "http://www.w3.org/1999/02/22-rdf-syntax-ns#",
          "foaf": "http://xmlns.com/foaf/0.1/",
          "datmm": "http://schema.org/",
          "fabio": "http://purl.org/spar/fabio/"
        }
      },
      {
        "@type": "datmm:Documentation",
        "rdf:type": "Comment",
        "dct:title": "Underserved Does Not Mean Undeserved: Unfurling the HCV Care in the Safety Net.",
        "dct:bibliographicCitation": "Khalili M, Wong RJ. Underserved Does Not Mean Undeserved: Unfurling the HCV Care in the Safety Net. Dig Dis Sci",
        "prism:doi": "10.1007/s10620-018-5316-9",
        "fabio:hasPubMedId": "30311153",
        "foaf:homepage": "https://pubmed.ncbi.nlm.nih.gov/30311153",
        "dct:identifier": "30311153",
        "@context": {
          "dct": "http://purl.org/dc/terms/",
          "prism": "http://prismstandard.org/namespaces/basic/3.0/",
          "rdf": "http://www.w3.org/1999/02/22-rdf-syntax-ns#",
          "foaf": "http://xmlns.com/foaf/0.1/",
          "datmm": "http://schema.org/",
          "fabio": "http://purl.org/spar/fabio/"
        }
      },
      {
        "@type": "datmm:Documentation",
        "rdf:type": "Published Erratum",
        "dct:title": "Erratum to: Rectocutaneous fistula with transmigration of the suture: a rare delayed complication of vault fixation with the sacrospinous ligament.",
        "dct:bibliographicCitation": "Kadam PD, Chuan HH. Erratum to: Rectocutaneous fistula with transmigration of the suture: a rare delayed complication of vault fixation with the sacrospinous ligament. Int Urogynecol J",
        "prism:doi": "10.1007/s00192-016-2952-5",
        "fabio:hasPubMedId": "26811110",
        "foaf:homepage": "https://pubmed.ncbi.nlm.nih.gov/26811110",
        "dct:identifier": "26811110",
        "@context": {
          "dct": "http://purl.org/dc/terms/",
          "prism": "http://prismstandard.org/namespaces/basic/3.0/",
          "rdf": "http://www.w3.org/1999/02/22-rdf-syntax-ns#",
          "foaf": "http://xmlns.com/foaf/0.1/",
          "datmm": "http://schema.org/",
          "fabio": "http://purl.org/spar/fabio/"
        }
      }
    ],
    "dct:subject": [
      {
        "@type": "skos:Concept",
        "dct:identifier": "D000465",
        "skos:inScheme": "MeSH",
        "rdfs:label": "Algorithms",
        "@context": {
          "rdfs": "http://www.w3.org/2000/01/rdf-schema#",
          "skos": "http://www.w3.org/2004/02/skos/core#",
          "dct": "http://purl.org/dc/terms/"
        }
      },
      {
        "@type": "skos:Concept",
        "dct:identifier": "D015233",
        "skos:inScheme": "MeSH",
        "rdfs:label": "Models, Statistical",
        "@context": {
          "rdfs": "http://www.w3.org/2000/01/rdf-schema#",
          "skos": "http://www.w3.org/2004/02/skos/core#",
          "dct": "http://purl.org/dc/terms/"
        }
      },
      {
        "@type": "skos:Concept",
        "dct:identifier": "D006526",
        "skos:inScheme": "MeSH",
        "rdfs:label": "Hepatitis C",
        "@context": {
          "rdfs": "http://www.w3.org/2000/01/rdf-schema#",
          "skos": "http://www.w3.org/2004/02/skos/core#",
          "dct": "http://purl.org/dc/terms/"
        }
      }
    ],
    "@context": {
      "dct": "http://purl.org/dc/terms/",
      "foaf": "http://xmlns.com/foaf/0.1/",
      "datmm": "http://schema.org/"
    }
  },
  {
    "@type": "datmm:Dataset",
    "dct:description": "This dataset consists of 140 computed tomography (CT) scans, each with five organs labeled in 3D: lung, bones, liver, kidneys and bladder. The brain is also labeled on the minority of scans which show it.",
    "dct:format": "Unknown",
    "dct:issued": "2020/01/09",
    "foaf:homepage": "https://www.ncbi.nlm.nih.gov/gap",
    "dct:title": "CT-ORG: CT volumes with multiple organ segmentations",
    "dct:language": "English",
    "bf:contribution": [],
    "dct:isPartOf": {
      "@type": "datmm:Repository",
      "dct:alternative": "TCIA",
      "foaf:homepage": "https://www.cancerimagingarchive.net",
      "dct:title": "The Cancer Imaging Archive",
      "@context": {
        "dct": "http://purl.org/dc/terms/",
        "foaf": "http://xmlns.com/foaf/0.1/",
        "datmm": "http://schema.org/"
      }
    },
    "frapo:isSupportedBy": [],
    "schema:distribution": [],
    "dct:isReferencedBy": [],
    "dct:subject": [],
    "@context": {
      "dct": "http://purl.org/dc/terms/",
      "foaf": "http://xmlns.com/foaf/0.1/",
      "datmm": "http://schema.org/"
    }
  },
  {
    "@type": "datmm:Dataset",
    "dct:description": "\n \n There currently is a dearth of phantom scans on large samples.",
    "dct:format": "Unknown",
    "dct:issued": "2019",
    "foaf:homepage": "https://www.ncbi.nlm.nih.gov/gap",
    "dct:title": "CT Phantom Scans for Head, Chest, and Controlled Protocols on 100 Scanners (CC-Radiomics-Phantom-3)",
    "dct:language": "English",
    "bf:contribution": [],
    "dct:isPartOf": {
      "@type": "datmm:Repository",
      "dct:alternative": "TCIA",
      "foaf:homepage": "https://www.cancerimagingarchive.net",
      "dct:title": "The Cancer Imaging Archive",
      "@context": {
        "dct": "http://purl.org/dc/terms/",
        "foaf": "http://xmlns.com/foaf/0.1/",
        "datmm": "http://schema.org/"
      }
    },
    "frapo:isSupportedBy": [],
    "schema:distribution": [
      {
        "@type": "schema:DataDownload",
        "schema:contentSize": "13.4GB",
        "schema:encodingFormat": "DICOM",
        "schema:inLanguage": "en",
        "schema:name": "Images and Radiation Therapy Structures ",
        "schema:url": "https://wiki.cancerimagingarchive.net/pages/viewpage.action?pageId=46334020/download/attachments/46334020/CC-Radiomics-Phantom-3-NBIA-manifest.tcia?version=1&modificationDate=1563986884466&api=v2",
        "@context": {
          "schema": "http://schema.org/"
        }
      },
      {
        "@type": "schema:DataDownload",
        "schema:encodingFormat": "DICOM",
        "schema:inLanguage": "en",
        "schema:name": "\nAcquisition & reconstruction settings\n",
        "schema:url": "https://wiki.cancerimagingarchive.net/pages/viewpage.action?pageId=46334020/download/attachments/46334020/TCIA_CCR_Parameters_Anonymized.xlsx?version=1&modificationDate=1556115106104&api=v2",
        "@context": {
          "schema": "http://schema.org/"
        }
      }
    ],
    "dct:isReferencedBy": [],
    "dct:subject": [],
    "@context": {
      "dct": "http://purl.org/dc/terms/",
      "foaf": "http://xmlns.com/foaf/0.1/",
      "datmm": "http://schema.org/"
    }
  },
  {
    "@type": "datmm:Dataset",
    "dct:description": "This collection contains CT scans and segmentations from subjects from the training set of the ",
    "dct:format": "Unknown",
    "dct:issued": "2020/06/18",
    "foaf:homepage": "https://www.ncbi.nlm.nih.gov/gap",
    "dct:title": "Data from the training set of the 2019 Kidney and Kidney Tumor Segmentation Challenge (C4KC-KiTS)",
    "dct:language": "English",
    "bf:contribution": [],
    "dct:isPartOf": {
      "@type": "datmm:Repository",
      "dct:alternative": "TCIA",
      "foaf:homepage": "https://www.cancerimagingarchive.net",
      "dct:title": "The Cancer Imaging Archive",
      "@context": {
        "dct": "http://purl.org/dc/terms/",
        "foaf": "http://xmlns.com/foaf/0.1/",
        "datmm": "http://schema.org/"
      }
    },
    "frapo:isSupportedBy": [],
    "schema:distribution": [],
    "dct:isReferencedBy": [
      {
        "@type": "datmm:Documentation",
        "rdf:type": "Journal Article",
        "dct:title": "The state of the art in kidney and kidney tumor segmentation in contrast-enhanced CT imaging: Results of the KiTS19 challenge.",
        "dct:bibliographicCitation": "Heller N, et al. The state of the art in kidney and kidney tumor segmentation in contrast-enhanced CT imaging: Results of the KiTS19 challenge. Med Image Anal",
        "prism:doi": "10.1016/j.media.2020.101821",
        "fabio:hasPubMedId": "33049579",
        "foaf:homepage": "https://pubmed.ncbi.nlm.nih.gov/33049579",
        "dct:identifier": "33049579",
        "@context": {
          "dct": "http://purl.org/dc/terms/",
          "prism": "http://prismstandard.org/namespaces/basic/3.0/",
          "rdf": "http://www.w3.org/1999/02/22-rdf-syntax-ns#",
          "foaf": "http://xmlns.com/foaf/0.1/",
          "datmm": "http://schema.org/",
          "fabio": "http://purl.org/spar/fabio/"
        }
      }
    ],
    "dct:subject": [
      {
        "@type": "skos:Concept",
        "dct:identifier": "D007680",
        "skos:inScheme": "MeSH",
        "rdfs:label": "Kidney Neoplasms",
        "@context": {
          "rdfs": "http://www.w3.org/2000/01/rdf-schema#",
          "skos": "http://www.w3.org/2004/02/skos/core#",
          "dct": "http://purl.org/dc/terms/"
        }
      },
      {
        "@type": "skos:Concept",
        "dct:identifier": "D014057",
        "skos:inScheme": "MeSH",
        "rdfs:label": "Tomography, X-Ray Computed",
        "@context": {
          "rdfs": "http://www.w3.org/2000/01/rdf-schema#",
          "skos": "http://www.w3.org/2004/02/skos/core#",
          "dct": "http://purl.org/dc/terms/"
        }
      }
    ],
    "@context": {
      "dct": "http://purl.org/dc/terms/",
      "foaf": "http://xmlns.com/foaf/0.1/",
      "datmm": "http://schema.org/"
    }
  },
  {
    "@type": "datmm:Dataset",
    "dct:description": "This collection contains data from the  National Cancer Institute Clinical Trial NCT00118209",
    "dct:format": "Unknown",
    "dct:issued": "2021/03/30",
    "foaf:homepage": "https://www.ncbi.nlm.nih.gov/gap",
    "dct:title": "Dose-Adjusted EPOCH-R Compared With R-CHOP as Frontline Therapy for Diffuse Large B-Cell Lymphoma (CALGB50303)",
    "dct:language": "English",
    "bf:contribution": [],
    "dct:isPartOf": {
      "@type": "datmm:Repository",
      "dct:alternative": "TCIA",
      "foaf:homepage": "https://www.cancerimagingarchive.net",
      "dct:title": "The Cancer Imaging Archive",
      "@context": {
        "dct": "http://purl.org/dc/terms/",
        "foaf": "http://xmlns.com/foaf/0.1/",
        "datmm": "http://schema.org/"
      }
    },
    "frapo:isSupportedBy": [],
    "schema:distribution": [],
    "dct:isReferencedBy": [
      {
        "@type": "datmm:Documentation",
        "rdf:type": "Journal Article",
        "dct:title": "Dose-Adjusted EPOCH-R Compared With R-CHOP as Frontline Therapy for Diffuse Large B-Cell Lymphoma: Clinical Outcomes of the Phase III Intergroup Trial Alliance/CALGB 50303.",
        "dct:bibliographicCitation": "Bartlett NL, et al. Dose-Adjusted EPOCH-R Compared With R-CHOP as Frontline Therapy for Diffuse Large B-Cell Lymphoma: Clinical Outcomes of the Phase III Intergroup Trial Alliance/CALGB 50303. J Clin Oncol",
        "prism:doi": "10.1200/JCO.18.01994",
        "fabio:hasPubMedId": "30939090",
        "foaf:homepage": "https://pubmed.ncbi.nlm.nih.gov/30939090",
        "dct:identifier": "30939090",
        "@context": {
          "dct": "http://purl.org/dc/terms/",
          "prism": "http://prismstandard.org/namespaces/basic/3.0/",
          "rdf": "http://www.w3.org/1999/02/22-rdf-syntax-ns#",
          "foaf": "http://xmlns.com/foaf/0.1/",
          "datmm": "http://schema.org/",
          "fabio": "http://purl.org/spar/fabio/"
        }
      }
    ],
    "dct:subject": [],
    "@context": {
      "dct": "http://purl.org/dc/terms/",
      "foaf": "http://xmlns.com/foaf/0.1/",
      "datmm": "http://schema.org/"
    }
  },
  {
    "@type": "datmm:Dataset",
    "dct:description": "Breast MRI is a common image modality to assess extent of disease in breast cancer patients. Recent studies show that MRI has a potential in prognosis of patient sort and long term outcomes as well as predicting pathological and genomic features of the tumors. However, large, well annotated datasets are needed to make further progress in the field.\u00a0In this dataset, we share MRI imaging and other data for 922 patients with invasive breast cancer. Their prone position axial breast MRI images were acquired by 1.5T or 3T scanners. Following MRI sequences are shared: a non-fat saturated T1-weighted sequence, a fat-saturated gradient echo T1-weighted pre-contrast sequence, and mostly three to four post-contrast sequences.",
    "dct:format": "Unknown",
    "dct:issued": "2021/04/06",
    "foaf:homepage": "https://www.ncbi.nlm.nih.gov/gap",
    "dct:title": "Dynamic contrast-enhanced magnetic resonance images of breast cancer patients with tumor locations (Duke-Breast-Cancer-MRI)",
    "dct:language": "English",
    "bf:contribution": [],
    "dct:isPartOf": {
      "@type": "datmm:Repository",
      "dct:alternative": "TCIA",
      "foaf:homepage": "https://www.cancerimagingarchive.net",
      "dct:title": "The Cancer Imaging Archive",
      "@context": {
        "dct": "http://purl.org/dc/terms/",
        "foaf": "http://xmlns.com/foaf/0.1/",
        "datmm": "http://schema.org/"
      }
    },
    "frapo:isSupportedBy": [],
    "schema:distribution": [],
    "dct:isReferencedBy": [
      {
        "@type": "datmm:Documentation",
        "rdf:type": "Journal Article",
        "dct:title": "A machine learning approach to radiogenomics of breast cancer: a study of 922 subjects and 529 DCE-MRI features.",
        "dct:bibliographicCitation": "Saha A, et al. A machine learning approach to radiogenomics of breast cancer: a study of 922 subjects and 529 DCE-MRI features. Br J Cancer",
        "prism:doi": "10.1038/s41416-018-0185-8",
        "fabio:hasPubMedId": "30033447",
        "foaf:homepage": "https://pubmed.ncbi.nlm.nih.gov/30033447",
        "dct:identifier": "30033447",
        "@context": {
          "dct": "http://purl.org/dc/terms/",
          "prism": "http://prismstandard.org/namespaces/basic/3.0/",
          "rdf": "http://www.w3.org/1999/02/22-rdf-syntax-ns#",
          "foaf": "http://xmlns.com/foaf/0.1/",
          "datmm": "http://schema.org/",
          "fabio": "http://purl.org/spar/fabio/"
        }
      }
    ],
    "dct:subject": [],
    "@context": {
      "dct": "http://purl.org/dc/terms/",
      "foaf": "http://xmlns.com/foaf/0.1/",
      "datmm": "http://schema.org/"
    }
  },
  {
    "@type": "datmm:Dataset",
    "dct:description": "Researchers will have the unique opportunity to visualize how head-and-neck squamous cell carcinoma (HNSCC) patients\u2019 3D CT image data changes with radiotherapy between pre-treatment, mid-treatment, and post-treatment. They will also have the advantage to receive additional information such as a) photon energy, b) number of arcs for volumetric modulated arc radiotherapy (VMAT) therapy, c) tumor volume and location, d) CT-to-density table, e) treatment related toxicities for parotid glands and oral cavity, f) patient age and weight, patient chemotherapy medication, g) prior surgery, h) performance status, i) histology, j) disease stage, k) number of targets, l) organs at risk, and m) other structures delineated on the CT image.",
    "dct:format": "Unknown",
    "dct:issued": "02-06-2019",
    "foaf:homepage": "https://www.ncbi.nlm.nih.gov/gap",
    "dct:title": "Head-and-neck squamous cell carcinoma patients with CT taken during pre-treatment, mid-treatment, and post-treatment (HNSCC-3DCT-RT)",
    "dct:language": "English",
    "bf:contribution": [],
    "dct:isPartOf": {
      "@type": "datmm:Repository",
      "dct:alternative": "TCIA",
      "foaf:homepage": "https://www.cancerimagingarchive.net",
      "dct:title": "The Cancer Imaging Archive",
      "@context": {
        "dct": "http://purl.org/dc/terms/",
        "foaf": "http://xmlns.com/foaf/0.1/",
        "datmm": "http://schema.org/"
      }
    },
    "frapo:isSupportedBy": [],
    "schema:distribution": [
      {
        "@type": "schema:DataDownload",
        "schema:contentSize": "14GB",
        "schema:encodingFormat": "DICOM",
        "schema:inLanguage": "en",
        "schema:name": "Images\u00a0and Radiation Therapy Structures ",
        "schema:url": "https://wiki.cancerimagingarchive.net/pages/viewpage.action?pageId=39879146/download/attachments/39879146/TCIA_HNSCC-3DCT-RT_v2_Jan2019.tcia?version=1&modificationDate=1549495845636&api=v2",
        "@context": {
          "schema": "http://schema.org/"
        }
      }
    ],
    "dct:isReferencedBy": [
      {
        "@type": "datmm:Documentation",
        "rdf:type": "Journal Article",
        "dct:title": "Longitudinal fan-beam computed tomography dataset for head-and-neck squamous cell carcinoma patients.",
        "dct:bibliographicCitation": "Bejarano T, et al. Longitudinal fan-beam computed tomography dataset for head-and-neck squamous cell carcinoma patients. Med Phys",
        "prism:doi": "10.1002/mp.13460",
        "fabio:hasPubMedId": "30806479",
        "foaf:homepage": "https://pubmed.ncbi.nlm.nih.gov/30806479",
        "dct:identifier": "30806479",
        "@context": {
          "dct": "http://purl.org/dc/terms/",
          "prism": "http://prismstandard.org/namespaces/basic/3.0/",
          "rdf": "http://www.w3.org/1999/02/22-rdf-syntax-ns#",
          "foaf": "http://xmlns.com/foaf/0.1/",
          "datmm": "http://schema.org/",
          "fabio": "http://purl.org/spar/fabio/"
        }
      }
    ],
    "dct:subject": [
      {
        "@type": "skos:Concept",
        "dct:identifier": "D014057",
        "skos:inScheme": "MeSH",
        "rdfs:label": "Tomography, X-Ray Computed",
        "@context": {
          "rdfs": "http://www.w3.org/2000/01/rdf-schema#",
          "skos": "http://www.w3.org/2004/02/skos/core#",
          "dct": "http://purl.org/dc/terms/"
        }
      }
    ],
    "@context": {
      "dct": "http://purl.org/dc/terms/",
      "foaf": "http://xmlns.com/foaf/0.1/",
      "datmm": "http://schema.org/"
    }
  },
  {
    "@type": "datmm:Dataset",
    "dct:description": "This collection combines advanced molecular imaging treatment response assessment through pre- and post-treatment FDG PET/CT scans with therapy of advanced head and neck cancer, including chemo-radiation therapy with and without addition of an EGFR inhibitor\u00a0molecular targeted agent (Cetuximab).\u00a0",
    "dct:format": "Unknown",
    "dct:issued": "2013/11/14",
    "foaf:homepage": "https://www.ncbi.nlm.nih.gov/gap",
    "dct:title": "Head-Neck Cetuximab",
    "dct:language": "English",
    "bf:contribution": [],
    "dct:isPartOf": {
      "@type": "datmm:Repository",
      "dct:alternative": "TCIA",
      "foaf:homepage": "https://www.cancerimagingarchive.net",
      "dct:title": "The Cancer Imaging Archive",
      "@context": {
        "dct": "http://purl.org/dc/terms/",
        "foaf": "http://xmlns.com/foaf/0.1/",
        "datmm": "http://schema.org/"
      }
    },
    "frapo:isSupportedBy": [],
    "schema:distribution": [
      {
        "@type": "schema:DataDownload",
        "schema:encodingFormat": "DICOM",
        "schema:inLanguage": "en",
        "schema:name": "DICOM Metadata Digest ",
        "schema:url": "https://wiki.cancerimagingarchive.net/display/Public/Head-Neck+Cetuximab/download/attachments/6884551/HeadNeckCetuximab_MetaData.csv?version=2&modificationDate=1495560309184&api=v2",
        "@context": {
          "schema": "http://schema.org/"
        }
      }
    ],
    "dct:isReferencedBy": [],
    "dct:subject": [],
    "@context": {
      "dct": "http://purl.org/dc/terms/",
      "foaf": "http://xmlns.com/foaf/0.1/",
      "datmm": "http://schema.org/"
    }
  },
  {
    "@type": "datmm:Dataset",
    "dct:description": "This collection contains FDG-PET/CT and radiotherapy planning CT imaging data of\u00a0",
    "dct:format": "Unknown",
    "dct:issued": "2018/06/07",
    "foaf:homepage": "https://www.ncbi.nlm.nih.gov/gap",
    "dct:title": "Head-Neck-PET-CT",
    "dct:language": "English",
    "bf:contribution": [],
    "dct:isPartOf": {
      "@type": "datmm:Repository",
      "dct:alternative": "TCIA",
      "foaf:homepage": "https://www.cancerimagingarchive.net",
      "dct:title": "The Cancer Imaging Archive",
      "@context": {
        "dct": "http://purl.org/dc/terms/",
        "foaf": "http://xmlns.com/foaf/0.1/",
        "datmm": "http://schema.org/"
      }
    },
    "frapo:isSupportedBy": [],
    "schema:distribution": [
      {
        "@type": "schema:DataDownload",
        "schema:contentSize": "72.5 GB",
        "schema:encodingFormat": "DICOM",
        "schema:inLanguage": "en",
        "schema:name": "Images\u00a0and Radiation Therapy Structures ",
        "schema:url": "https://wiki.cancerimagingarchive.net/display/Public/Head-Neck-PET-CT/download/attachments/24283867/Head-Neck-PET-CT-v2-doiJNLP-7hWXTIJS.tcia?version=1&modificationDate=1534787032596&api=v2",
        "@context": {
          "schema": "http://schema.org/"
        }
      }
    ],
    "dct:isReferencedBy": [
      {
        "@type": "datmm:Documentation",
        "rdf:type": "Journal Article",
        "dct:title": "Radiomics strategies for risk assessment of tumour failure in head-and-neck cancer.",
        "dct:bibliographicCitation": "Valli\u00e8res M, et al. Radiomics strategies for risk assessment of tumour failure in head-and-neck cancer. Sci Rep",
        "prism:doi": "10.1038/s41598-017-10371-5",
        "fabio:hasPubMedId": "28860628",
        "foaf:homepage": "https://pubmed.ncbi.nlm.nih.gov/28860628",
        "dct:identifier": "28860628",
        "@context": {
          "dct": "http://purl.org/dc/terms/",
          "prism": "http://prismstandard.org/namespaces/basic/3.0/",
          "rdf": "http://www.w3.org/1999/02/22-rdf-syntax-ns#",
          "foaf": "http://xmlns.com/foaf/0.1/",
          "datmm": "http://schema.org/",
          "fabio": "http://purl.org/spar/fabio/"
        }
      }
    ],
    "dct:subject": [],
    "@context": {
      "dct": "http://purl.org/dc/terms/",
      "foaf": "http://xmlns.com/foaf/0.1/",
      "datmm": "http://schema.org/"
    }
  },
  {
    "@type": "datmm:Dataset",
    "dct:description": "This collection contains clinical data and computed tomography (CT) from\u00a0137\u00a0head and neck squamous cell carcinoma (HNSCC) patients treated by radiotherapy. For these patients a pre-treatment CT scan was manual delineated by an experienced radiation oncologist of the 3D volume of the gross tumor volume.\u00a0This dataset refers to the \"H&N1\" dataset of the study published in Nature Communications (",
    "dct:format": "Unknown",
    "dct:issued": "2020/07/29",
    "foaf:homepage": "https://www.ncbi.nlm.nih.gov/gap",
    "dct:title": "Head-Neck-Radiomics-HN1",
    "dct:language": "English",
    "bf:contribution": [],
    "dct:isPartOf": {
      "@type": "datmm:Repository",
      "dct:alternative": "TCIA",
      "foaf:homepage": "https://www.cancerimagingarchive.net",
      "dct:title": "The Cancer Imaging Archive",
      "@context": {
        "dct": "http://purl.org/dc/terms/",
        "foaf": "http://xmlns.com/foaf/0.1/",
        "datmm": "http://schema.org/"
      }
    },
    "frapo:isSupportedBy": [],
    "schema:distribution": [
      {
        "@type": "schema:DataDownload",
        "schema:contentSize": "11.8 GB",
        "schema:encodingFormat": "DICOM",
        "schema:inLanguage": "en",
        "schema:name": "Images, Segmentations, and Radiation Therapy Structures\u00a0",
        "schema:url": "https://wiki.cancerimagingarchive.net/display/Public/Head-Neck-Radiomics-HN1/download/attachments/52762760/Head-Neck-Radiomics-HN1-Version%202-Sept%202019%20NBIA-manifest.tcia?version=1&modificationDate=1568995984096&api=v2",
        "@context": {
          "schema": "http://schema.org/"
        }
      }
    ],
    "dct:isReferencedBy": [],
    "dct:subject": [],
    "@context": {
      "dct": "http://purl.org/dc/terms/",
      "foaf": "http://xmlns.com/foaf/0.1/",
      "datmm": "http://schema.org/"
    }
  },
  {
    "@type": "datmm:Dataset",
    "dct:description": "We have used CODEX to image 56 proteins simultaneously in 140 tissue regions from the tumor invasive front of 35 advanced-stage colorectal cancer (CRC) patients (17 patients with Crohn's-like reaction (CLR) - leading to high amount of tertiary lymphoid structures (TLS); and 18 patients with diffuse inflammatory infiltration (DII) and no TLS). These patients were selected from an initial cohort of 715 CRC patients. Patients with low-stage CRC (pTNM 0-2), pre-operative chemotherapy, insufficient material, and low immune infiltration were excluded. The 35 resulting patients were matched for age, sex and tumor characteristics. CLR patients had a much better survival compared to DII patients.\u00a0 ",
    "dct:format": "Unknown",
    "dct:issued": "2020/08/05",
    "foaf:homepage": "https://www.ncbi.nlm.nih.gov/gap",
    "dct:title": "High-dimensional imaging of colorectal carcinoma and other tumors with 50+ markers (CRC_FFPE-CODEX_CellNeighs)",
    "dct:language": "English",
    "bf:contribution": [],
    "dct:isPartOf": {
      "@type": "datmm:Repository",
      "dct:alternative": "TCIA",
      "foaf:homepage": "https://www.cancerimagingarchive.net",
      "dct:title": "The Cancer Imaging Archive",
      "@context": {
        "dct": "http://purl.org/dc/terms/",
        "foaf": "http://xmlns.com/foaf/0.1/",
        "datmm": "http://schema.org/"
      }
    },
    "frapo:isSupportedBy": [],
    "schema:distribution": [],
    "dct:isReferencedBy": [
      {
        "@type": "datmm:Documentation",
        "rdf:type": "Journal Article",
        "dct:title": "Coordinated Cellular Neighborhoods Orchestrate Antitumoral Immunity at the Colorectal Cancer Invasive Front.",
        "dct:bibliographicCitation": "Sch\u00fcrch CM, et al. Coordinated Cellular Neighborhoods Orchestrate Antitumoral Immunity at the Colorectal Cancer Invasive Front. Cell",
        "prism:doi": "10.1016/j.cell.2020.07.005",
        "fabio:hasPubMedId": "32763154",
        "foaf:homepage": "https://pubmed.ncbi.nlm.nih.gov/32763154",
        "dct:identifier": "32763154",
        "@context": {
          "dct": "http://purl.org/dc/terms/",
          "prism": "http://prismstandard.org/namespaces/basic/3.0/",
          "rdf": "http://www.w3.org/1999/02/22-rdf-syntax-ns#",
          "foaf": "http://xmlns.com/foaf/0.1/",
          "datmm": "http://schema.org/",
          "fabio": "http://purl.org/spar/fabio/"
        }
      }
    ],
    "dct:subject": [],
    "@context": {
      "dct": "http://purl.org/dc/terms/",
      "foaf": "http://xmlns.com/foaf/0.1/",
      "datmm": "http://schema.org/"
    }
  },
  {
    "@type": "datmm:Dataset",
    "dct:description": "\n \n This collection contains imaging, radiation therapy, and clinical data from 627 head and neck squamous cell carcinoma (HNSCC) patients\u00a0",
    "dct:format": "Unknown",
    "dct:issued": "2020/03/31",
    "foaf:homepage": "https://www.ncbi.nlm.nih.gov/gap",
    "dct:title": "HNSCC",
    "dct:language": "English",
    "bf:contribution": [],
    "dct:isPartOf": {
      "@type": "datmm:Repository",
      "dct:alternative": "TCIA",
      "foaf:homepage": "https://www.cancerimagingarchive.net",
      "dct:title": "The Cancer Imaging Archive",
      "@context": {
        "dct": "http://purl.org/dc/terms/",
        "foaf": "http://xmlns.com/foaf/0.1/",
        "datmm": "http://schema.org/"
      }
    },
    "frapo:isSupportedBy": [],
    "schema:distribution": [
      {
        "@type": "schema:DataDownload",
        "schema:contentSize": "144 GB",
        "schema:encodingFormat": "DICOM",
        "schema:inLanguage": "en",
        "schema:name": "Images and Radiation Therapy Structures ",
        "schema:url": "https://wiki.cancerimagingarchive.net/display/Public/HNSCC/download/attachments/41518000/HNSCC.tcia?version=1&modificationDate=1588170765754&api=v2",
        "@context": {
          "schema": "http://schema.org/"
        }
      }
    ],
    "dct:isReferencedBy": [
      {
        "@type": "datmm:Documentation",
        "rdf:type": "Journal Article",
        "dct:title": "Imaging and clinical data archive for head and neck squamous cell carcinoma patients treated with radiotherapy.",
        "dct:bibliographicCitation": "Grossberg AJ, et al. Imaging and clinical data archive for head and neck squamous cell carcinoma patients treated with radiotherapy. Sci Data",
        "prism:doi": "10.1038/sdata.2018.173",
        "fabio:hasPubMedId": "30179230",
        "foaf:homepage": "https://pubmed.ncbi.nlm.nih.gov/30179230",
        "dct:identifier": "30179230",
        "@context": {
          "dct": "http://purl.org/dc/terms/",
          "prism": "http://prismstandard.org/namespaces/basic/3.0/",
          "rdf": "http://www.w3.org/1999/02/22-rdf-syntax-ns#",
          "foaf": "http://xmlns.com/foaf/0.1/",
          "datmm": "http://schema.org/",
          "fabio": "http://purl.org/spar/fabio/"
        }
      },
      {
        "@type": "datmm:Documentation",
        "rdf:type": "Journal Article",
        "dct:title": "Matched computed tomography segmentation and demographic data for oropharyngeal cancer radiomics challenges.",
        "dct:bibliographicCitation": ". Matched computed tomography segmentation and demographic data for oropharyngeal cancer radiomics challenges. Sci Data",
        "prism:doi": "10.1038/sdata.2017.77",
        "fabio:hasPubMedId": "28675381",
        "foaf:homepage": "https://pubmed.ncbi.nlm.nih.gov/28675381",
        "dct:identifier": "28675381",
        "@context": {
          "dct": "http://purl.org/dc/terms/",
          "prism": "http://prismstandard.org/namespaces/basic/3.0/",
          "rdf": "http://www.w3.org/1999/02/22-rdf-syntax-ns#",
          "foaf": "http://xmlns.com/foaf/0.1/",
          "datmm": "http://schema.org/",
          "fabio": "http://purl.org/spar/fabio/"
        }
      }
    ],
    "dct:subject": [
      {
        "@type": "skos:Concept",
        "dct:identifier": "D006258",
        "skos:inScheme": "MeSH",
        "rdfs:label": "Head and Neck Neoplasms",
        "@context": {
          "rdfs": "http://www.w3.org/2000/01/rdf-schema#",
          "skos": "http://www.w3.org/2004/02/skos/core#",
          "dct": "http://purl.org/dc/terms/"
        }
      },
      {
        "@type": "skos:Concept",
        "dct:identifier": "D000077195",
        "skos:inScheme": "MeSH",
        "rdfs:label": "Squamous Cell Carcinoma of Head and Neck",
        "@context": {
          "rdfs": "http://www.w3.org/2000/01/rdf-schema#",
          "skos": "http://www.w3.org/2004/02/skos/core#",
          "dct": "http://purl.org/dc/terms/"
        }
      },
      {
        "@type": "skos:Concept",
        "dct:identifier": "D009959",
        "skos:inScheme": "MeSH",
        "rdfs:label": "Oropharyngeal Neoplasms",
        "@context": {
          "rdfs": "http://www.w3.org/2000/01/rdf-schema#",
          "skos": "http://www.w3.org/2004/02/skos/core#",
          "dct": "http://purl.org/dc/terms/"
        }
      }
    ],
    "@context": {
      "dct": "http://purl.org/dc/terms/",
      "foaf": "http://xmlns.com/foaf/0.1/",
      "datmm": "http://schema.org/"
    }
  },
  {
    "@type": "datmm:Dataset",
    "dct:description": "Sporadic gliomas in companion dogs provide a window on the interaction between tumorigenic mechanisms and host environment. We compared the molecular profiles of canine gliomas with those of human pediatric and adult gliomas to characterize evolutionarily conserved mammalian mutational processes in gliomagenesis. Employing whole genome-, exome-, transcriptome- and methylation-sequencing of 81 canine gliomas, our cross-species comparative genomic analysis provides unique insights into glioma etiology and the chronology of glioma-causing somatic alterations, and rationalizes sporadic canine glioma as a preclinical model tailored to measuring treatment efficacies in patients with canine or human glioma. Here, we provide high-throughput multi-omics sequencing data in binary alignment map (BAM) format for the largest canine glioma cohort to date.",
    "dct:format": "Unknown",
    "dct:issued": "2020/12/18",
    "foaf:homepage": "https://www.ncbi.nlm.nih.gov/gap",
    "dct:title": "ICDC-Glioma01",
    "dct:language": "English",
    "bf:contribution": [],
    "dct:isPartOf": {
      "@type": "datmm:Repository",
      "dct:alternative": "TCIA",
      "foaf:homepage": "https://www.cancerimagingarchive.net",
      "dct:title": "The Cancer Imaging Archive",
      "@context": {
        "dct": "http://purl.org/dc/terms/",
        "foaf": "http://xmlns.com/foaf/0.1/",
        "datmm": "http://schema.org/"
      }
    },
    "frapo:isSupportedBy": [],
    "schema:distribution": [
      {
        "@type": "schema:DataDownload",
        "schema:contentSize": "5.1 GB",
        "schema:encodingFormat": "DICOM",
        "schema:inLanguage": "en",
        "schema:name": "Images ",
        "schema:url": "https://wiki.cancerimagingarchive.net/display/Public/ICDC-Glioma01/download/attachments/70227341/ICDC-Glioma.tcia?version=1&modificationDate=1609174648031&api=v2",
        "@context": {
          "schema": "http://schema.org/"
        }
      }
    ],
    "dct:isReferencedBy": [
      {
        "@type": "datmm:Documentation",
        "rdf:type": "Journal Article",
        "dct:title": "Comparative Molecular Life History of Spontaneous Canine and Human Gliomas.",
        "dct:bibliographicCitation": "Amin SB, et al. Comparative Molecular Life History of Spontaneous Canine and Human Gliomas. Cancer Cell",
        "prism:doi": "10.1016/j.ccell.2020.01.004",
        "fabio:hasPubMedId": "32049048",
        "foaf:homepage": "https://pubmed.ncbi.nlm.nih.gov/32049048",
        "dct:identifier": "32049048",
        "@context": {
          "dct": "http://purl.org/dc/terms/",
          "prism": "http://prismstandard.org/namespaces/basic/3.0/",
          "rdf": "http://www.w3.org/1999/02/22-rdf-syntax-ns#",
          "foaf": "http://xmlns.com/foaf/0.1/",
          "datmm": "http://schema.org/",
          "fabio": "http://purl.org/spar/fabio/"
        }
      }
    ],
    "dct:subject": [],
    "@context": {
      "dct": "http://purl.org/dc/terms/",
      "foaf": "http://xmlns.com/foaf/0.1/",
      "datmm": "http://schema.org/"
    }
  },
  {
    "@type": "datmm:Dataset",
    "dct:description": "Pre-clinical animal models of spontaneous metastatic cancer are infrequent; the few that exist\u00a0are resource intensive because determination of the presence of metastatic disease,\u00a0metastatic burden, and response to therapy normally require multiple timed cohorts with animal sacrifice and extensive\u00a0pathological examination. We identified and characterized a patient derived xenograft\u00a0model with metastatic potential, adenocarcinoma colon xenograft 997537-175-T. In this study we performed a detailed\u00a0imaging characterization (workflow below) of this model, which develops spontaneous lung metastases, details are provided in the attached standard operating procedures. Tumors in half of the mice were resected in the range 200-300 cm",
    "dct:format": "Unknown",
    "dct:issued": "2020/05/22",
    "foaf:homepage": "https://www.ncbi.nlm.nih.gov/gap",
    "dct:title": "Imaging characterization of a metastatic patient derived model of adenocarcinoma colon: PDMR-997537-175-T",
    "dct:language": "English",
    "bf:contribution": [],
    "dct:isPartOf": {
      "@type": "datmm:Repository",
      "dct:alternative": "TCIA",
      "foaf:homepage": "https://www.cancerimagingarchive.net",
      "dct:title": "The Cancer Imaging Archive",
      "@context": {
        "dct": "http://purl.org/dc/terms/",
        "foaf": "http://xmlns.com/foaf/0.1/",
        "datmm": "http://schema.org/"
      }
    },
    "frapo:isSupportedBy": [],
    "schema:distribution": [
      {
        "@type": "schema:DataDownload",
        "schema:contentSize": "2.3 GB",
        "schema:encodingFormat": "DICOM",
        "schema:inLanguage": "en",
        "schema:name": "Images ",
        "schema:url": "https://wiki.cancerimagingarchive.net/display/Public/Imaging+characterization+of+a+metastatic+patient+derived+model+of+adenocarcinoma+colon%3A+PDMR-997537-175-T/download/attachments/70225394/PDMR-997537-175-T.tcia?version=1&modificationDate=1590008255458&api=v2",
        "@context": {
          "schema": "http://schema.org/"
        }
      }
    ],
    "dct:isReferencedBy": [],
    "dct:subject": [],
    "@context": {
      "dct": "http://purl.org/dc/terms/",
      "foaf": "http://xmlns.com/foaf/0.1/",
      "datmm": "http://schema.org/"
    }
  },
  {
    "@type": "datmm:Dataset",
    "dct:description": "Pre-clinical animal models of spontaneous metastatic cancer are infrequent; the few that exist\u00a0are resource intensive because determination of the presence of metastatic disease,\u00a0metastatic burden, and response to therapy normally require multiple timed cohorts with animal sacrifice and extensive\u00a0pathological examination. We identified and characterized a patient derived xenograft\u00a0model with metastatic potential, adenocarcinoma pancreas xenograft 292921-168-R. In this study we performed a detailed\u00a0imaging characterization (workflow below) of this model, which develops spontaneous lung metastases, details are provided in the attached standard operating procedures. Tumors in half of the mice were resected in the range 200-300 cm",
    "dct:format": "Unknown",
    "dct:issued": "2020/03/23",
    "foaf:homepage": "https://www.ncbi.nlm.nih.gov/gap",
    "dct:title": "Imaging characterization of a metastatic patient derived model of adenocarcinoma pancreas: PDMR-292921-168-R",
    "dct:language": "English",
    "bf:contribution": [],
    "dct:isPartOf": {
      "@type": "datmm:Repository",
      "dct:alternative": "TCIA",
      "foaf:homepage": "https://www.cancerimagingarchive.net",
      "dct:title": "The Cancer Imaging Archive",
      "@context": {
        "dct": "http://purl.org/dc/terms/",
        "foaf": "http://xmlns.com/foaf/0.1/",
        "datmm": "http://schema.org/"
      }
    },
    "frapo:isSupportedBy": [],
    "schema:distribution": [
      {
        "@type": "schema:DataDownload",
        "schema:contentSize": "1.6 GB",
        "schema:encodingFormat": "DICOM",
        "schema:inLanguage": "en",
        "schema:name": "Images ",
        "schema:url": "https://wiki.cancerimagingarchive.net/display/Public/Imaging+characterization+of+a+metastatic+patient+derived+model+of+adenocarcinoma+pancreas%3A+PDMR-292921-168-R/download/attachments/61080585/PDMR-292921-168-R.tcia?version=1&modificationDate=1584982370329&api=v2",
        "@context": {
          "schema": "http://schema.org/"
        }
      }
    ],
    "dct:isReferencedBy": [],
    "dct:subject": [],
    "@context": {
      "dct": "http://purl.org/dc/terms/",
      "foaf": "http://xmlns.com/foaf/0.1/",
      "datmm": "http://schema.org/"
    }
  },
  {
    "@type": "datmm:Dataset",
    "dct:description": "\n \n \n \n \n Pre-clinical animal models of spontaneous metastatic cancer are infrequent; the few that exist\u00a0are resource intensive because determination of the presence of metastatic disease,\u00a0metastatic burden, and response to therapy normally require animal sacrifice and extensive\u00a0pathological examination. We recently identified and characterized a patient derived xenograft\u00a0model with metastatic potential, bladder xenograft BL0293-F563, developed by Jackson\u00a0Laboratories and the University of California at Davis. In this study we performed a detailed\u00a0imaging characterization of this model, which develops spontaneous liver and bone\u00a0metastases. Using non-contrast T2 weighted MRI, hepatic metastases were demonstrated in\u00a0over 70% of animals at 52 days post tumor implantation without resection of the xenograft and\u00a0in 100% of animals at day 52 following resection of the xenograft. T2w turbo spin echo (T2wTSE) sequence was applied in the coronal view with a repetition time (TR) 5333ms, echo time\u00a0(TE) 65ms, with an in-plane pixel of 0.180 \u00d7 0.180 mm2. A Spectral Presaturation with\u00a0Inversion Recovery (SPIR) sequence (Philips Healthcare, Best, The Netherlands) was used to\u00a0suppress the fat component and assist in distinguishing fat from cystic mass and tumor\u00a0tissue. In a group of animals receiving one cycle of effective chemotherapy ([Temozolomide;\u00a0(50 mg/kg; PO, QDx5)] plus [(veliparib, a poly (ADP-ribose) polymerase inhibitor) (7.75 mg/kg;\u00a0PO; BIDx7)]), no animals demonstrated metastasis by imaging. The imaging characteristics of\u00a0this model, which is available from the National Cancer Institute Patient-Derived Models\u00a0Repository (",
    "dct:format": "Unknown",
    "dct:issued": "2019/08/28",
    "foaf:homepage": "https://www.ncbi.nlm.nih.gov/gap",
    "dct:title": "Imaging characterization of a metastatic patient derived model of bladder cancer: BL0293F (PDMR-BL0293-F563)",
    "dct:language": "English",
    "bf:contribution": [],
    "dct:isPartOf": {
      "@type": "datmm:Repository",
      "dct:alternative": "TCIA",
      "foaf:homepage": "https://www.cancerimagingarchive.net",
      "dct:title": "The Cancer Imaging Archive",
      "@context": {
        "dct": "http://purl.org/dc/terms/",
        "foaf": "http://xmlns.com/foaf/0.1/",
        "datmm": "http://schema.org/"
      }
    },
    "frapo:isSupportedBy": [],
    "schema:distribution": [
      {
        "@type": "schema:DataDownload",
        "schema:contentSize": "3.2 GB",
        "schema:encodingFormat": "DICOM",
        "schema:inLanguage": "en",
        "schema:name": "Images ",
        "schema:url": "https://wiki.cancerimagingarchive.net/pages/viewpage.action?pageId=52757379/download/attachments/52757379/PDMR-BL0293-F563-manifest-08282019.tcia?version=1&modificationDate=1567010278936&api=v2",
        "@context": {
          "schema": "http://schema.org/"
        }
      }
    ],
    "dct:isReferencedBy": [
      {
        "@type": "datmm:Documentation",
        "rdf:type": "Journal Article",
        "dct:title": "A spontaneously metastatic model of bladder cancer: imaging characterization.",
        "dct:bibliographicCitation": "Tatum JL, et al. A spontaneously metastatic model of bladder cancer: imaging characterization. J Transl Med",
        "prism:doi": "10.1186/s12967-019-02177-y",
        "fabio:hasPubMedId": "31878948",
        "foaf:homepage": "https://pubmed.ncbi.nlm.nih.gov/31878948",
        "dct:identifier": "31878948",
        "@context": {
          "dct": "http://purl.org/dc/terms/",
          "prism": "http://prismstandard.org/namespaces/basic/3.0/",
          "rdf": "http://www.w3.org/1999/02/22-rdf-syntax-ns#",
          "foaf": "http://xmlns.com/foaf/0.1/",
          "datmm": "http://schema.org/",
          "fabio": "http://purl.org/spar/fabio/"
        }
      }
    ],
    "dct:subject": [
      {
        "@type": "skos:Concept",
        "dct:identifier": "D021621",
        "skos:inScheme": "MeSH",
        "rdfs:label": "Imaging, Three-Dimensional",
        "@context": {
          "rdfs": "http://www.w3.org/2000/01/rdf-schema#",
          "skos": "http://www.w3.org/2004/02/skos/core#",
          "dct": "http://purl.org/dc/terms/"
        }
      }
    ],
    "@context": {
      "dct": "http://purl.org/dc/terms/",
      "foaf": "http://xmlns.com/foaf/0.1/",
      "datmm": "http://schema.org/"
    }
  },
  {
    "@type": "datmm:Dataset",
    "dct:description": "Pre-clinical animal models of spontaneous metastatic cancer are infrequent; the few that exist\u00a0are resource intensive because determination of the presence of metastatic disease,\u00a0metastatic burden, and response to therapy normally require multiple timed cohorts with animal sacrifice and extensive\u00a0pathological examination. We identified and characterized a patient derived xenograft\u00a0model with metastatic potential, melanoma xenograft 425362-245-T. In this study we performed a detailed\u00a0imaging characterization (workflow below) of this model, which develops spontaneous lung metastases, details are provided in the attached standard operating procedures. Tumors in half of the mice were resected in the range 200-300 cm",
    "dct:format": "Unknown",
    "dct:issued": "2021/02/17",
    "foaf:homepage": "https://www.ncbi.nlm.nih.gov/gap",
    "dct:title": "Imaging characterization of a metastatic patient derived model of melanoma: PDMR-425362-245-T",
    "dct:language": "English",
    "bf:contribution": [],
    "dct:isPartOf": {
      "@type": "datmm:Repository",
      "dct:alternative": "TCIA",
      "foaf:homepage": "https://www.cancerimagingarchive.net",
      "dct:title": "The Cancer Imaging Archive",
      "@context": {
        "dct": "http://purl.org/dc/terms/",
        "foaf": "http://xmlns.com/foaf/0.1/",
        "datmm": "http://schema.org/"
      }
    },
    "frapo:isSupportedBy": [],
    "schema:distribution": [
      {
        "@type": "schema:DataDownload",
        "schema:contentSize": "2.3 GB",
        "schema:encodingFormat": "DICOM",
        "schema:inLanguage": "en",
        "schema:name": "Images ",
        "schema:url": "https://wiki.cancerimagingarchive.net/display/Public/Imaging+characterization+of+a+metastatic+patient+derived+model+of+melanoma%3A+PDMR-425362-245-T/download/attachments/70223880/PDMR-425362-245-T.tcia?version=1&modificationDate=1587751871622&api=v2",
        "@context": {
          "schema": "http://schema.org/"
        }
      }
    ],
    "dct:isReferencedBy": [],
    "dct:subject": [],
    "@context": {
      "dct": "http://purl.org/dc/terms/",
      "foaf": "http://xmlns.com/foaf/0.1/",
      "datmm": "http://schema.org/"
    }
  },
  {
    "@type": "datmm:Dataset",
    "dct:description": "Characterization of tissue using  in vivo  non-invasive imaging is the foundation of Radiology and is clinically used for detection and measurement of disease burden in oncology.\u00a0 With the migration of imaging to digital media the possibility for advanced mathematically based imaging biomarkers was realized. As part of this endeavor, researchers have developed various algorithms using neural networks, and classification techniques to improve tissue characterization (morphological changes).\u00a0 However, large datasets are a requirement in this research endeavor in part due to the genomic heterogeneity of tumors in the same histologic classification \u2013 many tumors from different patients are required to have enough with the same genomic characteristics to adequately evaluate the range of imaging variability for a specific genomic pattern.\u00a0 Pre-clinical animal models of patient derived xenografts may be an important resource by providing collections with a more homogenous tumor genome across the collection with companion extensive tumor genomic characterization available, allowing determination of the variability of imaging characteristics for that pattern in different individuals. This dataset of a patient derived xenograft\u00a0model adenocarcinoma pancreas ",
    "dct:format": "Unknown",
    "dct:issued": "2020/10/05",
    "foaf:homepage": "https://www.ncbi.nlm.nih.gov/gap",
    "dct:title": "Imaging tissue characterization of a patient derived xenograft model of adenocarcinoma pancreas: PDMR-833975-119-R",
    "dct:language": "English",
    "bf:contribution": [],
    "dct:isPartOf": {
      "@type": "datmm:Repository",
      "dct:alternative": "TCIA",
      "foaf:homepage": "https://www.cancerimagingarchive.net",
      "dct:title": "The Cancer Imaging Archive",
      "@context": {
        "dct": "http://purl.org/dc/terms/",
        "foaf": "http://xmlns.com/foaf/0.1/",
        "datmm": "http://schema.org/"
      }
    },
    "frapo:isSupportedBy": [],
    "schema:distribution": [
      {
        "@type": "schema:DataDownload",
        "schema:contentSize": "1.6 GB",
        "schema:encodingFormat": "DICOM",
        "schema:inLanguage": "en",
        "schema:name": "Images ",
        "schema:url": "https://wiki.cancerimagingarchive.net/display/Public/Imaging+tissue+characterization+of+a+patient+derived+xenograft+model+of+adenocarcinoma+pancreas%3A+PDMR-833975-119-R/download/attachments/70226465/PDMR-833975-119-R-NCI.tcia?version=1&modificationDate=1602877832091&api=v2",
        "@context": {
          "schema": "http://schema.org/"
        }
      }
    ],
    "dct:isReferencedBy": [],
    "dct:subject": [],
    "@context": {
      "dct": "http://purl.org/dc/terms/",
      "foaf": "http://xmlns.com/foaf/0.1/",
      "datmm": "http://schema.org/"
    }
  },
  {
    "@type": "datmm:Dataset",
    "dct:description": "    ACRIN 6657      was designed as a prospective study to test MRI for ability to predict response to treatment and risk-of-recurrence in patients with stage 2 or 3 breast cancer receiving neoadjuvant chemotherapy (NACT). ",
    "dct:format": "Unknown",
    "dct:issued": "2016/09/28",
    "foaf:homepage": "https://www.ncbi.nlm.nih.gov/gap",
    "dct:title": "ISPY1",
    "dct:language": "English",
    "bf:contribution": [],
    "dct:isPartOf": {
      "@type": "datmm:Repository",
      "dct:alternative": "TCIA",
      "foaf:homepage": "https://www.cancerimagingarchive.net",
      "dct:title": "The Cancer Imaging Archive",
      "@context": {
        "dct": "http://purl.org/dc/terms/",
        "foaf": "http://xmlns.com/foaf/0.1/",
        "datmm": "http://schema.org/"
      }
    },
    "frapo:isSupportedBy": [],
    "schema:distribution": [
      {
        "@type": "schema:DataDownload",
        "schema:contentSize": "76.2GB",
        "schema:encodingFormat": "DICOM",
        "schema:inLanguage": "en",
        "schema:name": "Images and Segmentations\u00a0",
        "schema:url": "https://wiki.cancerimagingarchive.net/display/Public/ISPY1/download/attachments/20643859/doiJNLP-ISPY1-full-09-26-2016.tcia?version=1&modificationDate=1534787010468&api=v2",
        "@context": {
          "schema": "http://schema.org/"
        }
      },
      {
        "@type": "schema:DataDownload",
        "schema:encodingFormat": "DICOM",
        "schema:inLanguage": "en",
        "schema:name": "DICOM Metadata Digest ",
        "schema:url": "https://wiki.cancerimagingarchive.net/display/Public/ISPY1/download/attachments/20643859/ISPY1_MetaData.csv?version=1&modificationDate=1495728168666&api=v2",
        "@context": {
          "schema": "http://schema.org/"
        }
      }
    ],
    "dct:isReferencedBy": [
      {
        "@type": "datmm:Documentation",
        "rdf:type": "Journal Article",
        "dct:title": "Neoadjuvant Chemotherapy for Breast Cancer: Functional Tumor Volume by MR Imaging Predicts Recurrence-free Survival-Results from the ACRIN 6657/CALGB 150007 I-SPY 1 TRIAL.",
        "dct:bibliographicCitation": "Hylton NM, et al. Neoadjuvant Chemotherapy for Breast Cancer: Functional Tumor Volume by MR Imaging Predicts Recurrence-free Survival-Results from the ACRIN 6657/CALGB 150007 I-SPY 1 TRIAL. Radiology",
        "prism:doi": "10.1148/radiol.2015150013",
        "fabio:hasPubMedId": "26624971",
        "foaf:homepage": "https://pubmed.ncbi.nlm.nih.gov/26624971",
        "dct:identifier": "26624971",
        "@context": {
          "dct": "http://purl.org/dc/terms/",
          "prism": "http://prismstandard.org/namespaces/basic/3.0/",
          "rdf": "http://www.w3.org/1999/02/22-rdf-syntax-ns#",
          "foaf": "http://xmlns.com/foaf/0.1/",
          "datmm": "http://schema.org/",
          "fabio": "http://purl.org/spar/fabio/"
        }
      }
    ],
    "dct:subject": [],
    "@context": {
      "dct": "http://purl.org/dc/terms/",
      "foaf": "http://xmlns.com/foaf/0.1/",
      "datmm": "http://schema.org/"
    }
  },
  {
    "@type": "datmm:Dataset",
    "dct:description": "This data collection consists of MRI/CT scan data for brain tumor patients that form the cohort for the resource Ivy Glioblastoma Atlas Project (Ivy GAP). There are 390 studies for 39 patients that include pre-surgery, post-surgery and follow up scans. The Ivy GAP is a collaborative partnership between the ",
    "dct:format": "Unknown",
    "dct:issued": "2016/12/30",
    "foaf:homepage": "https://www.ncbi.nlm.nih.gov/gap",
    "dct:title": "Ivy Glioblastoma Atlas Project (Ivy GAP)",
    "dct:language": "English",
    "bf:contribution": [],
    "dct:isPartOf": {
      "@type": "datmm:Repository",
      "dct:alternative": "TCIA",
      "foaf:homepage": "https://www.cancerimagingarchive.net",
      "dct:title": "The Cancer Imaging Archive",
      "@context": {
        "dct": "http://purl.org/dc/terms/",
        "foaf": "http://xmlns.com/foaf/0.1/",
        "datmm": "http://schema.org/"
      }
    },
    "frapo:isSupportedBy": [],
    "schema:distribution": [],
    "dct:isReferencedBy": [
      {
        "@type": "datmm:Documentation",
        "rdf:type": "Journal Article",
        "dct:title": "An anatomic transcriptional atlas of human glioblastoma.",
        "dct:bibliographicCitation": "Puchalski RB, et al. An anatomic transcriptional atlas of human glioblastoma. Science",
        "prism:doi": "10.1126/science.aaf2666",
        "fabio:hasPubMedId": "29748285",
        "foaf:homepage": "https://pubmed.ncbi.nlm.nih.gov/29748285",
        "dct:identifier": "29748285",
        "@context": {
          "dct": "http://purl.org/dc/terms/",
          "prism": "http://prismstandard.org/namespaces/basic/3.0/",
          "rdf": "http://www.w3.org/1999/02/22-rdf-syntax-ns#",
          "foaf": "http://xmlns.com/foaf/0.1/",
          "datmm": "http://schema.org/",
          "fabio": "http://purl.org/spar/fabio/"
        }
      }
    ],
    "dct:subject": [],
    "@context": {
      "dct": "http://purl.org/dc/terms/",
      "foaf": "http://xmlns.com/foaf/0.1/",
      "datmm": "http://schema.org/"
    }
  },
  {
    "@type": "datmm:Dataset",
    "dct:description": "These MRIs are pre-operative examinations performed in 159 subjects with Low Grade Gliomas (WHO grade II & III). Segmentation of tumors in three axial slices that include the one with the largest tumor\u00a0diameter and ones below and above are provided in NiFTI format.\u00a0\u00a0Tumor grade and histologic type are also available.\u00a0\u00a0All of these subjects have biopsy proven 1p/19q results, performed using FISH.\u00a0\u00a0For the 1p/19q status \"n/n\" means neither 1p nor 19q were deleted. \"d/d\" means 1p and 19q are co-deleted.\u00a0",
    "dct:format": "Unknown",
    "dct:issued": "6/26/2020",
    "foaf:homepage": "https://www.ncbi.nlm.nih.gov/gap",
    "dct:title": "LGG-1p19qDeletion",
    "dct:language": "English",
    "bf:contribution": [],
    "dct:isPartOf": {
      "@type": "datmm:Repository",
      "dct:alternative": "TCIA",
      "foaf:homepage": "https://www.cancerimagingarchive.net",
      "dct:title": "The Cancer Imaging Archive",
      "@context": {
        "dct": "http://purl.org/dc/terms/",
        "foaf": "http://xmlns.com/foaf/0.1/",
        "datmm": "http://schema.org/"
      }
    },
    "frapo:isSupportedBy": [],
    "schema:distribution": [
      {
        "@type": "schema:DataDownload",
        "schema:encodingFormat": "DICOM",
        "schema:inLanguage": "en",
        "schema:name": "Segmentations only ",
        "schema:url": "https://wiki.cancerimagingarchive.net/display/Public/LGG-1p19qDeletion/download/attachments/25789042/LGG-1p19qDeletion_v2_SEGonly_Jun2020.tcia?version=1&modificationDate=1593205562927&api=v2",
        "@context": {
          "schema": "http://schema.org/"
        }
      }
    ],
    "dct:isReferencedBy": [
      {
        "@type": "datmm:Documentation",
        "rdf:type": "Journal Article",
        "dct:title": "Predicting Deletion of Chromosomal Arms 1p/19q in Low-Grade Gliomas from MR Images Using Machine Intelligence.",
        "dct:bibliographicCitation": "Akkus Z, et al. Predicting Deletion of Chromosomal Arms 1p/19q in Low-Grade Gliomas from MR Images Using Machine Intelligence. J Digit Imaging",
        "prism:doi": "10.1007/s10278-017-9984-3",
        "fabio:hasPubMedId": "28600641",
        "foaf:homepage": "https://pubmed.ncbi.nlm.nih.gov/28600641",
        "dct:identifier": "28600641",
        "@context": {
          "dct": "http://purl.org/dc/terms/",
          "prism": "http://prismstandard.org/namespaces/basic/3.0/",
          "rdf": "http://www.w3.org/1999/02/22-rdf-syntax-ns#",
          "foaf": "http://xmlns.com/foaf/0.1/",
          "datmm": "http://schema.org/",
          "fabio": "http://purl.org/spar/fabio/"
        }
      }
    ],
    "dct:subject": [
      {
        "@type": "skos:Concept",
        "dct:identifier": "D001185",
        "skos:inScheme": "MeSH",
        "rdfs:label": "Artificial Intelligence",
        "@context": {
          "rdfs": "http://www.w3.org/2000/01/rdf-schema#",
          "skos": "http://www.w3.org/2004/02/skos/core#",
          "dct": "http://purl.org/dc/terms/"
        }
      },
      {
        "@type": "skos:Concept",
        "dct:identifier": "D002872",
        "skos:inScheme": "MeSH",
        "rdfs:label": "Chromosome Deletion",
        "@context": {
          "rdfs": "http://www.w3.org/2000/01/rdf-schema#",
          "skos": "http://www.w3.org/2004/02/skos/core#",
          "dct": "http://purl.org/dc/terms/"
        }
      },
      {
        "@type": "skos:Concept",
        "dct:identifier": "D002878",
        "skos:inScheme": "MeSH",
        "rdfs:label": "Chromosomes, Human, Pair 1",
        "@context": {
          "rdfs": "http://www.w3.org/2000/01/rdf-schema#",
          "skos": "http://www.w3.org/2004/02/skos/core#",
          "dct": "http://purl.org/dc/terms/"
        }
      },
      {
        "@type": "skos:Concept",
        "dct:identifier": "D002888",
        "skos:inScheme": "MeSH",
        "rdfs:label": "Chromosomes, Human, Pair 19",
        "@context": {
          "rdfs": "http://www.w3.org/2000/01/rdf-schema#",
          "skos": "http://www.w3.org/2004/02/skos/core#",
          "dct": "http://purl.org/dc/terms/"
        }
      }
    ],
    "@context": {
      "dct": "http://purl.org/dc/terms/",
      "foaf": "http://xmlns.com/foaf/0.1/",
      "datmm": "http://schema.org/"
    }
  },
  {
    "@type": "datmm:Dataset",
    "dct:description": "The Lung Image Database Consortium image collection (LIDC-IDRI) consists of diagnostic and lung cancer screening thoracic computed tomography (CT) scans with marked-up annotated lesions. It is a web-accessible international resource for development, training, and evaluation of computer-assisted diagnostic (CAD) methods for lung cancer detection and diagnosis. Initiated by the National Cancer Institute (NCI), further advanced by the Foundation for the National Institutes of Health (FNIH), and accompanied by the Food and Drug Administration (FDA) through active participation, this public-private partnership demonstrates the success of a consortium founded on a consensus-based process.",
    "dct:format": "Unknown",
    "dct:issued": "2020/09/21",
    "foaf:homepage": "https://www.ncbi.nlm.nih.gov/gap",
    "dct:title": "LIDC-IDRI",
    "dct:language": "English",
    "bf:contribution": [],
    "dct:isPartOf": {
      "@type": "datmm:Repository",
      "dct:alternative": "TCIA",
      "foaf:homepage": "https://www.cancerimagingarchive.net",
      "dct:title": "The Cancer Imaging Archive",
      "@context": {
        "dct": "http://purl.org/dc/terms/",
        "foaf": "http://xmlns.com/foaf/0.1/",
        "datmm": "http://schema.org/"
      }
    },
    "frapo:isSupportedBy": [],
    "schema:distribution": [
      {
        "@type": "schema:DataDownload",
        "schema:contentSize": "125GB",
        "schema:encodingFormat": "DICOM",
        "schema:inLanguage": "en",
        "schema:name": "Images ",
        "schema:url": "https://wiki.cancerimagingarchive.net/display/Public/LIDC-IDRI/download/attachments/1966254/TCIA_LIDC-IDRI_20200921.tcia?version=1&modificationDate=1600709265077&api=v2",
        "@context": {
          "schema": "http://schema.org/"
        }
      },
      {
        "@type": "schema:DataDownload",
        "schema:encodingFormat": "DICOM",
        "schema:inLanguage": "en",
        "schema:name": "DICOM Metadata Digest ",
        "schema:url": "https://wiki.cancerimagingarchive.net/display/Public/LIDC-IDRI/download/attachments/1966254/LIDC-IDRI_MetaData.csv?version=2&modificationDate=1600709332036&api=v2",
        "@context": {
          "schema": "http://schema.org/"
        }
      }
    ],
    "dct:isReferencedBy": [
      {
        "@type": "datmm:Documentation",
        "rdf:type": "Journal Article",
        "dct:title": "The Lung Image Database Consortium (LIDC) and Image Database Resource Initiative (IDRI): a completed reference database of lung nodules on CT scans.",
        "dct:bibliographicCitation": "Armato SG 3rd, et al. The Lung Image Database Consortium (LIDC) and Image Database Resource Initiative (IDRI): a completed reference database of lung nodules on CT scans. Med Phys",
        "prism:doi": "10.1118/1.3528204",
        "fabio:hasPubMedId": "21452728",
        "foaf:homepage": "https://pubmed.ncbi.nlm.nih.gov/21452728",
        "dct:identifier": "21452728",
        "@context": {
          "dct": "http://purl.org/dc/terms/",
          "prism": "http://prismstandard.org/namespaces/basic/3.0/",
          "rdf": "http://www.w3.org/1999/02/22-rdf-syntax-ns#",
          "foaf": "http://xmlns.com/foaf/0.1/",
          "datmm": "http://schema.org/",
          "fabio": "http://purl.org/spar/fabio/"
        }
      }
    ],
    "dct:subject": [
      {
        "@type": "skos:Concept",
        "dct:identifier": "D016208",
        "skos:inScheme": "MeSH",
        "rdfs:label": "Databases, Factual",
        "@context": {
          "rdfs": "http://www.w3.org/2000/01/rdf-schema#",
          "skos": "http://www.w3.org/2004/02/skos/core#",
          "dct": "http://purl.org/dc/terms/"
        }
      }
    ],
    "@context": {
      "dct": "http://purl.org/dc/terms/",
      "foaf": "http://xmlns.com/foaf/0.1/",
      "datmm": "http://schema.org/"
    }
  },
  {
    "@type": "datmm:Dataset",
    "dct:description": "Investigators at the Mayo Clinic, with funding from the National Institute of Biomedical Imaging and Bioengineering (EB 017095 and EB 017185), have built a library of CT patient projection data in an open and vendor-neutral format. This format, referred to as DICOM-CT-PD (1), is an extended DICOM format that contains CT projection data and acquisition geometry. The de-identified patient projection data in the library were decoded with help of the manufacturer and have been converted into an open standardized format.",
    "dct:format": "Unknown",
    "dct:issued": "2020/08/11",
    "foaf:homepage": "https://www.ncbi.nlm.nih.gov/gap",
    "dct:title": "Low Dose CT Image and Projection Data (LDCT-and-Projection-data)",
    "dct:language": "English",
    "bf:contribution": [],
    "dct:isPartOf": {
      "@type": "datmm:Repository",
      "dct:alternative": "TCIA",
      "foaf:homepage": "https://www.cancerimagingarchive.net",
      "dct:title": "The Cancer Imaging Archive",
      "@context": {
        "dct": "http://purl.org/dc/terms/",
        "foaf": "http://xmlns.com/foaf/0.1/",
        "datmm": "http://schema.org/"
      }
    },
    "frapo:isSupportedBy": [],
    "schema:distribution": [
      {
        "@type": "schema:DataDownload",
        "schema:contentSize": "952 GB",
        "schema:encodingFormat": "DICOM",
        "schema:inLanguage": "en",
        "schema:name": "Images ",
        "schema:url": "https://wiki.cancerimagingarchive.net/pages/viewpage.action?pageId=52758026/download/attachments/52758026/LDCT-and-Projection-data%20NBIA%20manifest%20August%202020.tcia?version=1&modificationDate=1597183142100&api=v2",
        "@context": {
          "schema": "http://schema.org/"
        }
      },
      {
        "@type": "schema:DataDownload",
        "schema:contentSize": "2.0 GB",
        "schema:encodingFormat": "DICOM",
        "schema:inLanguage": "en",
        "schema:name": "Images ",
        "schema:url": "https://wiki.cancerimagingarchive.net/pages/viewpage.action?pageId=52758026/download/attachments/52758026/LDCT-and-Projection-data-Phantom%20April%206%202020.tcia?version=1&modificationDate=1586191054091&api=v2",
        "@context": {
          "schema": "http://schema.org/"
        }
      },
      {
        "@type": "schema:DataDownload",
        "schema:encodingFormat": "DICOM",
        "schema:inLanguage": "en",
        "schema:name": "DICOM-CT-PD User Manual Version 3 ",
        "schema:url": "https://wiki.cancerimagingarchive.net/pages/viewpage.action?pageId=52758026/download/attachments/52758026/DICOM-CT-PD%20User%20Manual_Version%203.pdf?version=1&modificationDate=1586187875073&api=v2",
        "@context": {
          "schema": "http://schema.org/"
        }
      },
      {
        "@type": "schema:DataDownload",
        "schema:encodingFormat": "DICOM",
        "schema:inLanguage": "en",
        "schema:name": "Matlab DICOM-CTPD data dictionary ",
        "schema:url": "https://wiki.cancerimagingarchive.net/pages/viewpage.action?pageId=52758026/download/attachments/52758026/DICOM-CT-PD-dict_v10%20Matlab%20DICOM-CTPD%20data%20dict.txt?version=1&modificationDate=1573149224372&api=v2",
        "@context": {
          "schema": "http://schema.org/"
        }
      },
      {
        "@type": "schema:DataDownload",
        "schema:encodingFormat": "DICOM",
        "schema:inLanguage": "en",
        "schema:name": "Matlab DICOM-CTPD reader script ",
        "schema:url": "https://wiki.cancerimagingarchive.net/pages/viewpage.action?pageId=52758026/download/attachments/52758026/DICOMCTPDreader%20Matlab%20DICOM-CTPD%20reader%20script.m?version=1&modificationDate=1573149470905&api=v2",
        "@context": {
          "schema": "http://schema.org/"
        }
      }
    ],
    "dct:isReferencedBy": [
      {
        "@type": "datmm:Documentation",
        "rdf:type": "Journal Article",
        "dct:title": "Low-dose CT image and projection dataset.",
        "dct:bibliographicCitation": "Moen TR, et al. Low-dose CT image and projection dataset. Med Phys",
        "prism:doi": "10.1002/mp.14594",
        "fabio:hasPubMedId": "33202055",
        "foaf:homepage": "https://pubmed.ncbi.nlm.nih.gov/33202055",
        "dct:identifier": "33202055",
        "@context": {
          "dct": "http://purl.org/dc/terms/",
          "prism": "http://prismstandard.org/namespaces/basic/3.0/",
          "rdf": "http://www.w3.org/1999/02/22-rdf-syntax-ns#",
          "foaf": "http://xmlns.com/foaf/0.1/",
          "datmm": "http://schema.org/",
          "fabio": "http://purl.org/spar/fabio/"
        }
      }
    ],
    "dct:subject": [
      {
        "@type": "skos:Concept",
        "dct:identifier": "D001185",
        "skos:inScheme": "MeSH",
        "rdfs:label": "Artificial Intelligence",
        "@context": {
          "rdfs": "http://www.w3.org/2000/01/rdf-schema#",
          "skos": "http://www.w3.org/2004/02/skos/core#",
          "dct": "http://purl.org/dc/terms/"
        }
      },
      {
        "@type": "skos:Concept",
        "dct:identifier": "D014057",
        "skos:inScheme": "MeSH",
        "rdfs:label": "Tomography, X-Ray Computed",
        "@context": {
          "rdfs": "http://www.w3.org/2000/01/rdf-schema#",
          "skos": "http://www.w3.org/2004/02/skos/core#",
          "dct": "http://purl.org/dc/terms/"
        }
      }
    ],
    "@context": {
      "dct": "http://purl.org/dc/terms/",
      "foaf": "http://xmlns.com/foaf/0.1/",
      "datmm": "http://schema.org/"
    }
  },
  {
    "@type": "datmm:Dataset",
    "dct:description": "\n \n \n \n \n All the images are diagnostic contrast enhanced CT scans. The images were retrospectively acquired, to ensure sufficient patient follow-up. Slice thickness is variable : between 3 and 6 mm. All images were done at diagnosis and prior to surgery. The objective of the study was to extract prognostic image features that will describe lung adenocarcinomas and will associate with overall survival. \u00a0",
    "dct:format": "Unknown",
    "dct:issued": "2014/12/30",
    "foaf:homepage": "https://www.ncbi.nlm.nih.gov/gap",
    "dct:title": "LungCT-Diagnosis",
    "dct:language": "English",
    "bf:contribution": [],
    "dct:isPartOf": {
      "@type": "datmm:Repository",
      "dct:alternative": "TCIA",
      "foaf:homepage": "https://www.cancerimagingarchive.net",
      "dct:title": "The Cancer Imaging Archive",
      "@context": {
        "dct": "http://purl.org/dc/terms/",
        "foaf": "http://xmlns.com/foaf/0.1/",
        "datmm": "http://schema.org/"
      }
    },
    "frapo:isSupportedBy": [],
    "schema:distribution": [
      {
        "@type": "schema:DataDownload",
        "schema:contentSize": "2.5GB",
        "schema:encodingFormat": "DICOM",
        "schema:inLanguage": "en",
        "schema:name": "Images ",
        "schema:url": "https://wiki.cancerimagingarchive.net/display/Public/LungCT-Diagnosis/download/attachments/19039728/TCIA_LungCT-Diagnosis_06-22-2015.tcia?version=1&modificationDate=1534787004095&api=v2",
        "@context": {
          "schema": "http://schema.org/"
        }
      },
      {
        "@type": "schema:DataDownload",
        "schema:encodingFormat": "DICOM",
        "schema:inLanguage": "en",
        "schema:name": "DICOM Metadata Digest ",
        "schema:url": "https://wiki.cancerimagingarchive.net/display/Public/LungCT-Diagnosis/download/attachments/19039728/LungCT-Diagnosis_MetaData.csv?version=1&modificationDate=1495728280718&api=v2",
        "@context": {
          "schema": "http://schema.org/"
        }
      }
    ],
    "dct:isReferencedBy": [
      {
        "@type": "datmm:Documentation",
        "rdf:type": "Published Erratum",
        "dct:title": "Correction: Quantitative Computed Tomographic Descriptors Associate Tumor Shape Complexity and Intratumor Heterogeneity with Prognosis in Lung Adenocarcinoma.",
        "dct:bibliographicCitation": "Grove O, et al. Correction: Quantitative Computed Tomographic Descriptors Associate Tumor Shape Complexity and Intratumor Heterogeneity with Prognosis in Lung Adenocarcinoma. PLoS One",
        "prism:doi": "10.1371/journal.pone.0248541",
        "fabio:hasPubMedId": "33684181",
        "foaf:homepage": "https://pubmed.ncbi.nlm.nih.gov/33684181",
        "dct:identifier": "33684181",
        "@context": {
          "dct": "http://purl.org/dc/terms/",
          "prism": "http://prismstandard.org/namespaces/basic/3.0/",
          "rdf": "http://www.w3.org/1999/02/22-rdf-syntax-ns#",
          "foaf": "http://xmlns.com/foaf/0.1/",
          "datmm": "http://schema.org/",
          "fabio": "http://purl.org/spar/fabio/"
        }
      },
      {
        "@type": "datmm:Documentation",
        "rdf:type": "Journal Article",
        "dct:title": "Quantitative computed tomographic descriptors associate tumor shape complexity and intratumor heterogeneity with prognosis in lung adenocarcinoma.",
        "dct:bibliographicCitation": "Grove O, et al. Quantitative computed tomographic descriptors associate tumor shape complexity and intratumor heterogeneity with prognosis in lung adenocarcinoma. PLoS One",
        "prism:doi": "10.1371/journal.pone.0118261",
        "fabio:hasPubMedId": "25739030",
        "foaf:homepage": "https://pubmed.ncbi.nlm.nih.gov/25739030",
        "dct:identifier": "25739030",
        "@context": {
          "dct": "http://purl.org/dc/terms/",
          "prism": "http://prismstandard.org/namespaces/basic/3.0/",
          "rdf": "http://www.w3.org/1999/02/22-rdf-syntax-ns#",
          "foaf": "http://xmlns.com/foaf/0.1/",
          "datmm": "http://schema.org/",
          "fabio": "http://purl.org/spar/fabio/"
        }
      }
    ],
    "dct:subject": [
      {
        "@type": "skos:Concept",
        "dct:identifier": "D014057",
        "skos:inScheme": "MeSH",
        "rdfs:label": "Tomography, X-Ray Computed",
        "@context": {
          "rdfs": "http://www.w3.org/2000/01/rdf-schema#",
          "skos": "http://www.w3.org/2004/02/skos/core#",
          "dct": "http://purl.org/dc/terms/"
        }
      }
    ],
    "@context": {
      "dct": "http://purl.org/dc/terms/",
      "foaf": "http://xmlns.com/foaf/0.1/",
      "datmm": "http://schema.org/"
    }
  },
  {
    "@type": "datmm:Dataset",
    "dct:description": "\n \n This data set was provided in association with a ",
    "dct:format": "Unknown",
    "dct:issued": "2020/02/25",
    "foaf:homepage": "https://www.ncbi.nlm.nih.gov/gap",
    "dct:title": "Lung CT Segmentation Challenge 2017",
    "dct:language": "English",
    "bf:contribution": [],
    "dct:isPartOf": {
      "@type": "datmm:Repository",
      "dct:alternative": "TCIA",
      "foaf:homepage": "https://www.cancerimagingarchive.net",
      "dct:title": "The Cancer Imaging Archive",
      "@context": {
        "dct": "http://purl.org/dc/terms/",
        "foaf": "http://xmlns.com/foaf/0.1/",
        "datmm": "http://schema.org/"
      }
    },
    "frapo:isSupportedBy": [],
    "schema:distribution": [
      {
        "@type": "schema:DataDownload",
        "schema:contentSize": "4.8 GB",
        "schema:encodingFormat": "DICOM",
        "schema:inLanguage": "en",
        "schema:name": "Images\u00a0and Radiation Therapy Structures ",
        "schema:url": "https://wiki.cancerimagingarchive.net/display/Public/Lung+CT+Segmentation+Challenge+2017/download/attachments/24284539/LCTSC_v2_20190508.tcia?version=1&modificationDate=1557326860865&api=v2",
        "@context": {
          "schema": "http://schema.org/"
        }
      }
    ],
    "dct:isReferencedBy": [
      {
        "@type": "datmm:Documentation",
        "rdf:type": "Journal Article",
        "dct:title": "Autosegmentation for thoracic radiation treatment planning: A grand challenge at AAPM 2017.",
        "dct:bibliographicCitation": "Yang J, et al. Autosegmentation for thoracic radiation treatment planning: A grand challenge at AAPM 2017. Med Phys",
        "prism:doi": "10.1002/mp.13141",
        "fabio:hasPubMedId": "30144101",
        "foaf:homepage": "https://pubmed.ncbi.nlm.nih.gov/30144101",
        "dct:identifier": "30144101",
        "@context": {
          "dct": "http://purl.org/dc/terms/",
          "prism": "http://prismstandard.org/namespaces/basic/3.0/",
          "rdf": "http://www.w3.org/1999/02/22-rdf-syntax-ns#",
          "foaf": "http://xmlns.com/foaf/0.1/",
          "datmm": "http://schema.org/",
          "fabio": "http://purl.org/spar/fabio/"
        }
      }
    ],
    "dct:subject": [],
    "@context": {
      "dct": "http://purl.org/dc/terms/",
      "foaf": "http://xmlns.com/foaf/0.1/",
      "datmm": "http://schema.org/"
    }
  },
  {
    "@type": "datmm:Dataset",
    "dct:description": "This is the first attempt of mapping the extent of Invasive Adenocarcinoma onto ",
    "dct:format": "Unknown",
    "dct:issued": "07-30-2018",
    "foaf:homepage": "https://www.ncbi.nlm.nih.gov/gap",
    "dct:title": "Lung Fused-CT-Pathology",
    "dct:language": "English",
    "bf:contribution": [],
    "dct:isPartOf": {
      "@type": "datmm:Repository",
      "dct:alternative": "TCIA",
      "foaf:homepage": "https://www.cancerimagingarchive.net",
      "dct:title": "The Cancer Imaging Archive",
      "@context": {
        "dct": "http://purl.org/dc/terms/",
        "foaf": "http://xmlns.com/foaf/0.1/",
        "datmm": "http://schema.org/"
      }
    },
    "frapo:isSupportedBy": [],
    "schema:distribution": [
      {
        "@type": "schema:DataDownload",
        "schema:contentSize": "5.5 GB",
        "schema:encodingFormat": "DICOM",
        "schema:inLanguage": "en",
        "schema:name": "Images ",
        "schema:url": "https://wiki.cancerimagingarchive.net/display/Public/Lung+Fused-CT-Pathology/download/attachments/39878702/TCIA_Lung-Fused-CT-Pathology-2018-07-30.tcia?version=1&modificationDate=1541510138720&api=v2",
        "@context": {
          "schema": "http://schema.org/"
        }
      }
    ],
    "dct:isReferencedBy": [
      {
        "@type": "datmm:Documentation",
        "rdf:type": "Journal Article",
        "dct:title": "Co-registration of pre-operative CT with ex vivo surgically excised ground glass nodules to define spatial extent of invasive adenocarcinoma on in vivo imaging: a proof-of-concept study.",
        "dct:bibliographicCitation": "Rusu M, et al. Co-registration of pre-operative CT with ex vivo surgically excised ground glass nodules to define spatial extent of invasive adenocarcinoma on in vivo imaging: a proof-of-concept study. Eur Radiol",
        "prism:doi": "10.1007/s00330-017-4813-0",
        "fabio:hasPubMedId": "28386717",
        "foaf:homepage": "https://pubmed.ncbi.nlm.nih.gov/28386717",
        "dct:identifier": "28386717",
        "@context": {
          "dct": "http://purl.org/dc/terms/",
          "prism": "http://prismstandard.org/namespaces/basic/3.0/",
          "rdf": "http://www.w3.org/1999/02/22-rdf-syntax-ns#",
          "foaf": "http://xmlns.com/foaf/0.1/",
          "datmm": "http://schema.org/",
          "fabio": "http://purl.org/spar/fabio/"
        }
      }
    ],
    "dct:subject": [],
    "@context": {
      "dct": "http://purl.org/dc/terms/",
      "foaf": "http://xmlns.com/foaf/0.1/",
      "datmm": "http://schema.org/"
    }
  },
  {
    "@type": "datmm:Dataset",
    "dct:description": "The  FDA anthropomorphic thorax phantom  with 12 phantom lesions of different sizes (10 and 20 mm in effective diameter), shapes (spherical, elliptical, lobulated, and spiculated), and densities (\u2212630,\u221210, and +100 HU) was scanned at Columbia University Medical Center on a 64-detector row scanner (LightSpeed VCT, GE Healthcare, Milwaukee, WI). The CT scanning parameters were 120 kVp, 100 mAs, 64x0.625 collimation, and pitch of 1.375. The images were reconstructed with the lung kernel using 1.25 mm slice thickness.",
    "dct:format": "Unknown",
    "dct:issued": "2020/09/25",
    "foaf:homepage": "https://www.ncbi.nlm.nih.gov/gap",
    "dct:title": "Lung Phantom",
    "dct:language": "English",
    "bf:contribution": [],
    "dct:isPartOf": {
      "@type": "datmm:Repository",
      "dct:alternative": "TCIA",
      "foaf:homepage": "https://www.cancerimagingarchive.net",
      "dct:title": "The Cancer Imaging Archive",
      "@context": {
        "dct": "http://purl.org/dc/terms/",
        "foaf": "http://xmlns.com/foaf/0.1/",
        "datmm": "http://schema.org/"
      }
    },
    "frapo:isSupportedBy": [],
    "schema:distribution": [
      {
        "@type": "schema:DataDownload",
        "schema:encodingFormat": "DICOM",
        "schema:inLanguage": "en",
        "schema:name": "Images ",
        "schema:url": "https://wiki.cancerimagingarchive.net/display/Public/Lung+Phantom/download/attachments/19038256/TCIA_Lung_Phantom_06-22-2015.tcia?version=2&modificationDate=1601061652295&api=v2",
        "@context": {
          "schema": "http://schema.org/"
        }
      },
      {
        "@type": "schema:DataDownload",
        "schema:encodingFormat": "DICOM",
        "schema:inLanguage": "en",
        "schema:name": "DICOM Metadata Digest ",
        "schema:url": "https://wiki.cancerimagingarchive.net/display/Public/Lung+Phantom/download/attachments/19038256/LungPhantom_MetaData.csv?version=1&modificationDate=1495563917555&api=v2",
        "@context": {
          "schema": "http://schema.org/"
        }
      }
    ],
    "dct:isReferencedBy": [],
    "dct:subject": [],
    "@context": {
      "dct": "http://purl.org/dc/terms/",
      "foaf": "http://xmlns.com/foaf/0.1/",
      "datmm": "http://schema.org/"
    }
  },
  {
    "@type": "datmm:Dataset",
    "dct:description": "Background The COVID-19 pandemic is a global healthcare emergency. Prediction models for COVID-19 imaging are rapidly being developed to support medical decision making in imaging. However, inadequate availability of a diverse annotated dataset has limited the performance and generalizability of existing models.",
    "dct:format": "Unknown",
    "dct:issued": "2020/01/14",
    "foaf:homepage": "https://www.ncbi.nlm.nih.gov/gap",
    "dct:title": "Medical Imaging Data Resource Center (MIDRC) - RSNA International COVID-19 Open Radiology Database (RICORD) Release 1a - Chest CT Covid+ (MIDRC-RICORD-1a)",
    "dct:language": "English",
    "bf:contribution": [],
    "dct:isPartOf": {
      "@type": "datmm:Repository",
      "dct:alternative": "TCIA",
      "foaf:homepage": "https://www.cancerimagingarchive.net",
      "dct:title": "The Cancer Imaging Archive",
      "@context": {
        "dct": "http://purl.org/dc/terms/",
        "foaf": "http://xmlns.com/foaf/0.1/",
        "datmm": "http://schema.org/"
      }
    },
    "frapo:isSupportedBy": [],
    "schema:distribution": [],
    "dct:isReferencedBy": [
      {
        "@type": "datmm:Documentation",
        "rdf:type": "Journal Article",
        "dct:title": "The RSNA International COVID-19 Open Radiology Database (RICORD).",
        "dct:bibliographicCitation": "Tsai EB, et al. The RSNA International COVID-19 Open Radiology Database (RICORD). Radiology",
        "prism:doi": "10.1148/radiol.2021203957",
        "fabio:hasPubMedId": "33399506",
        "foaf:homepage": "https://pubmed.ncbi.nlm.nih.gov/33399506",
        "dct:identifier": "33399506",
        "@context": {
          "dct": "http://purl.org/dc/terms/",
          "prism": "http://prismstandard.org/namespaces/basic/3.0/",
          "rdf": "http://www.w3.org/1999/02/22-rdf-syntax-ns#",
          "foaf": "http://xmlns.com/foaf/0.1/",
          "datmm": "http://schema.org/",
          "fabio": "http://purl.org/spar/fabio/"
        }
      }
    ],
    "dct:subject": [],
    "@context": {
      "dct": "http://purl.org/dc/terms/",
      "foaf": "http://xmlns.com/foaf/0.1/",
      "datmm": "http://schema.org/"
    }
  },
  {
    "@type": "datmm:Dataset",
    "dct:description": "Background The COVID-19 pandemic is a global healthcare emergency. Prediction models for COVID-19 imaging are rapidly being developed to support medical decision making in imaging. However, inadequate availability of a diverse annotated dataset has limited the performance and generalizability of existing models.",
    "dct:format": "Unknown",
    "dct:issued": "2021/02/05",
    "foaf:homepage": "https://www.ncbi.nlm.nih.gov/gap",
    "dct:title": "Medical Imaging Data Resource Center (MIDRC) - RSNA International COVID-19 Open Radiology Database (RICORD) Release 1b - Chest CT Covid- (MIDRC-RICORD-1b)",
    "dct:language": "English",
    "bf:contribution": [],
    "dct:isPartOf": {
      "@type": "datmm:Repository",
      "dct:alternative": "TCIA",
      "foaf:homepage": "https://www.cancerimagingarchive.net",
      "dct:title": "The Cancer Imaging Archive",
      "@context": {
        "dct": "http://purl.org/dc/terms/",
        "foaf": "http://xmlns.com/foaf/0.1/",
        "datmm": "http://schema.org/"
      }
    },
    "frapo:isSupportedBy": [],
    "schema:distribution": [],
    "dct:isReferencedBy": [
      {
        "@type": "datmm:Documentation",
        "rdf:type": "Journal Article",
        "dct:title": "The RSNA International COVID-19 Open Radiology Database (RICORD).",
        "dct:bibliographicCitation": "Tsai EB, et al. The RSNA International COVID-19 Open Radiology Database (RICORD). Radiology",
        "prism:doi": "10.1148/radiol.2021203957",
        "fabio:hasPubMedId": "33399506",
        "foaf:homepage": "https://pubmed.ncbi.nlm.nih.gov/33399506",
        "dct:identifier": "33399506",
        "@context": {
          "dct": "http://purl.org/dc/terms/",
          "prism": "http://prismstandard.org/namespaces/basic/3.0/",
          "rdf": "http://www.w3.org/1999/02/22-rdf-syntax-ns#",
          "foaf": "http://xmlns.com/foaf/0.1/",
          "datmm": "http://schema.org/",
          "fabio": "http://purl.org/spar/fabio/"
        }
      }
    ],
    "dct:subject": [],
    "@context": {
      "dct": "http://purl.org/dc/terms/",
      "foaf": "http://xmlns.com/foaf/0.1/",
      "datmm": "http://schema.org/"
    }
  },
  {
    "@type": "datmm:Dataset",
    "dct:description": "Background The COVID-19 pandemic is a global healthcare emergency. Prediction models for COVID-19 imaging are rapidly being developed to support medical decision making in imaging. However, inadequate availability of a diverse annotated dataset has limited the performance and generalizability of existing models.",
    "dct:format": "Unknown",
    "dct:issued": "2021/01/15",
    "foaf:homepage": "https://www.ncbi.nlm.nih.gov/gap",
    "dct:title": "Medical Imaging Data Resource Center (MIDRC) - RSNA International COVID-19 Open Radiology Database (RICORD) Release 1c - Chest x-ray Covid+ (MIDRC-RICORD-1c)",
    "dct:language": "English",
    "bf:contribution": [],
    "dct:isPartOf": {
      "@type": "datmm:Repository",
      "dct:alternative": "TCIA",
      "foaf:homepage": "https://www.cancerimagingarchive.net",
      "dct:title": "The Cancer Imaging Archive",
      "@context": {
        "dct": "http://purl.org/dc/terms/",
        "foaf": "http://xmlns.com/foaf/0.1/",
        "datmm": "http://schema.org/"
      }
    },
    "frapo:isSupportedBy": [],
    "schema:distribution": [],
    "dct:isReferencedBy": [
      {
        "@type": "datmm:Documentation",
        "rdf:type": "Journal Article",
        "dct:title": "The RSNA International COVID-19 Open Radiology Database (RICORD).",
        "dct:bibliographicCitation": "Tsai EB, et al. The RSNA International COVID-19 Open Radiology Database (RICORD). Radiology",
        "prism:doi": "10.1148/radiol.2021203957",
        "fabio:hasPubMedId": "33399506",
        "foaf:homepage": "https://pubmed.ncbi.nlm.nih.gov/33399506",
        "dct:identifier": "33399506",
        "@context": {
          "dct": "http://purl.org/dc/terms/",
          "prism": "http://prismstandard.org/namespaces/basic/3.0/",
          "rdf": "http://www.w3.org/1999/02/22-rdf-syntax-ns#",
          "foaf": "http://xmlns.com/foaf/0.1/",
          "datmm": "http://schema.org/",
          "fabio": "http://purl.org/spar/fabio/"
        }
      }
    ],
    "dct:subject": [],
    "@context": {
      "dct": "http://purl.org/dc/terms/",
      "foaf": "http://xmlns.com/foaf/0.1/",
      "datmm": "http://schema.org/"
    }
  },
  {
    "@type": "datmm:Dataset",
    "dct:description": " Microscopic images were captured from bone marrow aspirate slides of patients diagnosed with multiple myeloma as per the standard guidelines. Slides were stained using Jenner- Giemsa stain. Images were captured at 1000x magnication using Nikon Eclipse-200 microscope equipped with a digital camera. Images were captured in raw BMP format with a size of 2560x1920 pixels. In all, this dataset consists of 85 images. All these 85 images were stain normalized using our in-house methodology before being used for segmentation. These stain normalized images have been provided as the annotated dataset with plasma cells marked in all image slides contained in a presentation for the ready reference of readers.",
    "dct:format": "Unknown",
    "dct:issued": "2019/03/25",
    "foaf:homepage": "https://www.ncbi.nlm.nih.gov/gap",
    "dct:title": "MiMM_SBILab Dataset: Microscopic Images of Multiple Myeloma",
    "dct:language": "English",
    "bf:contribution": [],
    "dct:isPartOf": {
      "@type": "datmm:Repository",
      "dct:alternative": "TCIA",
      "foaf:homepage": "https://www.cancerimagingarchive.net",
      "dct:title": "The Cancer Imaging Archive",
      "@context": {
        "dct": "http://purl.org/dc/terms/",
        "foaf": "http://xmlns.com/foaf/0.1/",
        "datmm": "http://schema.org/"
      }
    },
    "frapo:isSupportedBy": [],
    "schema:distribution": [],
    "dct:isReferencedBy": [
      {
        "@type": "datmm:Documentation",
        "rdf:type": "Published Erratum",
        "dct:title": "Correction to Lancet Infect Dis 2021; published online June 23. https://doi.org/10.1016/ S1473-3099(21)00330-3.",
        "dct:bibliographicCitation": ". Correction to Lancet Infect Dis 2021; published online June 23. https://doi.org/10.1016/ S1473-3099(21)00330-3. Lancet Infect Dis",
        "prism:doi": "10.1016/S1473-3099(21)00397-2",
        "fabio:hasPubMedId": "34237259",
        "foaf:homepage": "https://pubmed.ncbi.nlm.nih.gov/34237259",
        "dct:identifier": "34237259",
        "@context": {
          "dct": "http://purl.org/dc/terms/",
          "prism": "http://prismstandard.org/namespaces/basic/3.0/",
          "rdf": "http://www.w3.org/1999/02/22-rdf-syntax-ns#",
          "foaf": "http://xmlns.com/foaf/0.1/",
          "datmm": "http://schema.org/",
          "fabio": "http://purl.org/spar/fabio/"
        }
      },
      {
        "@type": "datmm:Documentation",
        "rdf:type": "Published Erratum",
        "dct:title": "Correction to Lancet Infectious Diseases 2020; published online April 29. https://doi.org/10.1016/ S1473-3099(20)30064-5.",
        "dct:bibliographicCitation": ". Correction to Lancet Infectious Diseases 2020; published online April 29. https://doi.org/10.1016/ S1473-3099(20)30064-5. Lancet Infect Dis",
        "prism:doi": "10.1016/S1473-3099(20)30370-4",
        "fabio:hasPubMedId": "32595044",
        "foaf:homepage": "https://pubmed.ncbi.nlm.nih.gov/32595044",
        "dct:identifier": "32595044",
        "@context": {
          "dct": "http://purl.org/dc/terms/",
          "prism": "http://prismstandard.org/namespaces/basic/3.0/",
          "rdf": "http://www.w3.org/1999/02/22-rdf-syntax-ns#",
          "foaf": "http://xmlns.com/foaf/0.1/",
          "datmm": "http://schema.org/",
          "fabio": "http://purl.org/spar/fabio/"
        }
      },
      {
        "@type": "datmm:Documentation",
        "rdf:type": "Journal Article",
        "dct:title": "Correction to Lancet Infect Dis 2020; published online March 11, https://doi.org/10.1016/ S1473-3099(20)30144-4.",
        "dct:bibliographicCitation": ". Correction to Lancet Infect Dis 2020; published online March 11, https://doi.org/10.1016/ S1473-3099(20)30144-4. Lancet Infect Dis",
        "prism:doi": "10.1016/S1473-3099(20)30251-6",
        "fabio:hasPubMedId": "32220652",
        "foaf:homepage": "https://pubmed.ncbi.nlm.nih.gov/32220652",
        "dct:identifier": "32220652",
        "@context": {
          "dct": "http://purl.org/dc/terms/",
          "prism": "http://prismstandard.org/namespaces/basic/3.0/",
          "rdf": "http://www.w3.org/1999/02/22-rdf-syntax-ns#",
          "foaf": "http://xmlns.com/foaf/0.1/",
          "datmm": "http://schema.org/",
          "fabio": "http://purl.org/spar/fabio/"
        }
      },
      {
        "@type": "datmm:Documentation",
        "rdf:type": "Published Erratum",
        "dct:title": "Correction to Lancet Diabetes Endocrinol 2019; published online March 1. DOI:10.1016/ S2213-8587(19)30066-X.",
        "dct:bibliographicCitation": ". Correction to Lancet Diabetes Endocrinol 2019; published online March 1. DOI:10.1016/ S2213-8587(19)30066-X. Lancet Diabetes Endocrinol",
        "prism:doi": "10.1016/S2213-8587(19)30109-3",
        "fabio:hasPubMedId": "30872122",
        "foaf:homepage": "https://pubmed.ncbi.nlm.nih.gov/30872122",
        "dct:identifier": "30872122",
        "@context": {
          "dct": "http://purl.org/dc/terms/",
          "prism": "http://prismstandard.org/namespaces/basic/3.0/",
          "rdf": "http://www.w3.org/1999/02/22-rdf-syntax-ns#",
          "foaf": "http://xmlns.com/foaf/0.1/",
          "datmm": "http://schema.org/",
          "fabio": "http://purl.org/spar/fabio/"
        }
      },
      {
        "@type": "datmm:Documentation",
        "rdf:type": "Journal Article",
        "dct:title": "Prohibitin 2: At a communications crossroads.",
        "dct:bibliographicCitation": "Bavelloni A, et al. Prohibitin 2: At a communications crossroads. IUBMB Life",
        "prism:doi": "10.1002/iub.1366",
        "fabio:hasPubMedId": "25904163",
        "foaf:homepage": "https://pubmed.ncbi.nlm.nih.gov/25904163",
        "dct:identifier": "25904163",
        "@context": {
          "dct": "http://purl.org/dc/terms/",
          "prism": "http://prismstandard.org/namespaces/basic/3.0/",
          "rdf": "http://www.w3.org/1999/02/22-rdf-syntax-ns#",
          "foaf": "http://xmlns.com/foaf/0.1/",
          "datmm": "http://schema.org/",
          "fabio": "http://purl.org/spar/fabio/"
        }
      },
      {
        "@type": "datmm:Documentation",
        "rdf:type": "Retraction of Publication",
        "dct:title": "Retraction for Ramos et al., The second RNA chaperone, Hfq2, is also required for survival under stress and full virulence of Burkholderia cenocepacia J2315.",
        "dct:bibliographicCitation": ". Retraction for Ramos et al., The second RNA chaperone, Hfq2, is also required for survival under stress and full virulence of Burkholderia cenocepacia J2315. J Bacteriol",
        "prism:doi": "10.1128/JB.02242-14",
        "fabio:hasPubMedId": "25319526",
        "foaf:homepage": "https://pubmed.ncbi.nlm.nih.gov/25319526",
        "dct:identifier": "25319526",
        "@context": {
          "dct": "http://purl.org/dc/terms/",
          "prism": "http://prismstandard.org/namespaces/basic/3.0/",
          "rdf": "http://www.w3.org/1999/02/22-rdf-syntax-ns#",
          "foaf": "http://xmlns.com/foaf/0.1/",
          "datmm": "http://schema.org/",
          "fabio": "http://purl.org/spar/fabio/"
        }
      },
      {
        "@type": "datmm:Documentation",
        "rdf:type": "Retraction of Publication",
        "dct:title": "Retraction notice to \u201cDifferential impact of diabetes and hypertension in the brain: adverse effects in grey matter\u201d [Neurobiol. Dis., 44 (2011) 161\u2013173, http://dx.doi.org/10.1016/ j.nbd.2011.06.005].",
        "dct:bibliographicCitation": ". Retraction notice to \u201cDifferential impact of diabetes and hypertension in the brain: adverse effects in grey matter\u201d [Neurobiol. Dis., 44 (2011) 161\u2013173, http://dx.doi.org/10.1016/ j.nbd.2011.06.005]. Neurobiol Dis",
        "prism:doi": "10.1016/j.nbd.2014.05.006",
        "fabio:hasPubMedId": "25077353",
        "foaf:homepage": "https://pubmed.ncbi.nlm.nih.gov/25077353",
        "dct:identifier": "25077353",
        "@context": {
          "dct": "http://purl.org/dc/terms/",
          "prism": "http://prismstandard.org/namespaces/basic/3.0/",
          "rdf": "http://www.w3.org/1999/02/22-rdf-syntax-ns#",
          "foaf": "http://xmlns.com/foaf/0.1/",
          "datmm": "http://schema.org/",
          "fabio": "http://purl.org/spar/fabio/"
        }
      },
      {
        "@type": "datmm:Documentation",
        "rdf:type": "Retraction of Publication",
        "dct:title": "Retraction notice to \u201cDifferential impact of diabetes and hypertension in the brain: adverse effects in white matter\u201d [Neurobiol. Dis., 42 (2011) 446\u2013458, http://dx.doi.org/10.1016/ j.nbd.2011.02.007].",
        "dct:bibliographicCitation": ". Retraction notice to \u201cDifferential impact of diabetes and hypertension in the brain: adverse effects in white matter\u201d [Neurobiol. Dis., 42 (2011) 446\u2013458, http://dx.doi.org/10.1016/ j.nbd.2011.02.007]. Neurobiol Dis",
        "prism:doi": "10.1016/j.nbd.2014.05.005",
        "fabio:hasPubMedId": "25077352",
        "foaf:homepage": "https://pubmed.ncbi.nlm.nih.gov/25077352",
        "dct:identifier": "25077352",
        "@context": {
          "dct": "http://purl.org/dc/terms/",
          "prism": "http://prismstandard.org/namespaces/basic/3.0/",
          "rdf": "http://www.w3.org/1999/02/22-rdf-syntax-ns#",
          "foaf": "http://xmlns.com/foaf/0.1/",
          "datmm": "http://schema.org/",
          "fabio": "http://purl.org/spar/fabio/"
        }
      },
      {
        "@type": "datmm:Documentation",
        "rdf:type": "Letter",
        "dct:title": "[Response to the response of the authors (DOI: 10.1016 / j.neuchi.2014.05.001), following our \"expert opinion\" (DOI: 10.1016 / j.neuchi.2014.06.001)].",
        "dct:bibliographicCitation": "Malca S. [Response to the response of the authors (DOI: 10.1016 / j.neuchi.2014.05.001), following our \"expert opinion\" (DOI: 10.1016 / j.neuchi.2014.06.001)]. Neurochirurgie",
        "prism:doi": "10.1016/j.neuchi.2014.06.003",
        "fabio:hasPubMedId": "25064137",
        "foaf:homepage": "https://pubmed.ncbi.nlm.nih.gov/25064137",
        "dct:identifier": "25064137",
        "@context": {
          "dct": "http://purl.org/dc/terms/",
          "prism": "http://prismstandard.org/namespaces/basic/3.0/",
          "rdf": "http://www.w3.org/1999/02/22-rdf-syntax-ns#",
          "foaf": "http://xmlns.com/foaf/0.1/",
          "datmm": "http://schema.org/",
          "fabio": "http://purl.org/spar/fabio/"
        }
      },
      {
        "@type": "datmm:Documentation",
        "rdf:type": "Letter",
        "dct:title": "[Response to the opinion of the expert Samuel Malca, regarding the article \"Ruptured aneurysm of the hepatic artery after lumbar spinal stenosis surgery. Forensic Reflections \"(Neurosurgery 2014; 60 (1-2): 38-41 DOI: 10.1016 / j.neuchi.2013.08.006.)].",
        "dct:bibliographicCitation": "Jecko V, et al. [Response to the opinion of the expert Samuel Malca, regarding the article \"Ruptured aneurysm of the hepatic artery after lumbar spinal stenosis surgery. Forensic Reflections \"(Neurosurgery 2014; 60 (1-2): 38-41 DOI: 10.1016 / j.neuchi.2013.08.006.)]. Neurochirurgie",
        "prism:doi": "10.1016/j.neuchi.2014.05.001",
        "fabio:hasPubMedId": "24994471",
        "foaf:homepage": "https://pubmed.ncbi.nlm.nih.gov/24994471",
        "dct:identifier": "24994471",
        "@context": {
          "dct": "http://purl.org/dc/terms/",
          "prism": "http://prismstandard.org/namespaces/basic/3.0/",
          "rdf": "http://www.w3.org/1999/02/22-rdf-syntax-ns#",
          "foaf": "http://xmlns.com/foaf/0.1/",
          "datmm": "http://schema.org/",
          "fabio": "http://purl.org/spar/fabio/"
        }
      },
      {
        "@type": "datmm:Documentation",
        "rdf:type": "Letter",
        "dct:title": "[Expert opinion on the article: \"Ruptured aneurysm of the hepatic artery after lumbar spinal stenosis surgery. Forensic Reflections \"(Neurosurgery 2014; 60 (1-2): 38-41 DOI: 10.1016 / j.neuchi.2013.08.006.)].",
        "dct:bibliographicCitation": "Malca S. [Expert opinion on the article: \"Ruptured aneurysm of the hepatic artery after lumbar spinal stenosis surgery. Forensic Reflections \"(Neurosurgery 2014; 60 (1-2): 38-41 DOI: 10.1016 / j.neuchi.2013.08.006.)]. Neurochirurgie",
        "prism:doi": "10.1016/j.neuchi.2014.06.001",
        "fabio:hasPubMedId": "24994470",
        "foaf:homepage": "https://pubmed.ncbi.nlm.nih.gov/24994470",
        "dct:identifier": "24994470",
        "@context": {
          "dct": "http://purl.org/dc/terms/",
          "prism": "http://prismstandard.org/namespaces/basic/3.0/",
          "rdf": "http://www.w3.org/1999/02/22-rdf-syntax-ns#",
          "foaf": "http://xmlns.com/foaf/0.1/",
          "datmm": "http://schema.org/",
          "fabio": "http://purl.org/spar/fabio/"
        }
      },
      {
        "@type": "datmm:Documentation",
        "rdf:type": "Journal Article",
        "dct:title": "WITHDRAWN: Ivory vertebra and systemic mastocytosis. Comments on the article by Frenzel et al.",
        "dct:bibliographicCitation": "Marhadour T, Saraux A. WITHDRAWN: Ivory vertebra and systemic mastocytosis. Comments on the article by Frenzel et al. Joint Bone Spine",
        "prism:doi": "10.1016/j.jbspin.2013.04.006",
        "fabio:hasPubMedId": "23731643",
        "foaf:homepage": "https://pubmed.ncbi.nlm.nih.gov/23731643",
        "dct:identifier": "23731643",
        "@context": {
          "dct": "http://purl.org/dc/terms/",
          "prism": "http://prismstandard.org/namespaces/basic/3.0/",
          "rdf": "http://www.w3.org/1999/02/22-rdf-syntax-ns#",
          "foaf": "http://xmlns.com/foaf/0.1/",
          "datmm": "http://schema.org/",
          "fabio": "http://purl.org/spar/fabio/"
        }
      },
      {
        "@type": "datmm:Documentation",
        "rdf:type": "Comment",
        "dct:title": "Comment on \"Ccl2, Cx3cr1 and Ccl2/Cx3cr1 chemokine deficiencies are not sufficient to cause age-related retinal degeneration\" by Luhmann et\u00a0al. (Exp. Eye Res. 2013; 107: 80.doi: 10.1016).",
        "dct:bibliographicCitation": "Combadi\u00e8re C, et al. Comment on \"Ccl2, Cx3cr1 and Ccl2/Cx3cr1 chemokine deficiencies are not sufficient to cause age-related retinal degeneration\" by Luhmann et\u00a0al. (Exp. Eye Res. 2013; 107: 80.doi: 10.1016). Exp Eye Res",
        "prism:doi": "10.1016/j.exer.2013.02.002",
        "fabio:hasPubMedId": "23402809",
        "foaf:homepage": "https://pubmed.ncbi.nlm.nih.gov/23402809",
        "dct:identifier": "23402809",
        "@context": {
          "dct": "http://purl.org/dc/terms/",
          "prism": "http://prismstandard.org/namespaces/basic/3.0/",
          "rdf": "http://www.w3.org/1999/02/22-rdf-syntax-ns#",
          "foaf": "http://xmlns.com/foaf/0.1/",
          "datmm": "http://schema.org/",
          "fabio": "http://purl.org/spar/fabio/"
        }
      }
    ],
    "dct:subject": [
      {
        "@type": "skos:Concept",
        "dct:identifier": "D006499",
        "skos:inScheme": "MeSH",
        "rdfs:label": "Hepatic Artery",
        "@context": {
          "rdfs": "http://www.w3.org/2000/01/rdf-schema#",
          "skos": "http://www.w3.org/2004/02/skos/core#",
          "dct": "http://purl.org/dc/terms/"
        }
      },
      {
        "@type": "skos:Concept",
        "dct:identifier": "D006499",
        "skos:inScheme": "MeSH",
        "rdfs:label": "Hepatic Artery",
        "@context": {
          "rdfs": "http://www.w3.org/2000/01/rdf-schema#",
          "skos": "http://www.w3.org/2004/02/skos/core#",
          "dct": "http://purl.org/dc/terms/"
        }
      },
      {
        "@type": "skos:Concept",
        "dct:identifier": "D006499",
        "skos:inScheme": "MeSH",
        "rdfs:label": "Hepatic Artery",
        "@context": {
          "rdfs": "http://www.w3.org/2000/01/rdf-schema#",
          "skos": "http://www.w3.org/2004/02/skos/core#",
          "dct": "http://purl.org/dc/terms/"
        }
      }
    ],
    "@context": {
      "dct": "http://purl.org/dc/terms/",
      "foaf": "http://xmlns.com/foaf/0.1/",
      "datmm": "http://schema.org/"
    }
  },
  {
    "@type": "datmm:Dataset",
    "dct:description": "This collection consists of magnetic resonance images (MRI) of genetically engineered mouse models (GEMMs) of high grade astrocytoma, including glioblastoma multiforme (GBM).",
    "dct:format": "Unknown",
    "dct:issued": "2017/03/21",
    "foaf:homepage": "https://www.ncbi.nlm.nih.gov/gap",
    "dct:title": "Mouse-Astrocytoma",
    "dct:language": "English",
    "bf:contribution": [],
    "dct:isPartOf": {
      "@type": "datmm:Repository",
      "dct:alternative": "TCIA",
      "foaf:homepage": "https://www.cancerimagingarchive.net",
      "dct:title": "The Cancer Imaging Archive",
      "@context": {
        "dct": "http://purl.org/dc/terms/",
        "foaf": "http://xmlns.com/foaf/0.1/",
        "datmm": "http://schema.org/"
      }
    },
    "frapo:isSupportedBy": [],
    "schema:distribution": [
      {
        "@type": "schema:DataDownload",
        "schema:contentSize": "2.0 GB",
        "schema:encodingFormat": "DICOM",
        "schema:inLanguage": "en",
        "schema:name": "Images ",
        "schema:url": "https://wiki.cancerimagingarchive.net/display/Public/Mouse-Astrocytoma/download/attachments/24283583/Mouse-Astrocytoma-doiJNLP.tcia?version=1&modificationDate=1534787031537&api=v2",
        "@context": {
          "schema": "http://schema.org/"
        }
      }
    ],
    "dct:isReferencedBy": [],
    "dct:subject": [],
    "@context": {
      "dct": "http://purl.org/dc/terms/",
      "foaf": "http://xmlns.com/foaf/0.1/",
      "datmm": "http://schema.org/"
    }
  },
  {
    "@type": "datmm:Dataset",
    "dct:description": "\n \n This collection consists of magnetic resonance images (MRI) of genetically engineered mouse models (GEMMs) of breast cancer.\u00a0 These images were acquired as part of a Department of Defense (DOD) Breast Cancer Research Program (BCRP) Postdoctoral Award W81XWH-12-1-0307 entitled \u201c",
    "dct:format": "Unknown",
    "dct:issued": "2015/03/18",
    "foaf:homepage": "https://www.ncbi.nlm.nih.gov/gap",
    "dct:title": "Mouse-Mammary",
    "dct:language": "English",
    "bf:contribution": [],
    "dct:isPartOf": {
      "@type": "datmm:Repository",
      "dct:alternative": "TCIA",
      "foaf:homepage": "https://www.cancerimagingarchive.net",
      "dct:title": "The Cancer Imaging Archive",
      "@context": {
        "dct": "http://purl.org/dc/terms/",
        "foaf": "http://xmlns.com/foaf/0.1/",
        "datmm": "http://schema.org/"
      }
    },
    "frapo:isSupportedBy": [],
    "schema:distribution": [
      {
        "@type": "schema:DataDownload",
        "schema:contentSize": "8.6GB",
        "schema:encodingFormat": "DICOM",
        "schema:inLanguage": "en",
        "schema:name": "Images ",
        "schema:url": "https://wiki.cancerimagingarchive.net/display/Public/Mouse-Mammary/download/attachments/20644280/TCIA_Mouse-Mammary_06-22-2015.tcia?version=1&modificationDate=1534787010965&api=v2",
        "@context": {
          "schema": "http://schema.org/"
        }
      }
    ],
    "dct:isReferencedBy": [],
    "dct:subject": [],
    "@context": {
      "dct": "http://purl.org/dc/terms/",
      "foaf": "http://xmlns.com/foaf/0.1/",
      "datmm": "http://schema.org/"
    }
  },
  {
    "@type": "datmm:Dataset",
    "dct:description": "This is a collection of F-18 NaF positron emission tomography/computed tomography (PET/CT) images in patients with prostate cancer, with suspected or known bone involvement.",
    "dct:format": "Unknown",
    "dct:issued": "2013/4/23",
    "foaf:homepage": "https://www.ncbi.nlm.nih.gov/gap",
    "dct:title": "NaF Prostate",
    "dct:language": "English",
    "bf:contribution": [],
    "dct:isPartOf": {
      "@type": "datmm:Repository",
      "dct:alternative": "TCIA",
      "foaf:homepage": "https://www.cancerimagingarchive.net",
      "dct:title": "The Cancer Imaging Archive",
      "@context": {
        "dct": "http://purl.org/dc/terms/",
        "foaf": "http://xmlns.com/foaf/0.1/",
        "datmm": "http://schema.org/"
      }
    },
    "frapo:isSupportedBy": [],
    "schema:distribution": [
      {
        "@type": "schema:DataDownload",
        "schema:encodingFormat": "DICOM",
        "schema:inLanguage": "en",
        "schema:name": "DICOM Metadata Digest ",
        "schema:url": "https://wiki.cancerimagingarchive.net/display/Public/NaF+Prostate/download/attachments/3539105/NaF%20Prostate_MetaData.csv?version=1&modificationDate=1495728368893&api=v2",
        "@context": {
          "schema": "http://schema.org/"
        }
      }
    ],
    "dct:isReferencedBy": [],
    "dct:subject": [],
    "@context": {
      "dct": "http://purl.org/dc/terms/",
      "foaf": "http://xmlns.com/foaf/0.1/",
      "datmm": "http://schema.org/"
    }
  },
  {
    "@type": "datmm:Dataset",
    "dct:description": "This data collection consists of images acquired in preparation for ",
    "dct:format": "Unknown",
    "dct:issued": "2015/09/14",
    "foaf:homepage": "https://www.ncbi.nlm.nih.gov/gap",
    "dct:title": "NRG-1308",
    "dct:language": "English",
    "bf:contribution": [],
    "dct:isPartOf": {
      "@type": "datmm:Repository",
      "dct:alternative": "TCIA",
      "foaf:homepage": "https://www.cancerimagingarchive.net",
      "dct:title": "The Cancer Imaging Archive",
      "@context": {
        "dct": "http://purl.org/dc/terms/",
        "foaf": "http://xmlns.com/foaf/0.1/",
        "datmm": "http://schema.org/"
      }
    },
    "frapo:isSupportedBy": [],
    "schema:distribution": [
      {
        "@type": "schema:DataDownload",
        "schema:contentSize": "1.7GB",
        "schema:encodingFormat": "DICOM",
        "schema:inLanguage": "en",
        "schema:name": "Images\u00a0and Radiation Therapy Structures ",
        "schema:url": "https://wiki.cancerimagingarchive.net/display/Public/NRG-1308/download/attachments/22513508/NRG-1308_2015-09-14.tcia?version=1&modificationDate=1542736564760&api=v2",
        "@context": {
          "schema": "http://schema.org/"
        }
      }
    ],
    "dct:isReferencedBy": [],
    "dct:subject": [],
    "@context": {
      "dct": "http://purl.org/dc/terms/",
      "foaf": "http://xmlns.com/foaf/0.1/",
      "datmm": "http://schema.org/"
    }
  },
  {
    "@type": "datmm:Dataset",
    "dct:description": "This collection contains data from the National Cancer Insitute Clinical Trial ",
    "dct:format": "Unknown",
    "dct:issued": "2019/04/15",
    "foaf:homepage": "https://www.ncbi.nlm.nih.gov/gap",
    "dct:title": "NSCLC-Cetuximab (RTOG-0617)",
    "dct:language": "English",
    "bf:contribution": [],
    "dct:isPartOf": {
      "@type": "datmm:Repository",
      "dct:alternative": "TCIA",
      "foaf:homepage": "https://www.cancerimagingarchive.net",
      "dct:title": "The Cancer Imaging Archive",
      "@context": {
        "dct": "http://purl.org/dc/terms/",
        "foaf": "http://xmlns.com/foaf/0.1/",
        "datmm": "http://schema.org/"
      }
    },
    "frapo:isSupportedBy": [],
    "schema:distribution": [],
    "dct:isReferencedBy": [],
    "dct:subject": [],
    "@context": {
      "dct": "http://purl.org/dc/terms/",
      "foaf": "http://xmlns.com/foaf/0.1/",
      "datmm": "http://schema.org/"
    }
  },
  {
    "@type": "datmm:Dataset",
    "dct:description": "Medical image biomarkers of cancer promise improvements in patient care through\u00a0advances in precision medicine. Compared to genomic biomarkers, image\u00a0biomarkers\u00a0provide the advantages of being a non-invasive procedure, and characterizing a\u00a0heterogeneous tumor in its entirety, as opposed to limited tissue available for\u00a0biopsy. We\u00a0developed a unique radiogenomic dataset from a Non-Small Cell Lung Cancer (NSCLC) cohort\u00a0of 211 subjects. The dataset comprises Computed\u00a0Tomography (CT), Positron Emission\u00a0Tomography (PET)/CT images, semantic annotations of the tumors as observed on the\u00a0medical images using a controlled\u00a0vocabulary, segmentation maps of tumors in the CT scans,\u00a0and quantitative values obtained from the PET/CT scans. Imaging data are also paired with\u00a0gene mutation,\u00a0RNA sequencing data from samples of surgically excised tumor tissue, and\u00a0clinical data, including survival outcomes. This dataset was created to facilitate the discovery\u00a0of the underlying relationship between genomic and medical image features, as well as the\u00a0development and evaluation of prognostic medical image biomarkers.",
    "dct:format": "Unknown",
    "dct:issued": "2021/06/01",
    "foaf:homepage": "https://www.ncbi.nlm.nih.gov/gap",
    "dct:title": "NSCLC Radiogenomics",
    "dct:language": "English",
    "bf:contribution": [],
    "dct:isPartOf": {
      "@type": "datmm:Repository",
      "dct:alternative": "TCIA",
      "foaf:homepage": "https://www.cancerimagingarchive.net",
      "dct:title": "The Cancer Imaging Archive",
      "@context": {
        "dct": "http://purl.org/dc/terms/",
        "foaf": "http://xmlns.com/foaf/0.1/",
        "datmm": "http://schema.org/"
      }
    },
    "frapo:isSupportedBy": [],
    "schema:distribution": [
      {
        "@type": "schema:DataDownload",
        "schema:contentSize": "97.6 GB",
        "schema:encodingFormat": "DICOM",
        "schema:inLanguage": "en",
        "schema:name": "Images and Segmentations ",
        "schema:url": "https://wiki.cancerimagingarchive.net/display/Public/NSCLC+Radiogenomics/download/attachments/28672347/NSCLC_Radiogenomics-6-1-21%20Version%204.tcia?version=1&modificationDate=1622561925765&api=v2",
        "@context": {
          "schema": "http://schema.org/"
        }
      }
    ],
    "dct:isReferencedBy": [
      {
        "@type": "datmm:Documentation",
        "rdf:type": "Journal Article",
        "dct:title": "A radiogenomic dataset of non-small cell lung cancer.",
        "dct:bibliographicCitation": "Bakr S, et al. A radiogenomic dataset of non-small cell lung cancer. Sci Data",
        "prism:doi": "10.1038/sdata.2018.202",
        "fabio:hasPubMedId": "30325352",
        "foaf:homepage": "https://pubmed.ncbi.nlm.nih.gov/30325352",
        "dct:identifier": "30325352",
        "@context": {
          "dct": "http://purl.org/dc/terms/",
          "prism": "http://prismstandard.org/namespaces/basic/3.0/",
          "rdf": "http://www.w3.org/1999/02/22-rdf-syntax-ns#",
          "foaf": "http://xmlns.com/foaf/0.1/",
          "datmm": "http://schema.org/",
          "fabio": "http://purl.org/spar/fabio/"
        }
      }
    ],
    "dct:subject": [
      {
        "@type": "skos:Concept",
        "dct:identifier": "D002289",
        "skos:inScheme": "MeSH",
        "rdfs:label": "Carcinoma, Non-Small-Cell Lung",
        "@context": {
          "rdfs": "http://www.w3.org/2000/01/rdf-schema#",
          "skos": "http://www.w3.org/2004/02/skos/core#",
          "dct": "http://purl.org/dc/terms/"
        }
      },
      {
        "@type": "skos:Concept",
        "dct:identifier": "D008175",
        "skos:inScheme": "MeSH",
        "rdfs:label": "Lung Neoplasms",
        "@context": {
          "rdfs": "http://www.w3.org/2000/01/rdf-schema#",
          "skos": "http://www.w3.org/2004/02/skos/core#",
          "dct": "http://purl.org/dc/terms/"
        }
      }
    ],
    "@context": {
      "dct": "http://purl.org/dc/terms/",
      "foaf": "http://xmlns.com/foaf/0.1/",
      "datmm": "http://schema.org/"
    }
  },
  {
    "@type": "datmm:Dataset",
    "dct:description": "This collection contains images from 422 non-small cell lung cancer (NSCLC) patients. For these patients pretreatment CT scans,\u00a0manual delineation by a radiation oncologist of the 3D volume of the gross tumor volume and clinical outcome data are available. This dataset refers to the Lung1 dataset of the ",
    "dct:format": "Unknown",
    "dct:issued": "2020/10/22",
    "foaf:homepage": "https://www.ncbi.nlm.nih.gov/gap",
    "dct:title": "NSCLC-Radiomics",
    "dct:language": "English",
    "bf:contribution": [],
    "dct:isPartOf": {
      "@type": "datmm:Repository",
      "dct:alternative": "TCIA",
      "foaf:homepage": "https://www.cancerimagingarchive.net",
      "dct:title": "The Cancer Imaging Archive",
      "@context": {
        "dct": "http://purl.org/dc/terms/",
        "foaf": "http://xmlns.com/foaf/0.1/",
        "datmm": "http://schema.org/"
      }
    },
    "frapo:isSupportedBy": [],
    "schema:distribution": [
      {
        "@type": "schema:DataDownload",
        "schema:contentSize": "33GB",
        "schema:encodingFormat": "DICOM",
        "schema:inLanguage": "en",
        "schema:name": "Images, Segmentations, and Radiation Therapy Structures ",
        "schema:url": "https://wiki.cancerimagingarchive.net/display/Public/NSCLC-Radiomics/download/attachments/16056854/NSCLC%20Radiomics%20Version%204%20Oct%202020%20NBIA-manifest.tcia?version=1&modificationDate=1603198863613&api=v2",
        "@context": {
          "schema": "http://schema.org/"
        }
      }
    ],
    "dct:isReferencedBy": [],
    "dct:subject": [],
    "@context": {
      "dct": "http://purl.org/dc/terms/",
      "foaf": "http://xmlns.com/foaf/0.1/",
      "datmm": "http://schema.org/"
    }
  },
  {
    "@type": "datmm:Dataset",
    "dct:description": "This collection contains images from 89 non-small cell lung cancer (NSCLC) patients that were treated with surgery. For these patients pretreatment CT scans, gene expression, and clinical data are available. This dataset refers to the Lung3 dataset of the ",
    "dct:format": "Unknown",
    "dct:issued": "2014/07/02",
    "foaf:homepage": "https://www.ncbi.nlm.nih.gov/gap",
    "dct:title": "NSCLC-Radiomics-Genomics",
    "dct:language": "English",
    "bf:contribution": [],
    "dct:isPartOf": {
      "@type": "datmm:Repository",
      "dct:alternative": "TCIA",
      "foaf:homepage": "https://www.cancerimagingarchive.net",
      "dct:title": "The Cancer Imaging Archive",
      "@context": {
        "dct": "http://purl.org/dc/terms/",
        "foaf": "http://xmlns.com/foaf/0.1/",
        "datmm": "http://schema.org/"
      }
    },
    "frapo:isSupportedBy": [],
    "schema:distribution": [
      {
        "@type": "schema:DataDownload",
        "schema:contentSize": "6.6GB",
        "schema:encodingFormat": "DICOM",
        "schema:inLanguage": "en",
        "schema:name": "Images ",
        "schema:url": "https://wiki.cancerimagingarchive.net/display/Public/NSCLC-Radiomics-Genomics/download/attachments/16056856/TCIA_NSCLC-Radiomics-Genomics_06-22-2015.tcia?version=1&modificationDate=1534787429713&api=v2",
        "@context": {
          "schema": "http://schema.org/"
        }
      }
    ],
    "dct:isReferencedBy": [
      {
        "@type": "datmm:Documentation",
        "rdf:type": "Journal Article",
        "dct:title": "Decoding tumour phenotype by noninvasive imaging using a quantitative radiomics approach.",
        "dct:bibliographicCitation": "Aerts HJ, et al. Decoding tumour phenotype by noninvasive imaging using a quantitative radiomics approach. Nat Commun",
        "prism:doi": "10.1038/ncomms5006",
        "fabio:hasPubMedId": "24892406",
        "foaf:homepage": "https://pubmed.ncbi.nlm.nih.gov/24892406",
        "dct:identifier": "24892406",
        "@context": {
          "dct": "http://purl.org/dc/terms/",
          "prism": "http://prismstandard.org/namespaces/basic/3.0/",
          "rdf": "http://www.w3.org/1999/02/22-rdf-syntax-ns#",
          "foaf": "http://xmlns.com/foaf/0.1/",
          "datmm": "http://schema.org/",
          "fabio": "http://purl.org/spar/fabio/"
        }
      }
    ],
    "dct:subject": [],
    "@context": {
      "dct": "http://purl.org/dc/terms/",
      "foaf": "http://xmlns.com/foaf/0.1/",
      "datmm": "http://schema.org/"
    }
  },
  {
    "@type": "datmm:Dataset",
    "dct:description": "This collection contains clinical data and computed tomography (CT) from 22 non-small cell lung cancer (NSCLC) radiotherapy patients. For 21 of these patients with pre-treatment CT scans, repeated blinded manual delineations by five different radiation oncologists of the 3D volume of the gross tumor volume on CT and clinical outcome data are available. The above was repeated with the same set of five radiation oncologists, using an in-house autosegmentation tool for initial delineation followed by manual adjustment of the primary gross tumor volume outline. For one patient, clinical data and CT was available but the tumor delineations were not extracted. This patient was included in this collection for the sake of completeness.",
    "dct:format": "Unknown",
    "dct:issued": "2020/08/31",
    "foaf:homepage": "https://www.ncbi.nlm.nih.gov/gap",
    "dct:title": "NSCLC-Radiomics-Interobserver1",
    "dct:language": "English",
    "bf:contribution": [],
    "dct:isPartOf": {
      "@type": "datmm:Repository",
      "dct:alternative": "TCIA",
      "foaf:homepage": "https://www.cancerimagingarchive.net",
      "dct:title": "The Cancer Imaging Archive",
      "@context": {
        "dct": "http://purl.org/dc/terms/",
        "foaf": "http://xmlns.com/foaf/0.1/",
        "datmm": "http://schema.org/"
      }
    },
    "frapo:isSupportedBy": [],
    "schema:distribution": [
      {
        "@type": "schema:DataDownload",
        "schema:contentSize": "3.2 GB",
        "schema:encodingFormat": "DICOM",
        "schema:inLanguage": "en",
        "schema:name": "Images ",
        "schema:url": "https://wiki.cancerimagingarchive.net/display/Public/NSCLC-Radiomics-Interobserver1/download/attachments/52756590/NSCLC-RADIOMICS-INTEROBSERVER1-Aug%2031%202020-NBIA-manifest.tcia?version=1&modificationDate=1598890227618&api=v2",
        "@context": {
          "schema": "http://schema.org/"
        }
      }
    ],
    "dct:isReferencedBy": [],
    "dct:subject": [],
    "@context": {
      "dct": "http://purl.org/dc/terms/",
      "foaf": "http://xmlns.com/foaf/0.1/",
      "datmm": "http://schema.org/"
    }
  },
  {
    "@type": "datmm:Dataset",
    "dct:description": "Osteosarcoma is the most common type of bone cancer that occurs in adolescents in the age of 10 to 14 years. The dataset is composed of Hematoxylin and eosin (H&E) stained osteosarcoma histology images. The data was collected by a team of clinical scientists at University of Texas Southwestern Medical Center, Dallas. Archival samples for 50 patients treated at Children\u2019 s Medical Center, Dallas, between 1995 and 2015, were used to create this dataset. Four patients (out of 50) were selected by pathologists based on diversity of tumor specimens after surgical resection. The images are labelled as Non-Tumor, Viable Tumor and Necrosis according to the predominant cancer type in each image. The annotation was performed by two medical experts. All images were divided between two pathologists for the annotation activity. Each image had a single annotation as any given image was annotated by only one pathologist. The dataset consists of 1144 images of size 1024 X 1024 at 10X resolution with the following distribution: 536 (47%) non-tumor images, 263 (23%) necrotic tumor images and 345 (30%) viable tumor tiles.",
    "dct:format": "Unknown",
    "dct:issued": "2019/03/22",
    "foaf:homepage": "https://www.ncbi.nlm.nih.gov/gap",
    "dct:title": "Osteosarcoma data from UT Southwestern/UT Dallas for Viable and Necrotic Tumor Assessment (Osteosarcoma-Tumor-Assessment)",
    "dct:language": "English",
    "bf:contribution": [],
    "dct:isPartOf": {
      "@type": "datmm:Repository",
      "dct:alternative": "TCIA",
      "foaf:homepage": "https://www.cancerimagingarchive.net",
      "dct:title": "The Cancer Imaging Archive",
      "@context": {
        "dct": "http://purl.org/dc/terms/",
        "foaf": "http://xmlns.com/foaf/0.1/",
        "datmm": "http://schema.org/"
      }
    },
    "frapo:isSupportedBy": [],
    "schema:distribution": [],
    "dct:isReferencedBy": [],
    "dct:subject": [],
    "@context": {
      "dct": "http://purl.org/dc/terms/",
      "foaf": "http://xmlns.com/foaf/0.1/",
      "datmm": "http://schema.org/"
    }
  },
  {
    "@type": "datmm:Dataset",
    "dct:description": "The National Institutes of Health Clinical Center performed 82 abdominal contrast enhanced 3D CT scans (~70 seconds after intravenous contrast injection in portal-venous) from 53 male and 27 female subjects.\u00a0 Seventeen of the subjects are healthy kidney donors scanned prior to nephrectomy.\u00a0 The remaining 65 patients were selected by a radiologist from patients who neither had major abdominal pathologies nor pancreatic cancer lesions.\u00a0 Subjects' ages range from 18 to 76 years with a mean age of 46.8 \u00b1 16.7. The CT scans have resolutions of 512x512 pixels with varying pixel sizes and slice thickness between 1.5 \u2212 2.5 mm, acquired on Philips and Siemens MDCT scanners (120 kVp tube voltage).",
    "dct:format": "Unknown",
    "dct:issued": "2020/09/10",
    "foaf:homepage": "https://www.ncbi.nlm.nih.gov/gap",
    "dct:title": "Pancreas-CT",
    "dct:language": "English",
    "bf:contribution": [],
    "dct:isPartOf": {
      "@type": "datmm:Repository",
      "dct:alternative": "TCIA",
      "foaf:homepage": "https://www.cancerimagingarchive.net",
      "dct:title": "The Cancer Imaging Archive",
      "@context": {
        "dct": "http://purl.org/dc/terms/",
        "foaf": "http://xmlns.com/foaf/0.1/",
        "datmm": "http://schema.org/"
      }
    },
    "frapo:isSupportedBy": [],
    "schema:distribution": [
      {
        "@type": "schema:DataDownload",
        "schema:contentSize": "9.3 GB",
        "schema:encodingFormat": "DICOM",
        "schema:inLanguage": "en",
        "schema:name": "Images ",
        "schema:url": "https://wiki.cancerimagingarchive.net/display/Public/Pancreas-CT/download/attachments/22514040/Pancreas-CT%2020200910.tcia?version=1&modificationDate=1599754273288&api=v2",
        "@context": {
          "schema": "http://schema.org/"
        }
      }
    ],
    "dct:isReferencedBy": [],
    "dct:subject": [],
    "@context": {
      "dct": "http://purl.org/dc/terms/",
      "foaf": "http://xmlns.com/foaf/0.1/",
      "datmm": "http://schema.org/"
    }
  },
  {
    "@type": "datmm:Dataset",
    "dct:description": "Purpose:  Expert selected landmark points on clinical image pairs provide a basis for rigid registration validation. Using combinatorial rigid registration optimization (CORRO) we provide a statistically characterized reference data set for image registration of the pelvis by estimating the optimal ground truth.",
    "dct:format": "Unknown",
    "dct:issued": "2019/09/13",
    "foaf:homepage": "https://www.ncbi.nlm.nih.gov/gap",
    "dct:title": "Pelvic Reference Data",
    "dct:language": "English",
    "bf:contribution": [],
    "dct:isPartOf": {
      "@type": "datmm:Repository",
      "dct:alternative": "TCIA",
      "foaf:homepage": "https://www.cancerimagingarchive.net",
      "dct:title": "The Cancer Imaging Archive",
      "@context": {
        "dct": "http://purl.org/dc/terms/",
        "foaf": "http://xmlns.com/foaf/0.1/",
        "datmm": "http://schema.org/"
      }
    },
    "frapo:isSupportedBy": [],
    "schema:distribution": [
      {
        "@type": "schema:DataDownload",
        "schema:contentSize": "7 GB",
        "schema:encodingFormat": "DICOM",
        "schema:inLanguage": "en",
        "schema:name": "Images ",
        "schema:url": "https://wiki.cancerimagingarchive.net/display/Public/Pelvic+Reference+Data/download/attachments/59310517/TCIA-Pelvic-Reference-Data.tcia?version=1&modificationDate=1568393224796&api=v2",
        "@context": {
          "schema": "http://schema.org/"
        }
      }
    ],
    "dct:isReferencedBy": [],
    "dct:subject": [],
    "@context": {
      "dct": "http://purl.org/dc/terms/",
      "foaf": "http://xmlns.com/foaf/0.1/",
      "datmm": "http://schema.org/"
    }
  },
  {
    "@type": "datmm:Dataset",
    "dct:description": "As part of a more general effort to probe the interrelated factors impacting the accuracy and precision of lung nodule size estimation, we have been conducting phantom CT studies with an anthropomorphic thoracic phantom containing a vasculature insert on which synthetic nodules were inserted or attached.",
    "dct:format": "Unknown",
    "dct:issued": "2017/08/30",
    "foaf:homepage": "https://www.ncbi.nlm.nih.gov/gap",
    "dct:title": "Phantom FDA",
    "dct:language": "English",
    "bf:contribution": [],
    "dct:isPartOf": {
      "@type": "datmm:Repository",
      "dct:alternative": "TCIA",
      "foaf:homepage": "https://www.cancerimagingarchive.net",
      "dct:title": "The Cancer Imaging Archive",
      "@context": {
        "dct": "http://purl.org/dc/terms/",
        "foaf": "http://xmlns.com/foaf/0.1/",
        "datmm": "http://schema.org/"
      }
    },
    "frapo:isSupportedBy": [],
    "schema:distribution": [
      {
        "@type": "schema:DataDownload",
        "schema:contentSize": "728.5GB",
        "schema:encodingFormat": "DICOM",
        "schema:inLanguage": "en",
        "schema:name": "Images ",
        "schema:url": "https://wiki.cancerimagingarchive.net/display/Public/Phantom+FDA/download/attachments/3997704/Phantom_FDAv2-doiJNLP-FIR0jVwr.tcia?version=1&modificationDate=1534786955884&api=v2",
        "@context": {
          "schema": "http://schema.org/"
        }
      },
      {
        "@type": "schema:DataDownload",
        "schema:encodingFormat": "DICOM",
        "schema:inLanguage": "en",
        "schema:name": "DICOM Metadata Digest ",
        "schema:url": "https://wiki.cancerimagingarchive.net/display/Public/Phantom+FDA/download/attachments/3997704/PhantomFDA_MetaData_v2.csv?version=1&modificationDate=1504111582281&api=v2",
        "@context": {
          "schema": "http://schema.org/"
        }
      }
    ],
    "dct:isReferencedBy": [
      {
        "@type": "datmm:Documentation",
        "rdf:type": "Journal Article",
        "dct:title": "A resource for the assessment of lung nodule size estimation methods: database of thoracic CT scans of an anthropomorphic phantom.",
        "dct:bibliographicCitation": "Gavrielides MA, et al. A resource for the assessment of lung nodule size estimation methods: database of thoracic CT scans of an anthropomorphic phantom. Opt Express",
        "prism:doi": "10.1364/OE.18.015244",
        "fabio:hasPubMedId": "20640011",
        "foaf:homepage": "https://pubmed.ncbi.nlm.nih.gov/20640011",
        "dct:identifier": "20640011",
        "@context": {
          "dct": "http://purl.org/dc/terms/",
          "prism": "http://prismstandard.org/namespaces/basic/3.0/",
          "rdf": "http://www.w3.org/1999/02/22-rdf-syntax-ns#",
          "foaf": "http://xmlns.com/foaf/0.1/",
          "datmm": "http://schema.org/",
          "fabio": "http://purl.org/spar/fabio/"
        }
      }
    ],
    "dct:subject": [
      {
        "@type": "skos:Concept",
        "dct:identifier": "D019047",
        "skos:inScheme": "MeSH",
        "rdfs:label": "Phantoms, Imaging",
        "@context": {
          "rdfs": "http://www.w3.org/2000/01/rdf-schema#",
          "skos": "http://www.w3.org/2004/02/skos/core#",
          "dct": "http://purl.org/dc/terms/"
        }
      }
    ],
    "@context": {
      "dct": "http://purl.org/dc/terms/",
      "foaf": "http://xmlns.com/foaf/0.1/",
      "datmm": "http://schema.org/"
    }
  },
  {
    "@type": "datmm:Dataset",
    "dct:description": "\n Prostate transversal T2-weighted magnetic resonance images (MRIs) acquired on a 3.0T Siemens TrioTim using only a pelvic phased-array coil were acquired for prostate cancer detection. The data was provided to TCIA as part of an ",
    "dct:format": "Unknown",
    "dct:issued": "2013/05/31",
    "foaf:homepage": "https://www.ncbi.nlm.nih.gov/gap",
    "dct:title": "Prostate-3T",
    "dct:language": "English",
    "bf:contribution": [],
    "dct:isPartOf": {
      "@type": "datmm:Repository",
      "dct:alternative": "TCIA",
      "foaf:homepage": "https://www.cancerimagingarchive.net",
      "dct:title": "The Cancer Imaging Archive",
      "@context": {
        "dct": "http://purl.org/dc/terms/",
        "foaf": "http://xmlns.com/foaf/0.1/",
        "datmm": "http://schema.org/"
      }
    },
    "frapo:isSupportedBy": [],
    "schema:distribution": [
      {
        "@type": "schema:DataDownload",
        "schema:encodingFormat": "DICOM",
        "schema:inLanguage": "en",
        "schema:name": "Images ",
        "schema:url": "https://wiki.cancerimagingarchive.net/display/Public/Prostate-3T/download/attachments/6882785/TCIA_Prostate-3T_06-22-2015.jnlp?version=2&modificationDate=1450816899831&api=v2",
        "@context": {
          "schema": "http://schema.org/"
        }
      }
    ],
    "dct:isReferencedBy": [],
    "dct:subject": [],
    "@context": {
      "dct": "http://purl.org/dc/terms/",
      "foaf": "http://xmlns.com/foaf/0.1/",
      "datmm": "http://schema.org/"
    }
  },
  {
    "@type": "datmm:Dataset",
    "dct:description": "Prostate cancer T1- and T2-weighted magnetic resonance images (MRIs) were acquired on a 1.5 T Philips Achieva by combined surface and endorectal coil, including dynamic contrast-enhanced images obtained prior to, during and after I.V. administration of 0.1 mmol/kg body weight of Gadolinium-DTPA (pentetic acid). For general or scientific inquiries please\u00a0",
    "dct:format": "Unknown",
    "dct:issued": "2021/08/09:",
    "foaf:homepage": "https://www.ncbi.nlm.nih.gov/gap",
    "dct:title": "PROSTATE-DIAGNOSIS",
    "dct:language": "English",
    "bf:contribution": [],
    "dct:isPartOf": {
      "@type": "datmm:Repository",
      "dct:alternative": "TCIA",
      "foaf:homepage": "https://www.cancerimagingarchive.net",
      "dct:title": "The Cancer Imaging Archive",
      "@context": {
        "dct": "http://purl.org/dc/terms/",
        "foaf": "http://xmlns.com/foaf/0.1/",
        "datmm": "http://schema.org/"
      }
    },
    "frapo:isSupportedBy": [],
    "schema:distribution": [
      {
        "@type": "schema:DataDownload",
        "schema:contentSize": "5.6GB",
        "schema:encodingFormat": "DICOM",
        "schema:inLanguage": "en",
        "schema:name": "Images ",
        "schema:url": "https://wiki.cancerimagingarchive.net/display/Public/PROSTATE-DIAGNOSIS/download/attachments/3277254/TCIA_PROSTATE-DIAGNOSIS_06-22-2015.tcia?version=1&modificationDate=1534787404534&api=v2",
        "@context": {
          "schema": "http://schema.org/"
        }
      }
    ],
    "dct:isReferencedBy": [],
    "dct:subject": [],
    "@context": {
      "dct": "http://purl.org/dc/terms/",
      "foaf": "http://xmlns.com/foaf/0.1/",
      "datmm": "http://schema.org/"
    }
  },
  {
    "@type": "datmm:Dataset",
    "dct:description": "This collection comprises a total of 28 3 Tesla T1-weighted, T2-weighted, Diffusion weighted and Dynamic Contrast Enhanced prostate MRI along with accompanying digitized histopathology (H&Estained) images of corresponding radical prostatectomy specimens. The MRI scans also have a mapping of extent of prostate cancer on them [1]. Each surgically excised prostate specimen was originally sectioned and quartered resulting in 4 slides for each section. Each of these individual slides was digitized at 20x magnification using an Aperio slide scanner resulting in a set of 4 .svs images. Each of the 4 .svs images were then digitally stitched together to constitute a pseudo-whole mount section (.tiff) using the program in [2]. Annotations of cancer presence on the pseudo-whole mount sections were made by an expert pathologist. Slice correspondences were established between the individual T2w MRI and stitched pseudo-whole mount sections by the program in [3] and checked for accuracy by an expert pathologist and radiologist. Deformable co-registration [4] was employed to spatially co-registered the corresponding radiologic and histopathologic tissue sections to map disease extent onto the corresponding MRI scans.",
    "dct:format": "Unknown",
    "dct:issued": "11-30-2016",
    "foaf:homepage": "https://www.ncbi.nlm.nih.gov/gap",
    "dct:title": "Prostate Fused-MRI-Pathology",
    "dct:language": "English",
    "bf:contribution": [],
    "dct:isPartOf": {
      "@type": "datmm:Repository",
      "dct:alternative": "TCIA",
      "foaf:homepage": "https://www.cancerimagingarchive.net",
      "dct:title": "The Cancer Imaging Archive",
      "@context": {
        "dct": "http://purl.org/dc/terms/",
        "foaf": "http://xmlns.com/foaf/0.1/",
        "datmm": "http://schema.org/"
      }
    },
    "frapo:isSupportedBy": [],
    "schema:distribution": [
      {
        "@type": "schema:DataDownload",
        "schema:contentSize": "4.4 GB",
        "schema:encodingFormat": "DICOM",
        "schema:inLanguage": "en",
        "schema:name": "Images ",
        "schema:url": "https://wiki.cancerimagingarchive.net/display/Public/Prostate+Fused-MRI-Pathology/download/attachments/23691514/doiJNLP-auLIj9wT-Prostate_Fused-MRI-Pathologyv1.tcia?version=1&modificationDate=1534787026838&api=v2",
        "@context": {
          "schema": "http://schema.org/"
        }
      }
    ],
    "dct:isReferencedBy": [
      {
        "@type": "datmm:Documentation",
        "rdf:type": "Journal Article",
        "dct:title": "Identifying in vivo DCE MRI markers associated with microvessel architecture and gleason grades of prostate cancer.",
        "dct:bibliographicCitation": "Singanamalli A, et al. Identifying in vivo DCE MRI markers associated with microvessel architecture and gleason grades of prostate cancer. J Magn Reson Imaging",
        "prism:doi": "10.1002/jmri.24975",
        "fabio:hasPubMedId": "26110513",
        "foaf:homepage": "https://pubmed.ncbi.nlm.nih.gov/26110513",
        "dct:identifier": "26110513",
        "@context": {
          "dct": "http://purl.org/dc/terms/",
          "prism": "http://prismstandard.org/namespaces/basic/3.0/",
          "rdf": "http://www.w3.org/1999/02/22-rdf-syntax-ns#",
          "foaf": "http://xmlns.com/foaf/0.1/",
          "datmm": "http://schema.org/",
          "fabio": "http://purl.org/spar/fabio/"
        }
      }
    ],
    "dct:subject": [],
    "@context": {
      "dct": "http://purl.org/dc/terms/",
      "foaf": "http://xmlns.com/foaf/0.1/",
      "datmm": "http://schema.org/"
    }
  },
  {
    "@type": "datmm:Dataset",
    "dct:description": "This collection of prostate Magnetic Resonance Images (MRIs) was obtained with an endorectal and phased array surface coil at 3T (Philips Achieva). Each patient had biopsy confirmation of cancer and underwent a robotic-assisted radical prostatectomy. A mold was generated from each MRI, and the prostatectomy specimen was first placed in the mold, then cut in the same plane as the MRI. The data was generated at the National Cancer Institute, Bethesda, Maryland, USA between 2008-2010. For scientific or other inquiries relating to this data set, please\u00a0",
    "dct:format": "Unknown",
    "dct:issued": "2011/06/30",
    "foaf:homepage": "https://www.ncbi.nlm.nih.gov/gap",
    "dct:title": "PROSTATE-MRI",
    "dct:language": "English",
    "bf:contribution": [],
    "dct:isPartOf": {
      "@type": "datmm:Repository",
      "dct:alternative": "TCIA",
      "foaf:homepage": "https://www.cancerimagingarchive.net",
      "dct:title": "The Cancer Imaging Archive",
      "@context": {
        "dct": "http://purl.org/dc/terms/",
        "foaf": "http://xmlns.com/foaf/0.1/",
        "datmm": "http://schema.org/"
      }
    },
    "frapo:isSupportedBy": [],
    "schema:distribution": [
      {
        "@type": "schema:DataDownload",
        "schema:contentSize": "3.2GB",
        "schema:encodingFormat": "DICOM",
        "schema:inLanguage": "en",
        "schema:name": "Images ",
        "schema:url": "https://wiki.cancerimagingarchive.net/display/Public/PROSTATE-MRI/download/attachments/3277260/PROSTATE-MRI-5-18-2018-doiJNLP-dKJJAqnS.tcia?version=1&modificationDate=1534786953393&api=v2",
        "@context": {
          "schema": "http://schema.org/"
        }
      }
    ],
    "dct:isReferencedBy": [],
    "dct:subject": [],
    "@context": {
      "dct": "http://purl.org/dc/terms/",
      "foaf": "http://xmlns.com/foaf/0.1/",
      "datmm": "http://schema.org/"
    }
  },
  {
    "@type": "datmm:Dataset",
    "dct:description": "  This dataset was derived from tracked biopsy sessions using the Artemis biopsy system, many of which included image fusion with MRI targets. Patients received a 3D transrectal ultrasound scan, after which nonrigid registration (e.g. \u201cfusion\u201d) was performed between real-time ultrasound and preoperative MRI, enabling biopsy cores to be sampled from MR regions of interest.\u00a0Most cases also included sampling of systematic biopsy cores using a 12-core digital template.\u00a0The Artemis system tracked targeted and systematic core locations using encoder kinematics of a mechanical arm, and recorded locations relative to the Ultrasound scan. MRI biopsy coordinates were also recorded for most cases.\u00a0",
    "dct:format": "Unknown",
    "dct:issued": "2020/09/17",
    "foaf:homepage": "https://www.ncbi.nlm.nih.gov/gap",
    "dct:title": "Prostate MRI and Ultrasound With Pathology and Coordinates of Tracked Biopsy (Prostate-MRI-US-Biopsy)",
    "dct:language": "English",
    "bf:contribution": [],
    "dct:isPartOf": {
      "@type": "datmm:Repository",
      "dct:alternative": "TCIA",
      "foaf:homepage": "https://www.cancerimagingarchive.net",
      "dct:title": "The Cancer Imaging Archive",
      "@context": {
        "dct": "http://purl.org/dc/terms/",
        "foaf": "http://xmlns.com/foaf/0.1/",
        "datmm": "http://schema.org/"
      }
    },
    "frapo:isSupportedBy": [],
    "schema:distribution": [
      {
        "@type": "schema:DataDownload",
        "schema:contentSize": "(GB",
        "schema:encodingFormat": "DICOM",
        "schema:inLanguage": "en",
        "schema:name": "Images ",
        "schema:url": "https://wiki.cancerimagingarchive.net/pages/viewpage.action?pageId=68550661/download/attachments/68550661/Prostate-MRI-US-Biopsy-NBIA-manifest_20200910.tcia?version=1&modificationDate=1599764668817&api=v2",
        "@context": {
          "schema": "http://schema.org/"
        }
      }
    ],
    "dct:isReferencedBy": [
      {
        "@type": "datmm:Documentation",
        "rdf:type": "Journal Article",
        "dct:title": "Targeted biopsy in the detection of prostate cancer using an office based magnetic resonance ultrasound fusion device.",
        "dct:bibliographicCitation": "Sonn GA, et al. Targeted biopsy in the detection of prostate cancer using an office based magnetic resonance ultrasound fusion device. J Urol",
        "prism:doi": "10.1016/j.juro.2012.08.095",
        "fabio:hasPubMedId": "23158413",
        "foaf:homepage": "https://pubmed.ncbi.nlm.nih.gov/23158413",
        "dct:identifier": "23158413",
        "@context": {
          "dct": "http://purl.org/dc/terms/",
          "prism": "http://prismstandard.org/namespaces/basic/3.0/",
          "rdf": "http://www.w3.org/1999/02/22-rdf-syntax-ns#",
          "foaf": "http://xmlns.com/foaf/0.1/",
          "datmm": "http://schema.org/",
          "fabio": "http://purl.org/spar/fabio/"
        }
      }
    ],
    "dct:subject": [
      {
        "@type": "skos:Concept",
        "dct:identifier": "D008279",
        "skos:inScheme": "MeSH",
        "rdfs:label": "Magnetic Resonance Imaging",
        "@context": {
          "rdfs": "http://www.w3.org/2000/01/rdf-schema#",
          "skos": "http://www.w3.org/2004/02/skos/core#",
          "dct": "http://purl.org/dc/terms/"
        }
      },
      {
        "@type": "skos:Concept",
        "dct:identifier": "D018084",
        "skos:inScheme": "MeSH",
        "rdfs:label": "Ultrasonography, Interventional",
        "@context": {
          "rdfs": "http://www.w3.org/2000/01/rdf-schema#",
          "skos": "http://www.w3.org/2004/02/skos/core#",
          "dct": "http://purl.org/dc/terms/"
        }
      }
    ],
    "@context": {
      "dct": "http://purl.org/dc/terms/",
      "foaf": "http://xmlns.com/foaf/0.1/",
      "datmm": "http://schema.org/"
    }
  },
  {
    "@type": "datmm:Dataset",
    "dct:description": "\n \n The QIBA CT-1C phantom collection was designed and shared to assist in Characterizing Variability, sans Biology. This data set was contributed by RSNA's ",
    "dct:format": "Unknown",
    "dct:issued": "2011/11/28",
    "foaf:homepage": "https://www.ncbi.nlm.nih.gov/gap",
    "dct:title": "QIBA CT-1C",
    "dct:language": "English",
    "bf:contribution": [],
    "dct:isPartOf": {
      "@type": "datmm:Repository",
      "dct:alternative": "TCIA",
      "foaf:homepage": "https://www.cancerimagingarchive.net",
      "dct:title": "The Cancer Imaging Archive",
      "@context": {
        "dct": "http://purl.org/dc/terms/",
        "foaf": "http://xmlns.com/foaf/0.1/",
        "datmm": "http://schema.org/"
      }
    },
    "frapo:isSupportedBy": [],
    "schema:distribution": [
      {
        "@type": "schema:DataDownload",
        "schema:contentSize": "36.51 GB",
        "schema:encodingFormat": "DICOM",
        "schema:inLanguage": "en",
        "schema:name": "\nImages and Segmentations\u00a0",
        "schema:url": "https://wiki.cancerimagingarchive.net/display/Public/QIBA+CT-1C/download/attachments/22513061/TCIA_QIBA_CT-1C_06-22-2015.tcia?version=1&modificationDate=1534787018694&api=v2",
        "@context": {
          "schema": "http://schema.org/"
        }
      }
    ],
    "dct:isReferencedBy": [],
    "dct:subject": [],
    "@context": {
      "dct": "http://purl.org/dc/terms/",
      "foaf": "http://xmlns.com/foaf/0.1/",
      "datmm": "http://schema.org/"
    }
  },
  {
    "@type": "datmm:Dataset",
    "dct:description": "This collection contains MR images of both low and high grade glial brain lesions. Data includes post-contrast T1w images with co-registered volumes of dynamic susceptibility contrast (DSC) MR images in DICOM format. Binary regions of interest are also included, in DICOM format, of the lesion, arterial input function, normal appearing white matter, normal appearing cerebral cortex, and whole brain. The data was provided to help facilitate research activities of the National Cancer Institute's (NCI's) Quantitative Imaging Network (QIN). This collection was supported by Grant U01 CA176110.",
    "dct:format": "Unknown",
    "dct:issued": "2019/08/28",
    "foaf:homepage": "https://www.ncbi.nlm.nih.gov/gap",
    "dct:title": "QIN-BRAIN-DSC-MRI",
    "dct:language": "English",
    "bf:contribution": [],
    "dct:isPartOf": {
      "@type": "datmm:Repository",
      "dct:alternative": "TCIA",
      "foaf:homepage": "https://www.cancerimagingarchive.net",
      "dct:title": "The Cancer Imaging Archive",
      "@context": {
        "dct": "http://purl.org/dc/terms/",
        "foaf": "http://xmlns.com/foaf/0.1/",
        "datmm": "http://schema.org/"
      }
    },
    "frapo:isSupportedBy": [],
    "schema:distribution": [
      {
        "@type": "schema:DataDownload",
        "schema:contentSize": "30.8 GB",
        "schema:encodingFormat": "DICOM",
        "schema:inLanguage": "en",
        "schema:name": "Images ",
        "schema:url": "https://wiki.cancerimagingarchive.net/display/Public/QIN-BRAIN-DSC-MRI/download/attachments/21267383/QIN-BRAIN-DSC-MRI_2016-03-29.tcia?version=1&modificationDate=1542736923443&api=v2",
        "@context": {
          "schema": "http://schema.org/"
        }
      }
    ],
    "dct:isReferencedBy": [
      {
        "@type": "datmm:Documentation",
        "rdf:type": "Journal Article",
        "dct:title": "Multisite Concordance of DSC-MRI Analysis for Brain Tumors: Results of a National Cancer Institute Quantitative Imaging Network Collaborative Project.",
        "dct:bibliographicCitation": "Schmainda KM, et al. Multisite Concordance of DSC-MRI Analysis for Brain Tumors: Results of a National Cancer Institute Quantitative Imaging Network Collaborative Project. AJNR Am J Neuroradiol",
        "prism:doi": "10.3174/ajnr.A5675",
        "fabio:hasPubMedId": "29794239",
        "foaf:homepage": "https://pubmed.ncbi.nlm.nih.gov/29794239",
        "dct:identifier": "29794239",
        "@context": {
          "dct": "http://purl.org/dc/terms/",
          "prism": "http://prismstandard.org/namespaces/basic/3.0/",
          "rdf": "http://www.w3.org/1999/02/22-rdf-syntax-ns#",
          "foaf": "http://xmlns.com/foaf/0.1/",
          "datmm": "http://schema.org/",
          "fabio": "http://purl.org/spar/fabio/"
        }
      }
    ],
    "dct:subject": [],
    "@context": {
      "dct": "http://purl.org/dc/terms/",
      "foaf": "http://xmlns.com/foaf/0.1/",
      "datmm": "http://schema.org/"
    }
  },
  {
    "@type": "datmm:Dataset",
    "dct:description": "\n \n \n \n \n This collection contains longitudinal PET/CT and quantitative MR images collected for the purpose of studying treatment assessment in breast cancer in the neoadjuvant setting. Images were acquired at three time points: prior to the start of treatment (t1), after the first cycle of treatment (t2), and either after the second cycle of treatment or at the completion of all treatments (prior to surgery) (t3). The PET/CT images were acquired with a support device built in-house to allow the patient to be in the prone position to facilitate registration with the MRI data. The value of this collection is to provide clinical imaging data for the development and evaluation of quantitative imaging methods for treatment assessment early in the course of therapy for breast cancer. Data is provided by Vanderbilt University, PI Dr. Thomas E. Yankeelov.",
    "dct:format": "Unknown",
    "dct:issued": "2020/01/10",
    "foaf:homepage": "https://www.ncbi.nlm.nih.gov/gap",
    "dct:title": "QIN-Breast",
    "dct:language": "English",
    "bf:contribution": [],
    "dct:isPartOf": {
      "@type": "datmm:Repository",
      "dct:alternative": "TCIA",
      "foaf:homepage": "https://www.cancerimagingarchive.net",
      "dct:title": "The Cancer Imaging Archive",
      "@context": {
        "dct": "http://purl.org/dc/terms/",
        "foaf": "http://xmlns.com/foaf/0.1/",
        "datmm": "http://schema.org/"
      }
    },
    "frapo:isSupportedBy": [],
    "schema:distribution": [
      {
        "@type": "schema:DataDownload",
        "schema:contentSize": "11.286 GB",
        "schema:encodingFormat": "DICOM",
        "schema:inLanguage": "en",
        "schema:name": "Images ",
        "schema:url": "https://wiki.cancerimagingarchive.net/display/Public/QIN-Breast/download/attachments/18513974/QIN-BREAST_2015-09-04.tcia?version=1&modificationDate=1542735424249&api=v2",
        "@context": {
          "schema": "http://schema.org/"
        }
      }
    ],
    "dct:isReferencedBy": [],
    "dct:subject": [],
    "@context": {
      "dct": "http://purl.org/dc/terms/",
      "foaf": "http://xmlns.com/foaf/0.1/",
      "datmm": "http://schema.org/"
    }
  },
  {
    "@type": "datmm:Dataset",
    "dct:description": "This data is from a multi-site, multi-parametric quantitative MRI study of adult (18+ years old) females diagnosed with invasive breast cancer.\u00a0 Subjects all had a lesion size >1cm in longest dimension and were undergoing neoadjuvant therapy. Participants were scanned prior to any therapy and then 2-3 times after the initiation of neoadjuvant therapy, depending upon their treatment regimen.\u00a0All data sets were acquired with a research-only protocol, including: DWI (SE EPI), OGSE, qMT, B0 map, multi-flip T1 map, Bloch-Siegert B1 map, DCE, and a T1-weighted anatomical image.",
    "dct:format": "Unknown",
    "dct:issued": "changed",
    "foaf:homepage": "https://www.ncbi.nlm.nih.gov/gap",
    "dct:title": "QIN-BREAST-02",
    "dct:language": "English",
    "bf:contribution": [],
    "dct:isPartOf": {
      "@type": "datmm:Repository",
      "dct:alternative": "TCIA",
      "foaf:homepage": "https://www.cancerimagingarchive.net",
      "dct:title": "The Cancer Imaging Archive",
      "@context": {
        "dct": "http://purl.org/dc/terms/",
        "foaf": "http://xmlns.com/foaf/0.1/",
        "datmm": "http://schema.org/"
      }
    },
    "frapo:isSupportedBy": [],
    "schema:distribution": [
      {
        "@type": "schema:DataDownload",
        "schema:contentSize": "3.9 GB",
        "schema:encodingFormat": "DICOM",
        "schema:inLanguage": "en",
        "schema:name": "Images ",
        "schema:url": "https://wiki.cancerimagingarchive.net/display/Public/QIN-BREAST-02/download/attachments/52756887/QIN-BREAST-02_20190408_v1.tcia?version=1&modificationDate=1554747017546&api=v2",
        "@context": {
          "schema": "http://schema.org/"
        }
      }
    ],
    "dct:isReferencedBy": [],
    "dct:subject": [],
    "@context": {
      "dct": "http://purl.org/dc/terms/",
      "foaf": "http://xmlns.com/foaf/0.1/",
      "datmm": "http://schema.org/"
    }
  },
  {
    "@type": "datmm:Dataset",
    "dct:description": "This collection of breast dynamic contrast-enhanced (DCE) MRI data contains images from a longitudinal study to assess breast cancer response to neoadjuvant chemotherapy. Images were acquired at four time points: prior to the start of treatment (Visit 1, V1), after the first cycle of treatment (Visit 2, V2), at midpoint of treatment course (Visit 3, V3), and after completion of treatment (prior to surgery) (Visit 4, V4). The value of this collection is to provide clinical imaging data for the development and validation of quantitative imaging methods for assessment of breast cancer response to treatment. Data is provided by Oregon Health & Science University, PI Dr. Wei Huang.",
    "dct:format": "Unknown",
    "dct:issued": "2019/04/18",
    "foaf:homepage": "https://www.ncbi.nlm.nih.gov/gap",
    "dct:title": "QIN Breast DCE-MRI",
    "dct:language": "English",
    "bf:contribution": [],
    "dct:isPartOf": {
      "@type": "datmm:Repository",
      "dct:alternative": "TCIA",
      "foaf:homepage": "https://www.cancerimagingarchive.net",
      "dct:title": "The Cancer Imaging Archive",
      "@context": {
        "dct": "http://purl.org/dc/terms/",
        "foaf": "http://xmlns.com/foaf/0.1/",
        "datmm": "http://schema.org/"
      }
    },
    "frapo:isSupportedBy": [],
    "schema:distribution": [
      {
        "@type": "schema:DataDownload",
        "schema:contentSize": "15.8GB",
        "schema:encodingFormat": "DICOM",
        "schema:inLanguage": "en",
        "schema:name": "Images ",
        "schema:url": "https://wiki.cancerimagingarchive.net/display/Public/QIN+Breast+DCE-MRI/download/attachments/18514286/qin-dce-mri-challenge_DCM_NIFTI.tcia?version=1&modificationDate=1534786993310&api=v2",
        "@context": {
          "schema": "http://schema.org/"
        }
      }
    ],
    "dct:isReferencedBy": [
      {
        "@type": "datmm:Documentation",
        "rdf:type": "Journal Article",
        "dct:title": "Variations of dynamic contrast-enhanced magnetic resonance imaging in evaluation of breast cancer therapy response: a multicenter data analysis challenge.",
        "dct:bibliographicCitation": "Huang W, et al. Variations of dynamic contrast-enhanced magnetic resonance imaging in evaluation of breast cancer therapy response: a multicenter data analysis challenge. Transl Oncol",
        "prism:doi": "10.1593/tlo.13838",
        "fabio:hasPubMedId": "24772219",
        "foaf:homepage": "https://pubmed.ncbi.nlm.nih.gov/24772219",
        "dct:identifier": "24772219",
        "@context": {
          "dct": "http://purl.org/dc/terms/",
          "prism": "http://prismstandard.org/namespaces/basic/3.0/",
          "rdf": "http://www.w3.org/1999/02/22-rdf-syntax-ns#",
          "foaf": "http://xmlns.com/foaf/0.1/",
          "datmm": "http://schema.org/",
          "fabio": "http://purl.org/spar/fabio/"
        }
      }
    ],
    "dct:subject": [],
    "@context": {
      "dct": "http://purl.org/dc/terms/",
      "foaf": "http://xmlns.com/foaf/0.1/",
      "datmm": "http://schema.org/"
    }
  },
  {
    "@type": "datmm:Dataset",
    "dct:description": "\n This collection contains \u201cdouble baseline\u201d multi-parametric MRI images collected on patients with newly diagnosed glioblastoma.\u00a0 The patients were scanned after surgery but prior to the start of therapy, typically 2-5 days apart. The structural images included T1-weighted pre- and post-contrast images, T2-weighted images, FLAIR and MEMPRAGE images.\u00a0 Advanced MRI sequences included Diffusion Weighted (DW) Imaging, Dynamic Contrast-Enhanced MRI (DCE-MRI), and Dynamic Susceptibility Contrast MRI (DSC-MRI). The value of this collection is to provide clinical image data to establish the test-retest characteristics of parameters calculated from DW-MRI, DCE-MRI, and DSC-MRI such as ADC, Ktrans and rCBV. Data were provided by Dr. Elizabeth Gerstner and Dr. Kalpathy-Cramer (MGH) as part of their participation in the Quantitative Imaging Network.",
    "dct:format": "Unknown",
    "dct:issued": "2020/04/03",
    "foaf:homepage": "https://www.ncbi.nlm.nih.gov/gap",
    "dct:title": "QIN GBM Treatment Response",
    "dct:language": "English",
    "bf:contribution": [],
    "dct:isPartOf": {
      "@type": "datmm:Repository",
      "dct:alternative": "TCIA",
      "foaf:homepage": "https://www.cancerimagingarchive.net",
      "dct:title": "The Cancer Imaging Archive",
      "@context": {
        "dct": "http://purl.org/dc/terms/",
        "foaf": "http://xmlns.com/foaf/0.1/",
        "datmm": "http://schema.org/"
      }
    },
    "frapo:isSupportedBy": [],
    "schema:distribution": [
      {
        "@type": "schema:DataDownload",
        "schema:contentSize": "33.5 GB",
        "schema:encodingFormat": "DICOM",
        "schema:inLanguage": "en",
        "schema:name": "Images ",
        "schema:url": "https://wiki.cancerimagingarchive.net/display/Public/QIN+GBM+Treatment+Response/download/attachments/21267249/QIN%20GBM%20Treatment%20Response_2015-08-12.tcia?version=1&modificationDate=1542736617463&api=v2",
        "@context": {
          "schema": "http://schema.org/"
        }
      }
    ],
    "dct:isReferencedBy": [
      {
        "@type": "datmm:Documentation",
        "rdf:type": "Journal Article",
        "dct:title": "Repeatability of Standardized and Normalized Relative CBV in Patients with Newly Diagnosed Glioblastoma.",
        "dct:bibliographicCitation": "Prah MA, et al. Repeatability of Standardized and Normalized Relative CBV in Patients with Newly Diagnosed Glioblastoma. AJNR Am J Neuroradiol",
        "prism:doi": "10.3174/ajnr.A4374",
        "fabio:hasPubMedId": "26066626",
        "foaf:homepage": "https://pubmed.ncbi.nlm.nih.gov/26066626",
        "dct:identifier": "26066626",
        "@context": {
          "dct": "http://purl.org/dc/terms/",
          "prism": "http://prismstandard.org/namespaces/basic/3.0/",
          "rdf": "http://www.w3.org/1999/02/22-rdf-syntax-ns#",
          "foaf": "http://xmlns.com/foaf/0.1/",
          "datmm": "http://schema.org/",
          "fabio": "http://purl.org/spar/fabio/"
        }
      },
      {
        "@type": "datmm:Documentation",
        "rdf:type": "Journal Article",
        "dct:title": "Repeatability of Cerebral Perfusion Using Dynamic Susceptibility Contrast MRI in Glioblastoma Patients.",
        "dct:bibliographicCitation": "Jafari-Khouzani K, et al. Repeatability of Cerebral Perfusion Using Dynamic Susceptibility Contrast MRI in Glioblastoma Patients. Transl Oncol",
        "prism:doi": "10.1016/j.tranon.2015.03.002",
        "fabio:hasPubMedId": "26055170",
        "foaf:homepage": "https://pubmed.ncbi.nlm.nih.gov/26055170",
        "dct:identifier": "26055170",
        "@context": {
          "dct": "http://purl.org/dc/terms/",
          "prism": "http://prismstandard.org/namespaces/basic/3.0/",
          "rdf": "http://www.w3.org/1999/02/22-rdf-syntax-ns#",
          "foaf": "http://xmlns.com/foaf/0.1/",
          "datmm": "http://schema.org/",
          "fabio": "http://purl.org/spar/fabio/"
        }
      }
    ],
    "dct:subject": [],
    "@context": {
      "dct": "http://purl.org/dc/terms/",
      "foaf": "http://xmlns.com/foaf/0.1/",
      "datmm": "http://schema.org/"
    }
  },
  {
    "@type": "datmm:Dataset",
    "dct:description": "This collection is a set of head and neck cancer patients' multiple positron emission tomography/computed tomography (PET/CT) 18F-FDG scans\u2013before and after therapy\u2013with follow up scans where clinically indicated.\u00a0The data was provided to help facilitate research activities of the National Cancer Institute's (NCI's) Quantitative Imaging Network (QIN). This collection was supported by Grants",
    "dct:format": "Unknown",
    "dct:issued": "2020/09/15",
    "foaf:homepage": "https://www.ncbi.nlm.nih.gov/gap",
    "dct:title": "QIN-HEADNECK",
    "dct:language": "English",
    "bf:contribution": [],
    "dct:isPartOf": {
      "@type": "datmm:Repository",
      "dct:alternative": "TCIA",
      "foaf:homepage": "https://www.cancerimagingarchive.net",
      "dct:title": "The Cancer Imaging Archive",
      "@context": {
        "dct": "http://purl.org/dc/terms/",
        "foaf": "http://xmlns.com/foaf/0.1/",
        "datmm": "http://schema.org/"
      }
    },
    "frapo:isSupportedBy": [],
    "schema:distribution": [],
    "dct:isReferencedBy": [
      {
        "@type": "datmm:Documentation",
        "rdf:type": "Journal Article",
        "dct:title": "DICOM for quantitative imaging biomarker development: a standards based approach to sharing clinical data and structured PET/CT analysis results in head and neck cancer research.",
        "dct:bibliographicCitation": "Fedorov A, et al. DICOM for quantitative imaging biomarker development: a standards based approach to sharing clinical data and structured PET/CT analysis results in head and neck cancer research. PeerJ",
        "prism:doi": "10.7717/peerj.2057",
        "fabio:hasPubMedId": "27257542",
        "foaf:homepage": "https://pubmed.ncbi.nlm.nih.gov/27257542",
        "dct:identifier": "27257542",
        "@context": {
          "dct": "http://purl.org/dc/terms/",
          "prism": "http://prismstandard.org/namespaces/basic/3.0/",
          "rdf": "http://www.w3.org/1999/02/22-rdf-syntax-ns#",
          "foaf": "http://xmlns.com/foaf/0.1/",
          "datmm": "http://schema.org/",
          "fabio": "http://purl.org/spar/fabio/"
        }
      }
    ],
    "dct:subject": [],
    "@context": {
      "dct": "http://purl.org/dc/terms/",
      "foaf": "http://xmlns.com/foaf/0.1/",
      "datmm": "http://schema.org/"
    }
  },
  {
    "@type": "datmm:Dataset",
    "dct:description": "The Computed tomography (CT) Image data was obtained on patients diagnosed with Non-Small Cell Lung Cancer (NSCLC) with mixed stage & histology from the H. Lee Moffitt Cancer Center and Research Institute. Scans were obtained from patients who underwent surgical resection and had corresponding pre-surgery diagnostic CTs. The scans were de-identified following HIPPA guidelines to protect patient privacy. The data was shared with the QIN collaborators for research purpose complying with collaborative data sharing policy of the H. Lee Moffitt Total Cancer Care (TCC) .",
    "dct:format": "Unknown",
    "dct:issued": "2017/07/31",
    "foaf:homepage": "https://www.ncbi.nlm.nih.gov/gap",
    "dct:title": "QIN LUNG CT",
    "dct:language": "English",
    "bf:contribution": [],
    "dct:isPartOf": {
      "@type": "datmm:Repository",
      "dct:alternative": "TCIA",
      "foaf:homepage": "https://www.cancerimagingarchive.net",
      "dct:title": "The Cancer Imaging Archive",
      "@context": {
        "dct": "http://purl.org/dc/terms/",
        "foaf": "http://xmlns.com/foaf/0.1/",
        "datmm": "http://schema.org/"
      }
    },
    "frapo:isSupportedBy": [],
    "schema:distribution": [
      {
        "@type": "schema:DataDownload",
        "schema:contentSize": "2.08GB",
        "schema:encodingFormat": "DICOM",
        "schema:inLanguage": "en",
        "schema:name": "Images ",
        "schema:url": "https://wiki.cancerimagingarchive.net/display/Public/QIN+LUNG+CT/download/attachments/19039647/QIN_LUNG_CT_B2-doiJNLP-XGGYZcSr.tcia?version=1&modificationDate=1534787001274&api=v2",
        "@context": {
          "schema": "http://schema.org/"
        }
      }
    ],
    "dct:isReferencedBy": [],
    "dct:subject": [],
    "@context": {
      "dct": "http://purl.org/dc/terms/",
      "foaf": "http://xmlns.com/foaf/0.1/",
      "datmm": "http://schema.org/"
    }
  },
  {
    "@type": "datmm:Dataset",
    "dct:description": "\n \n This collection consists of positron emission tomography (PET) phantom scans originally utilized by the Quantitative Imaging Network (QIN) PET Segmentation Challenge to assess the variability of segmentations and subsequently derived quantitative analysis results on phantom PET scans with known ground truth.",
    "dct:format": "Unknown",
    "dct:issued": "2014/09/04",
    "foaf:homepage": "https://www.ncbi.nlm.nih.gov/gap",
    "dct:title": "QIN PET Phantom",
    "dct:language": "English",
    "bf:contribution": [],
    "dct:isPartOf": {
      "@type": "datmm:Repository",
      "dct:alternative": "TCIA",
      "foaf:homepage": "https://www.cancerimagingarchive.net",
      "dct:title": "The Cancer Imaging Archive",
      "@context": {
        "dct": "http://purl.org/dc/terms/",
        "foaf": "http://xmlns.com/foaf/0.1/",
        "datmm": "http://schema.org/"
      }
    },
    "frapo:isSupportedBy": [],
    "schema:distribution": [
      {
        "@type": "schema:DataDownload",
        "schema:contentSize": "0.246GB",
        "schema:encodingFormat": "DICOM",
        "schema:inLanguage": "en",
        "schema:name": "Images ",
        "schema:url": "https://wiki.cancerimagingarchive.net/display/Public/QIN+PET+Phantom/download/attachments/18514787/TCIA_QIN_PET_Phantom_06-22-2015.tcia?version=1&modificationDate=1534787432834&api=v2",
        "@context": {
          "schema": "http://schema.org/"
        }
      },
      {
        "@type": "schema:DataDownload",
        "schema:encodingFormat": "DICOM",
        "schema:inLanguage": "en",
        "schema:name": "DICOM Metadata Digest ",
        "schema:url": "https://wiki.cancerimagingarchive.net/display/Public/QIN+PET+Phantom/download/attachments/18514787/QIN%20PET%20Phantom_MetaData.csv?version=1&modificationDate=1495728442496&api=v2",
        "@context": {
          "schema": "http://schema.org/"
        }
      }
    ],
    "dct:isReferencedBy": [],
    "dct:subject": [],
    "@context": {
      "dct": "http://purl.org/dc/terms/",
      "foaf": "http://xmlns.com/foaf/0.1/",
      "datmm": "http://schema.org/"
    }
  }
]